[Term]
id: DBO:0000001
name: Dog Breed
def: "There are more than 400 purebred dogs in the world. The American Kennel Club (AKC) only recognizes purebreds and classifies the breeds to organize the massive list. Each breed's ideal physical traits, movement, and temperament are set down in a written document called a "breed standard". For example, the breed standard sets forth the traits that make a Cocker Spaniel a Cocker Spaniel and not a Springer Spaniel." []

[Term]
id: DBO:0000002
name: Sporting Group
def: "Breeds in the Sporting Group were bred to assist hunters in the capture and retrieval of feathered game. Retrievers, built for swimming, specialize in waterfowl, while the hunting grounds of setters, spaniels, and pointing breeds are grasslands where quail, pheasant, and other game birds nest. Many Sporting Group breeds possess thick, water-repellant coats resistant to harsh hunting conditions." []
is_a: DBO:0000001 ! Dog Breed

[Term]
id: DBO:0000003
name: Hound Group
def: "All breeds in the Hound Group were bred to pursue warm-blooded quarry. The sleek, long-legged sighthounds use explosive speed and wide vision to chase swift prey, like jackrabbits and antelope, while tough, durable scenthounds rely on their powerful noses to trail anything from raccoons to escaped convicts. Members of the Hound Group possess strong prey drives and often will stop at nothing to catch their quarries." []
is_a: DBO:0000001 ! Dog Breed

[Term]
id: DBO:0000004
name: Working Group
def: "Breeds in the Working Group are dogkind's punch-the-clock, blue-collar workers, and the group includes some of the world's most ancient breeds. They were developed to assist humans in some capacity—including pulling sleds and carts, guarding flocks and homes, and protecting their families—and many of these breeds are still used as working dogs today. Breeds in the Working Group tend to be known for imposing stature, strength, and intelligence." []
is_a: DBO:0000001 ! Dog Breed

[Term]
id: DBO:0000005
name: Terrier Group
def: "The feisty, short-legged breeds in the Terrier Group were first bred to go underground in pursuit of rodents and other vermin. Long-legged terrier breeds dig out varmints rather than burrowing in after them, while the group's "bully" breeds, created long ago for ghastly pursuits like bull-baiting, are popular companion dogs today. Breeds in the Terrier Group are excellent competitors in the sport of Earthdog." []
is_a: DBO:0000001 ! Dog Breed

[Term]
id: DBO:0000006
name: Companion and Companion and Toy Group
def: "From FCI Group 9."[]
is_a: DBO:0000001 ! Dog Breed

[Term]
id: DBO:0000007
name: Non-Sporting Group
def: "The breeds of the Non-Sporting Group have two things in common: wet noses and four legs. After that, there's not much shared by this patchwork group of breeds whose job descriptions defy categorization in the six other groups, though they all have fascinating histories. Today, the varied breeds of the Non-Sporting Group are largely sought after as companion animals, as they were all developed to interact with people in some capacity." []
is_a: DBO:0000001 ! Dog Breed

[Term]
id: DBO:0000008
name: Herding Group
def: "The Herding Group comprises breeds developed for moving livestock, including sheep, cattle, and even reindeer. Herding dogs work closely with their human shepherds, and their natural intelligence and responsiveness make them highly trainable. Today, some Herding breeds, such as the German Shepherd Dog, are commonly trained for police work. The high levels of energy found in Herding Group breeds means finding them a job is recommended so they don't begin herding children at home." []
is_a: DBO:0000001 ! Dog Breed

[Term]
id: DBO:0000009
name: Miscellaneous
def: "The breeds currently eligible to participate in the Miscellaneous Class Class are still enrolled in the AKC Foundation Stock Service. FSS enrollment is maintained until the AKC Board of Directors accepts the breed for regular status. Authorities acknowledge that throughout the world there are several hundred distinct breeds of purebred dogs, not all of which are AKC recognized breeds." []
is_a: DBO:0000001 ! Dog Breed

[Term]
id: DBO:0000010
name: Foundation Stock Service
def: "The AKC provides this service to allow these purebred breeds to continue to develop while providing them with the security of a reliable and reputable avenue to maintain their records. FSS® breeds are not eligible for AKC registration. Most of the FSS breeds are approved to compete in AKC Companion Events. Contact information is available for a majority of the Foundation Stock Service® breeds. The AKC does not recommend one club over another. None of the clubs are affiliated with the AKC at this time (except for the Coonhound national breed clubs)." []
is_a: DBO:0000001 ! Dog Breed

[Term]
id: DBO:0000011
name: Extinct
def: "From Wikipedia, the free encyclopedia" []
is_a: DBO:0000001 ! Dog Breed

[Term]
id: DBO:0000442
name: Gun Group
def: "Many Gun Dog breeds were already in use by hunters before the advent of hunting with firearms. Originally used to hunt a variety of game types, today's Gun Dogs are primarily used to hunt birds. The dogs in this Group can be roughly subdivided into four often overlapping categories, based on their primary usage: Retrievers, Pointers, Setters and Flushing Spaniels.[UKC]"[]
is_a: DBO:0000001 ! Dog Breed

[Term]
id: DBO:0000012
name: Affenpinshcher(Monkey Terrier)
def: "1936;The Affenpinscher was officially recognized by the AKC." []
is_a: DBO:0000006 ! Companion and Toy Group
synonym: "Affen" EXACT[]
synonym: "Affie" EXACT[]
synonym: "Monkey Dog" EXACT[]

[Term]
id: DBO:0000013
name: Afghan Hound
def: "This is a very old breed. In fact, some authorities maintain that the Afghan Hound is the oldest breed of purebred dogs. (An ancient myth says that a brace of Afghan Hounds represented the canine species on Noah's Ark.) Because the breed predates written history by a few thousand years, and because it was developed in some of the world's most remote locales, its exact time and place of origin within the vast area that is now Afghanistan, India, and Pakistan will never be known. What we do know is that for centuries Afghans were rugged, fleet-footed hunting companions and status symbols of royals, tribal chieftains, and aristocrats in Asia's mountain kingdoms. Afghan Hounds belong to the subcategory of hound breeds known as sighthounds, dogs who rely on their panoramic vision and explosive speed to spot and pursue their prey.;A fixture of Eastern culture since the dawn of civilization, the Afghan hound didn't make its entrance on the stage of Western history until the late 1800s. It was then that English officers returning from the British Empire's farthest corners introduced the breed to Europe. By the early 1900s, the Afghan was a preferred breed of the British gentry.;The AKC registered its first of the breed in 1927, but not until the early '30s did the breed really catch on with U.S. breeders and owners. Among the most important dogs of those early years in America were a breeding pair imported from England by Zeppo Marx, the youngest of the wacky Marx Brothers. Since then, the Afghan's fame in America has been built on his sterling qualities as a pet and his show-stopping presence in the ring. The giant sculpture by Pablo Picasso in Chicago's Daley Plaza depicts Kabul, the artist's much-loved Afghan Hound.1926;The Afghan Hound was officially recognized by the AKC" []
is_a: DBO:0000003 ! Hound Group

[Term]
id: DBO:0000014
name: Airedale Terrier
def: "1888;The Airedale Terrier was officially recognized by the AKC" []
is_a: DBO:0000005 ! Terrier Group
synonym: "Airedale" EXACT[]
synonym: "King of Terriers" EXACT[]

[Term]
id: DBO:0000015
name: Akita
def: "1972;The Akita was officially recognized by the AKC" []
is_a: DBO:0000004 ! Working Group

[Term]
id: DBO:0000016
name: Alaskan Malamute
def: "1935;The Alaskan Malamute was officially recognized by the AKC." []
is_a: DBO:0000004 ! Working Group
synonym: "Mal or Mally" EXACT[]

[Term]
id: DBO:0000017
name: American English Coonhound
def: "2011;The American English Coonhound was officially recognized by the AKC" []
is_a: DBO:0000003 ! Hound Group

[Term]
id: DBO:0000018
name: American Eskimo Dog
def: "1994;The American Eskimo was officially recognized by the AKC" []
is_a: DBO:0000007 ! Non-Sporting Group
synonym: "Eskie" EXACT[]

[Term]
id: DBO:0000019
name: American Foxhound
def: "1886;The American Foxhound was officially recognized by the AKC" []
is_a: DBO:0000003 ! Hound Group
synonym: "Foxhound" EXACT[]

[Term]
id: DBO:0000020
name: American Hairless Terrier
def: "2016;The American Hairless Terrier was officially recognized by the AKC" []
is_a: DBO:0000005 ! Terrier Group
synonym: "AHT" EXACT[]

[Term]
id: DBO:0000021
name: American Staffordshire Terrier
def: "The Staffordshire Terrier's ancestor, the bull and terrier was first bred in the nineteenth century in Birmingham. The early ancestors of this breed came from England where, until the first part of the 19th century, the Bulldog was bred. Bulldogs pictured as late as 1870 resemble the Staffordshire Terrier's ancestor, the contemporary American Staffordshire Terriers, to a greater degree than present-day Bulldogs. Some writers contend it was the White English Terrier, Fox Terrier, or the Black and Tan Terrier that was crossed with the Bulldog to develop the Staffordshire Bull Terrier; all three breeds shared many traits, the greatest differences being in color and spirit. The cross of Bulldog and Terrier was called by several names, including Bull-and-Terrier Dog, "Pit Bull Terrier" (Bull terrier used to fight on pit), or Half and Half.Later, it assumed the name of Staffordshire Bull Terrier in England. These dogs began to find their way into America as early as 1850. It became a new breed and was recognized by the United Kennel Club in 10 February, 1898, with the name American Pit Bull Terrier. In 1936 50 Ukc registered pit bulls were accepted for registration in the American Kennel Club (AKC) Stud Book as Staffordshire Terriers with a new standard and purpose, belonging to the terrier and molosser groups. The name of the breed was revised January 1, 1969 to American Staffordshire Terrier; breeders in the United States of America had developed a variety which was heavier in weight than the Staffordshire Bull Terrier of England. The name change was to distinguish them as separate breeds.;The breed's popularity began to decline in the United States following World War II.;1936;The American Staffordshire Terrier was officially recognized by the AKC (From wikipedia)" []
is_a: DBO:0000005 ! Terrier Group
synonym: "AmStaff" EXACT[]

[Term]
id: DBO:0000022
name: American Water Spaniel
def: "1940;The American Water Spaniel was officially recognized by the AKC" []
is_a: DBO:0000002 ! Sporting Group
synonym: "AWS" EXACT[]

[Term]
id: DBO:0000023
name: Anatolian Shepherd Dog
def: "1996;The Anatolian Shepherd Dog was officially recognized by the AKC" []
is_a: DBO:0000004 ! Working Group

[Term]
id: DBO:0000024
name: Appenzeller Sennenhunde
def: "The Appenzeller Sennenhund is descended from the general Sennenhund type which may have existed in antiquity, or descended from "cattle dogs left there by the Romans",but the first breed club for the breed was founded and the stud book for the breed started in 1906 by Albert Heim and others, who wrote the first breed standard in 1916. An early reference to the breed's predecessors was made in an 1853 book, "Tierleben der Alpenwelt" (Animal Life in the Alps), referring to dogs in the Appenzell region. The Appenzeller Sennenhund was only recognised internationally as a separate breed in 1989.;The Appenzeller Sennenhund was originally kept primarily as a cattle herding dog, and a flock guardian. It was also used as a draft dog, and general farm dog. The breed also was known for its affinity to both herd and guard with such devotion that they would give their life to protect their charge. Today the breed is primarily kept as a companion, and excels in agility/flyball competitions, obedience competitions and Schutzhund. They are also still used in many places as working cattle dogs even now. They are highly intelligent, and learn quickly. (From wikipedia)" []
is_a: DBO:0000010 ! Foundation Stock Service

[Term]
id: DBO:0000025
name: Australian Cattle Dog
def: "1980;The Australian Cattle Dog was officially recognized by the AKC" []
is_a: DBO:0000008 ! Herding Group

[Term]
id: DBO:0000026
name: Australian Shepherd
def: "1991;The Australian Shepherd was officially recognized by the AKC" []
is_a: DBO:0000008 ! Herding Group

[Term]
id: DBO:0000027
name: Australian Terrier
def: "1960;The Australian Terrier was officially recognized by the AKC" []
is_a: DBO:0000005 ! Terrier Group
synonym: "Aussie" EXACT[]

[Term]
id: DBO:0000028
name: Azawakh
def: "The original homeland of the Azawakh, are the endless arid regions of the south Sahara and the Sahel zone. Geographically encompassing the border region of Mali and Niger, lies the center of the Azawakh Valley. Found here are most of the types of examples of the breed. Traditionally owned by the blue-clad Tuareg nomads, they are called, "idii n' illeli" (Translated from the native tongue, this means, "sighthound of the free people."). The Azawakh enjoy a special appreciation from the nomads. They live under the same roof and are fully accepted members of the family. They assume the duty of protecting the encampment and flocks from invaders. They are passionate hunters and provide the family with meat, however, the diminishing of game and usage of firearms, lessens the utilization of the dogs. The preferred prey is a hare, antelope, and wild boar. It is here the dog can utilize their agility and stamina. The rough and broken terrain is no hindrance. In spite of their fine-limbness, they are not prone to injury.1997;The Azawakh was first recorded in the Foundation Stock Service." []
is_a: DBO:0000009 ! Miscellaneous

[Term]
id: DBO:0000029
name: Barbet(French Water Dog)
def: "The Barbet is more than a versatile gun dog. It is a joyful, smart, loving, and devoted breed. The Barbet was originally a water dog and was primarily used in France for hunting water game, as mentioned in 16th century scripts. Other references to the breed are throughout history, doing various jobs with historical lineage, always referenced with respect and admiration.;After the World Wars, the Barbet was nearly extinct, but through the efforts of a very devoted few, this old breed is slowly being reborn as a dog for the future. These loving canines, although rare and in small numbers, continue to delight and amaze people around the world. Keen intellect, propensity for water and versatile abilities make it an "all round" dog. With such an extensive historical lineage, the Barbet is a timeless and classic breed of canine.2007;The Barbet has been recorded in the Foundation Stock Service since 2007." []
is_a: DBO:0000009 ! Miscellaneous

[Term]
id: DBO:0000030
name: Basenji(African Barkless Dog)
def: "1943;The Basenji was officially recognized by the AKC" []
is_a: DBO:0000003 ! Hound Group

[Term]
id: DBO:0000031
name: Basset Fauve de Bretagne(Fawn Brittany Basset)
def: "The breed was developed in France as a hunting dog from the larger Grand Fauve de Bretagne, a breed that is now extinct. There was a rumour that the Basset Fauve de Bretagne was also close to extinction after the Second World War, and the breed was recreated using the remaining examples of the breed and crossing in Petit Basset Griffon Vendéen and standard wirehaired Dachshunds. However, the French club denies this, and says that Basset Fauve numbers were never so low. The middle breed, the Griffon Fauve de Bretagne, still exists but it is certainly rarer than the Basset. The breed in the UK is mainly seen as a show dog and family pet, finally coming off the Kennel Club's rare breed register in 2007. It can also be found in other parts of Europe where it is used to scent trail and also as a family pet. They are loving, happy, outgoing dogs and are good with children, but it must be remembered that they are scent hounds and do retain their love of the hunt so may not suit every family. In the UK the breed has no hereditary faults; however, epilepsy has been identified in some breeding lines in France and other parts of Europe. Some Fauves are born with black in the coat; this may or may not go with maturity. It is less common to see them with white patches but when they do occur it is generally confined to the chest and top of the head. However, even though the black ticking and white patches are not accepted colours, of course it does not interfere with their hunting ability, which is their prime job, and so these colour Fauves are still seen and occur fairly often in litters. The correct colour for a Fauve is anything from fawn to red but it should be solid with darker shaded ears.(From wikipedia);2015;The Basset Fauve de Bretagne has been recorded in the Foundation Stock Service since February 2015." []
is_a: DBO:0000010 ! Foundation Stock Service

[Term]
id: DBO:0000032
name: Basset Hound
def: "1935;The Basset Hound was officially recognized by the AKC" []
is_a: DBO:0000003 ! Hound Group

[Term]
id: DBO:0000033
name: Bavarian Mountain Scent Hound
def: "The German Bracken were the original hunting dogs, having "the finest nose" and a strongly developed will to follow scents and trails, but only the most reliable and perseverant Bracken were put on leash to find the lost trail of hunted game. From these particular Bracken, all Liam Hounds (Leithunde) and Leashhounds (Schweisshunde) were bred, including the Bayerischer Gebirgsschweisshund (Bavarian Mountain Scent Hound).;Toward the end of the Eighteenth Century and beginning of the Nineteenth, the Hanoverian Scenthound had evolved and was the breed of choice by hunters in lower elevations. After the Revolution of 1848 and the advancements in hunting and firearms, a dog was needed for "after the shot" to track down injured game in the more mountainous regions. The heavy Hanoverian Scenthound was not suitable for the task. To fill this need of a lighter, more agile hound, in the 1870s, Baron Karg-Bebenburg, Reichenhall, crossed a Hanoverian Scenthound with a red Mountain Scenthound to achieve what became the Bavarian Mountain Scenthound. In 1912, the Club for Bavarian Mountain Scenthounds was established in Munich, Germany and is the only recognized club for the breed in that country.;Today, these dogs are the quintessential hunting companion for professional hunters and gamekeepers. Though still rare, there is growing interest in this breed, with clubs in multiple countries including Great Britain and the United States, as well as Germany..2016;The Bavarian Mountain Scent Hound has been recorded in the Foundation Stock Service since October 2016." []
is_a: DBO:0000010 ! Foundation Stock Service

[Term]
id: DBO:0000034
name: English Beagle
def: "1885;The Beagle was officially recognized by the AKC." []
is_a: DBO:0000003 ! Hound Group

[Term]
id: DBO:0000035
name: Bearded Collie
def: "1976;The Bearded Collie was officially recognized by the AKC." []
is_a: DBO:0000008 ! Herding Group
synonym: "Beardie" EXACT[]

[Term]
id: DBO:0000036
name: Beauceron(French Short-Haired Shepherd Dog)
def: "2007;The Beauceron was officially recognized by the AKC." []
is_a: DBO:0000008 ! Herding Group

[Term]
id: DBO:0000037
name: Bedlington Terrier
def: "1886;The Bedlington Terrier was officially recognized by the AKC." []
is_a: DBO:0000005 ! Terrier Group

[Term]
id: DBO:0000038
name: Belgian Laekenois
def: "In September of 1891, the Belgian Shepherd Dog Club (Club du Chien de Berger Beige) was organized to investigate the characteristics of the native dogs in Belgium. They defined the consistent type of this native dog that was identical in body and temperament but differing in coat (color, texture and length).;During the early part of the twentieth century, the owners and breeders in Belgium urged the acceptance of additional varieties based on the color and regions of origin. The fawn rough haired varieties were given the name Laekenois (derived from the town of Laeken). The abilities of these dogs as intelligent and versatile workers soon gained popularity in other countries.;The Laekenois' original duty, in addition to guarding and tending the flock, was to guard linen drying in the fields. He was an enthusiast worker and a quick learner that made him a desirable choice for the task at hand. He was later called on to serve as a messenger dog during World War I and II. At this time his numbers were severely decreased. Many breeders worked very hard to restore this variety, while retaining the typical Belgian Shepherd Dog intelligence, type and structure. He is admired today for these attributes. He is still able to herd and guard his flock, and protect his people and their property. His ability to adapt to new situations and to respond to his master's commands makes him an alert, intelligent, inquisitive animal. He typically is reserved with strangers.1998;The Belgian Laekenois was first recorded in the Foundation Stock Service." []
is_a: DBO:0000009 ! Miscellaneous

[Term]
id: DBO:0000039
name: Belgian Malinois
def: "1959;The Belgian Malinois was officially recognized by the AKC." []
is_a: DBO:0000008 ! Herding Group

[Term]
id: DBO:0000040
name: Belgian Shepherd Dog
def: "1912;The Belgian Shepherd was officially recognized by the AKC." []
is_a: DBO:0000008 ! Herding Group

[Term]
id: DBO:0000041
name: Belgian Tervuren
def: "1959;The Belgian Tervuren was officially recognized by the AKC" []
is_a: DBO:0000008 ! Herding Group

[Term]
id: DBO:0000042
name: Bergamasco Shepherd Dog
def: "2015;The Bergamasco Sheepdog was officially recognized by the AKC" []
is_a: DBO:0000008 ! Herding Group

[Term]
id: DBO:0000043
name: Berger Picard
def: "2015;The Berger Picard was officially recognized by the AKC." []
is_a: DBO:0000008 ! Herding Group

[Term]
id: DBO:0000044
name: Bernese Mountain Dog
def: "1937;The Bernese Mountain Dog was officially recognized by the AKC" []
is_a: DBO:0000004 ! Working Group
synonym: "Berner" EXACT[]

[Term]
id: DBO:0000045
name: Bichon Frise
def: "1972;The Bichon Frise was officially recognized by the AKC" []
is_a: DBO:0000007 ! Non-Sporting Group

[Term]
id: DBO:0000046
name: Biewer Terrier
def: "The heritage of the Biewer Terrier has been an interesting and much discussed topic over the years. It started with Mr. and Mrs. Biewer, who instead of having children, bred, raised, sold, and showed Yorkshire Terriers. They had a very large and successful breeding program throughout the 1970s and into the '80s. By 1981, their enthusiasm for showing the standard Yorkshire Terriers tapered off.;The first documented black, white and tan puppy born was Schneeflockchen von Friedheck on January 20, 1984. Three months later, another black, white and tan puppy was born named Schneeman. These puppies were unique and rare, as they possessed the recessive piebald gene, a gene not usually found in Yorkies. During a visit one day, their vet and friend, Dr. Bardeleben, suggested they name the dogs after Mrs. Biewer. They chuckled as they contemplated the name, "Gertrud Biewer Yorkshire Terrier." After much consideration, they found the "Biewer Yorkshire Terrier" to be a more suitable name. Documentation shows that both of these puppies were sold to the famous German singer, Margot Eskens, who suggested adding "a la Pom Pon" to their name. The Biewer Yorkshire Terrier a la Pom Pon made its actual public debut in 1986.;The demand was hard to meet for these exclusive dogs, as the Biewer family did not produce many Biewer-type dogs and they were very selective where their dogs were placed. Many breeders tried to replicate the "Biewer Dog" by mixing other breeds together. It wasn't long before Mr. Biewer became ill and was unable to help Mrs. Biewer carry on the dream they had set out to accomplish for the Biewer breed. Sadly, Mrs. Biewer soon phased out their breeding program in order to better care for her husband during his illness.;The Biewer Terrier was introduced into mainstream America in 2003, at which time there were only a handful of breeders, both in Germany and the US alike. Noticing the development story of the Biewer did not match the dogs coming in from Germany, Myrna Torres and Gayle Pruett, now the BTCA president and director, respectively, contacted Mars Veterinary to see if they could help them determine if the Biewer was a Yorkshire Terrier or a purebred due to the introduction of other breeds. Mars Veterinary accepted the challenge and so began the process proving the Biewer Terrier a purebred dog and establishing it as such.;This is the first time in the history of dog breeding that a dog has been proven to be a purebred using the tools science has to offer. The Biewer Terrier was now established as a purebred dog through the collection of genetic data rather than through pedigree documentation as is customary.;2014;The Biewer Terrier was recorded in the Foundation Stock Service" []
is_a: DBO:0000010 ! Foundation Stock Service

[Term]
id: DBO:0000047
name: American Black and Tan Coonhound
def: "1945;The Black and Tan Coonhound was officially recognized by the AKC" []
is_a: DBO:0000003 ! Hound Group

[Term]
id: DBO:0000048
name: Black Russian Terrier
def: "2004;The Black Russian Terrier was officially recognized by the AKC" []
is_a: DBO:0000004 ! Working Group

[Term]
id: DBO:0000049
name: Bloodhound
def: "1885;The Bloodhound was officially recognized by the AKC" []
is_a: DBO:0000003 ! Hound Group

[Term]
id: DBO:0000050
name: Bluetick Coonhound
def: "2009;The Bluetick Coonhound was officially recognized by the AKC" []
is_a: DBO:0000003 ! Hound Group

[Term]
id: DBO:0000051
name: Boerboel(South African Mastiff)
def: "2015;The Boerboel was officially recognized by the AKC." []
is_a: DBO:0000004 ! Working Group

[Term]
id: DBO:0000052
name: Bolognese
def: "The Bolognese was developed centuries ago in Bologna, Italy, and it is written that they were already valued in Italy as early as the Eleventh and Twelfth centuries. Because of its beauty, grace and charm, it became a favorite of the nobility during the Renaissance. King Umberto of Italy gave a beautiful little Bolognese to Princess Jose of Belgium on her birthday. Also, in 1668 Cosimo de Medici sent eight Bolognese by royal courier and asked his friend Colonel Alamanni in Belgium that these be given as gifts to several of the wealthy and influential families of Brussels.;As time passed and the nobility passed along with it, the Bolognese went almost extinct. A few breeders in Europe, however, and especially one man in Italy, Gian Franco Giannelli, who loved the breed, restored it to its present-day popularity. The breed was brought into England by Liz Stannard in 1990 and first shown that year in Imported Register classes. In 2001, the breed was able to be shown at all shows with their own classes and, in 2002, they were at Crufts dog show for the first time." []
is_a: DBO:0000010 ! Foundation Stock Service

[Term]
id: DBO:0000053
name: Border Collie
def: "1995;The Border Collie was officially recognized by the AKC" []
is_a: DBO:0000008 ! Herding Group

[Term]
id: DBO:0000054
name: Border Terrier
def: "1930;The Border Terrier was officially recognized by the AKC." []
is_a: DBO:0000005 ! Terrier Group

[Term]
id: DBO:0000055
name: Borzoi(Russian wolfhound)
def: "1891;The Borzoi was officially recognized by the AKC" []
is_a: DBO:0000003 ! Hound Group

[Term]
id: DBO:0000056
name: Boston Terrier
def: "1893;The Boston Terrier was officially recognized by the AKC" []
is_a: DBO:0000007 ! Non-Sporting Group

[Term]
id: DBO:0000057
name: Bouvier des Flandres(Flanders Cattle Dog)
def: "1931;The Bouvier des Flandres was officially recognized by the AKC." []
is_a: DBO:0000008 ! Herding Group

[Term]
id: DBO:0000058
name: German Boxer
def: "1904;The Boxer was officially recognized by the AKC" []
is_a: DBO:0000004 ! Working Group

[Term]
id: DBO:0000059
name: Boykin Spaniel
def: "2009;The Boykin Spaniel was officially recognized by the AKC." []
is_a: DBO:0000002 ! Sporting Group

[Term]
id: DBO:0000060
name: Bracco Italiano(Italian Pointer)
def: "The Bracco Italiano has been called the oldest European pointer, and its history reaches back to the fourth or fifth century BC. While the exact ancestral origins are unknown, it is generally accepted that the Bracco Italiano was first a cross between the Segugio Italiano and the Asiatic Mastiff, which has since become extinct. The breed was developed in northern Italy, with two distinct varieties: the white-and-orange-colored variety known to be from the Piedmont region and the roan-and-brown from Lombardy.;By the medieval period, the breed had become well-established and the Italian aristocracy exported the Bracco across the Old World. The Bracco's popularity peaked during the Renaissance, and they remained at healthy numbers until the turn of the twentieth century, when they faced a sharp decline.;By the end of the 1800s, the Bracco Italiano faced extinction. Over the years, crossing with hounds and poor breeding resulted in dogs that were too heavily built to perform their work, and the breed suffered from various health problems. Diligent breeding selection and care aided in rebuilding the breed. In the 1920s, it was decided to unify the two variations of the breed in order to preserve genetic diversity.;First, the Piedmontese Pointer was a dog of lighter construction and color, and it originated in the Piedmont region of Italy, as its name suggests. This dog was used for work in the mountains, which its conformation and temperament reflected. The Piedmontese dog was smaller than its counterpart in Lombardy, and its hunting style was reminiscent of some western European pointers in that it traveled with a jaunty gallop. This dog was primarily white, with or without orange markings.;Alternately, the Lombard Pointer was a rich brown roan and had a heavier body type. This dog was used for hunting in the marshy lowlands, and was a trotting breed. These big dogs were bred both for their eye appeal and natural hunting ability.;Shortly after the breed was officially unified, the working standard was written and released, and in 1949 the Societa Amatori Bracco Italiano was founded in Italy. When the Italian conformation standard was published, it incorporated aspects of both breed types, resulting in noted variability within the standard. The breed standard had existed for over a century prior to being compiled into this single document.;The Bracco Italiano was brought to the United Kingdom in the late 1980s, however the United States did not experience the Italian Pointer until approximately 1994. In 2001, the Bracco was accepted into the AKC Foundation Stock Service. In 2005, the first national "Gathering" was held, and the Bracco Italiano Club of America was founded in 2007..2001;The Bracco Italiano was recorded in the Foundation Stock Service" []
is_a: DBO:0000010 ! Foundation Stock Service

[Term]
id: DBO:0000061
name: Braque du Bourbonnais(Bourbonnais Pointer)
def: "The Bourbonnais Pointing Dog was already known in 1598 ("Natural History", Aldovrandi National Library).The ancient authors described him as a pleasant companion of the hunter, of hardy and healthy appearance. His white coat is entirely covered with fine brown or fawn ticking.The breeders of the 1930's wanted to impose a "faded lilac" coloured coat along with the obligation of being born with a naturally short tail. This strict selection put the existence of the breed in danger. In the 1970's, a team of breeders decided to work for the survival of the Bourbonnais Pointing Dog.The present state of the breed allows us to be confident about the future of the breed.. 2011;The Braque du Bourbonnais was recorded in the Foundation Stock Service" []
is_a: DBO:0000010 ! Foundation Stock Service

[Term]
id: DBO:0000062
name: Braque Francais Pyrenean(French Pointing Dog-Pyrenean type)
def: "The Braque Français, in general, descends from an old type of gun dog used to point the location of game birds, specifically the Old Spanish Pointer and the now extinct Southern Hound. They have existed since the 15th century.Over time, this hunting breed was taken to other countries and crossed with other breeds. At the end of the 19th century, a search began to find the original dogs and two separate varieties were found. The Gascony type were the heavier, larger size and were considered truer to their classic gun dog fathers and grandfathers. The Pyrenean type dogs were bred by hunters wanting a leaner, faster version of the classic Braque Français.;Interest grew in these rustic hunting dogs, so by the early 20th century, the first breed club formed. They decided to support both varieties of Braque Français with separate standards for each.;Today, the Pyrenean Type is the most popular French Pointing Dog in its native country of France, with small, devoted followings in Canada and the US as well. He is recognized by the French Kennel Club at home and the FCI internationally.2016;The Braque Francais Pyrenean has been recorded in the Foundation Stock Service since 2016." []
is_a: DBO:0000010 ! Foundation Stock Service

[Term]
id: DBO:0000063
name: Berger Briard
def: "1928;The Briard was officially recognized by the AKC." []
is_a: DBO:0000008 ! Herding Group

[Term]
id: DBO:0000064
name: Brittany
def: "1934;The Brittany was officially recognized by the AKC." []
is_a: DBO:0000002 ! Sporting Group

[Term]
id: DBO:0000065
name: Danish Broholmer
def: "As a type, this breed has been known since the Middle Ages, when it was used for stag-hunting. Later, it was used mainly as a guard dog for large farms and manors. At the end of the 18th century, these dogs were pure-bred and increased in number thanks to the Count Sehested of Broholm, from whom the breed has inherited its name. After World War II, the breed became almost extinct, but around 1975, a group of committed people, later organized as The Society for Reconstruction of the Broholmer Breed, supported by the Danish Kennel Club, began the work of reviving the breed.;In 1998, the Broholmer breed was officially acknowledged by the international breed registry, FCI. Up until 2009, the Broholmer had only been found in Denmark and a few other European countries. Then in June of that year, the very first Danish Masitff named Honor was imported into the United States by Joe and Kathy Kimmeth of the Broholmer Club of the USA. Since then, interest in the breed has surged.2013;The Broholmer was recorded in the Foundation Stock Service." []
is_a: DBO:0000010 ! Foundation Stock Service

[Term]
id: DBO:0000066
name: English Bull Terrier
def: "1885;The Bull Terrier was officially recognized by the AKC" []
is_a: DBO:0000005 ! Terrier Group

[Term]
id: DBO:0000067
name: English Bulldog
def: "1886;The Bulldog was officially recognized by the AKC" []
is_a: DBO:0000007 ! Non-Sporting Group

[Term]
id: DBO:0000068
name: Bullmastiff
def: "The Bullmastiff's nickname is "The Gamekeeper's Night Dog," and this pretty much sums up the breed's early history.;During the mid- to late 19th century, the vast country estates and game preserves of the English aristocracy were the irresistible targets of poachers. "Penalties were severe," wrote a breed historian, "yet poaching seemed impossible to eradicate by mere laws." Because a poacher might face the death penalty if captured, they had nothing to lose when encountering an estate's gamekeeper. They might choose to shoot it out with the gamekeeper when cornered, rather than face the gallows.;Gamekeepers responded by breeding dogs big, swift, and brave enough to pursue and pin a man prowling the grounds in the dead of night. Eventually they hit upon just the right combination of breeding stock by crossing Mastiffs to Bulldogs at a ratio of 60 percent Mastiff and 40 percent Bulldog. The new breed was smart enough to work on command, tractable enough to hold but not maul a poacher, a big enough to scare the bejesus out of any intruder.;Inevitably, rivalries developed among Britain's gamekeepers over who had the best-quality Bullmastiffs. Competitions and exhibitions of the best specimens were staged, and from there it was but a short leap for the Bullmastiff into the show ring. Dog shows in England were gaining in popularity just as Bullmastiff fanciers were standardizing their breed. By 1924, the Bullmastiff as we now know it was ready to join the ranks of the Kennel Club (England). The AKC granted the breed full recognition in 1933.1934;The Bullmastiff was officially recognized by the AKC" []
is_a: DBO:0000004 ! Working Group

[Term]
id: DBO:0000069
name: Cairn Terrier
def: "1913;The Cairn Terrier was officially recognized by the AKC" []
is_a: DBO:0000005 ! Terrier Group

[Term]
id: DBO:0000070
name: Canaan Dog
def: "1997;The Canaan Dog was officially recognized by the AKC" []
is_a: DBO:0000008 ! Herding Group

[Term]
id: DBO:0000071
name: Cane Corso(Italian Mastiff)
def: "2010;The Cane Corso was officially recognized by the AKC." []
is_a: DBO:0000004 ! Working Group

[Term]
id: DBO:0000072
name: Cardigan Welsh Corgi
def: "1935;The Cardigan Welsh Corgi was officially recognized by the AKC" []
is_a: DBO:0000008 ! Herding Group

[Term]
id: DBO:0000073
name: Carolina Dog
def: "When primitive humans migrated across the Bering land bridge from Asia into North America, they brought with them a primitive form of dog that were domesticated from Asian wolves thousands of years earlier. Skeletal and mummified remains of these dogs have been discovered alongside other artifacts belonging to the Southwest Indians and from there, they moved further into Central and South America and over to the eastern United States. Archaeologists discovered similar canine remains in ceremonial burials in the southeastern forests, denoting their companionship with Native Americans long before Europeans arrived.;Recent studies of free-ranging dogs of the Southeast and Southwest suggest a close ancestry and possible descent from these primitive companions based on appearance, behavior, and ecology. These free-ranging dogs were named Carolina Dogs by Dr. I. Lehr Brisbin, who initially made contact with the breed in the Southeast.2017;The Carolina Dog has been recorded in the Foundation Stock Service since July 2017." []
is_a: DBO:0000010 ! Foundation Stock Service

[Term]
id: DBO:0000074
name: Catahoula Leopard Dog
def: "In 1539, when Spanish explorer Hernando de Soto landed in Florida and began his expedition through the Southeastern United States, his scribes noted there was only one species of domestic animal in North America: the Native American's dog, who looked like a wolf but barked like a dog. These native dogs were crossed with the "bloodhounds, mastiffs, and greyhounds" brought by the Spanish explorers. In Northern Louisiana, the Native Americans called these new dogs "Wolf Dogs." Once the French arrived with their hounds, they were crossbred again, resulting in today's Catahoula Leopard Dog.;How the Catahoula obtained his working instincts is another story: The early settlers of Central Louisiana, specifically the Catahoula Lake area, used these crossbred dogs to pen and catch the wild hogs and cows that were rampant in the area, and this practice turned into a planned method of managing the wild herds. The Catahoula developed a unique way of working the stock that sets them apart from other herding and working breeds; they create a "canine fence" around the herd, and within this "fence," the wild herd is directed by the dog's master. This natural working instinct is of the utmost importance to Catahoula Leopard Dog breeders. Regardless of appearance, he must have these working instincts to be a pure Catahoula.1996;The Catahoula Leopard Dog was recorded in the Foundation Stock Service." []
is_a: DBO:0000010 ! Foundation Stock Service

[Term]
id: DBO:0000075
name: Caucasian Shepherd Dog
def: "The Kavkaz (Caucasus) mountain range of Eastern Europe – so many nations with different cultures calling it their home through the centuries. The territories of Armenia, Georgia, Azerbaijan, Kabardino-Balkaria, Daghestan, Osettia, Turkey, Chechnia, Ingushetia and Iran, the Caucasus mountains are also home to the Caucasian Ovcharka or Caucasian Shepherd Dog. Although its first official Western Show-Ring appearance was in the 1930s in Germany, the Caucasian Shepherd has existed since ancient times and was introduced to the bloodlines of many of today's world breeds throughout history. Many researches show the Caucasian dog as being a close relative of the sheepdogs of the Balkans and mastiffs of Asia.;Historically, Caucasian Shepherd Dogs were used for the guarding and safe-keeping of herds, flocks and dwellings from predators. The first mention of a large molossoid dog used by the army of Armenian Tsar Tigran the II dates from the first century BC. Selection work with the breed started in the USSR in the 1920s. Obligatory qualities such as physical power, self-confidence, fearlessness, sharply developed hearing, good sight, and a dense and waterproof coat have been cultivated in the process of selection. All these qualities, as well as endurance, allows people to use Caucasian Shepherd Dogs in all kinds of climatic conditions, including the most severe ones.1996;The Caucasian Shepherd Dog was recorded in the Foundation Stock Service." []
is_a: DBO:0000010 ! Foundation Stock Service

[Term]
id: DBO:0000076
name: Cavalier King Charles Spaniel
def: "1995;The Cavalier King Charles Spaniel was officially recognized by the AKC" []
is_a: DBO:0000006 ! Companion and Toy Group

[Term]
id: DBO:0000077
name: Central Asian Shepherd Dog
def: "The Central Asian Shepherd Dogs are said to be the oldest known group of dogs in existence today, dating back over 5,000 years according to artifacts found in native lands. Unlike most breeds today, they are not man-made or created by any specific person or country. They were created by the climate and culture of an uncivilized time long forgotten. You will find in CASDs different breed types depending on the terrain, from the mountains of Mongolia to the deserts of the Kara Kum. Their history is merged with the civilization of man and their timeline can be found by tracing the history of the ancient Silk Road. To understand their past, you must understand a time when surviving one day against extreme climates, predators now extinct, and invading tribes was a goal not easily achieved. Today, you will find nomadic tribes using this pedigree group of dogs to guard what they hold sacred: their family and their ancient form of transportation, be it camels or horses. Recent History has these dogs improperly classified as traditional Livestock Guardian dogs. They are territorial guardians bred to guard people and their possessions. They seek out human attention, thus bonding with their humans first and the flock second, and they guard whatever is placed in their perceived territory.Present history has a division between breed types and creations of new ones. The former USSR is credited with standardizing the breed in the 1920s, however, the recent creation of a new Russian standard years after USSR rule ended in their native lands has resulted in a modern version of the breed in Russia called the Central Asian Ovcharka. This new version has separated them from other aboriginal types found in the native countries of Central Asia. We are just now seeing the difference of size, color and temperament between the native species and the modern, Russian-cultivated dogs." []
is_a: DBO:0000010 ! Foundation Stock Service

[Term]
id: DBO:0000078
name: Cesky Terrier
def: "2011;The Cesky Terrier was officially recognized by the AKC." []
is_a: DBO:0000005 ! Terrier Group

[Term]
id: DBO:0000079
name: Chesapeake Bay Retriever
def: "1878;The Chesapeake Bay Retriever was officially recognized by the AKC." []
is_a: DBO:0000002 ! Sporting Group

[Term]
id: DBO:0000080
name: Chihuahua
def: "1904;The Chihuahua was officially recognized by the AKC." []
is_a: DBO:0000006 ! Companion and Toy Group
synonym: "Chi" EXACT[]

[Term]
id: DBO:0000081
name: Chinese Shar-Pei
def: "1992;The Chinese Shar-Pei was officially recognized by the AKC." []
is_a: DBO:0000007 ! Non-Sporting Group

[Term]
id: DBO:0000082
name: Chinook
def: "2010;The Chinook was officially recognized by the AKC.." []
is_a: DBO:0000004 ! Working Group

[Term]
id: DBO:0000083
name: Chow Chow
def: "1903;The Chow Chow was officially recognized by the AKC" []
is_a: DBO:0000007 ! Non-Sporting Group

[Term]
id: DBO:0000084
name: Cirneco dell'Etna
def: "It is thought that ancient Egyptians perfected "sighthounds" or "coursing hounds," the canine clan of explosively fast hunters struck from the Greyhound template. In antiquity, offshoots of the "Egyptian Hound" were developed and bartered around the Middle East and Mediterranean basin.;A clue to the Cirneco's origin is in its name: Cirneco is derived from a Greek word meaning "dog of Cyrene (Libya)." It is likely that the breed has existed in Sicily since its ancestors arrived on its craggy shores some 3,000 years ago in the holds of ships piloted by those master traders of the ancient world, the Phoenicians. As far back as 500 b.c., dogs resembling Cirnechi appeared on Sicilian coins.;For thousands of years Cirnechi (sometimes called Sicilian Greyhounds) have been chasing rabbit, hare, and game birds across the rocky slopes of Mount Etna, Europe's largest active volcano. Don't be fooled by the breed's delicate appearance; the Cirneco dell'Etna is a tough and durable worker, able to go without food or water for hours on the hunt in the hot climate and rugged terrain of its homeland.;By the early 1930s, the Cirneco was on the verge of oblivion. Dr. Maurizio Migneco, a veterinarian, wrote a passionate article about the breed's imminent demise. It caught the attention of a Sicilian aristocrat, Baroness Agata Paternó Castello, who spent the next 26 years reviving the breed in Sicily.;The Cirneco was recognized by Italy's national kennel club in 1939, and the AKC recognized the breed in 2015.2015;The Cirneco dell'Etna was officially recognized by the AKC." []
is_a: DBO:0000003 ! Hound Group
synonym: "Cirneco" EXACT[]

[Term]
id: DBO:0000085
name: Clumber Spaniel
def: "1884;The Clumber Spaniel was officially recognized by the AKC" []
is_a: DBO:0000002 ! Sporting Group

[Term]
id: DBO:0000086
name: Coton de Tulear
def: "2014;The Coton de Tulear was officially recognized by the AKC." []
is_a: DBO:0000007 ! Non-Sporting Group
synonym: "Coton" EXACT[]
synonym: "Cotie" EXACT[]

[Term]
id: DBO:0000087
name: Curly-Coated Retriever
def: "1924;The Curly-Coated Retriever was officially recognized by the AKC" []
is_a: DBO:0000002 ! Sporting Group
synonym: "Curly" EXACT[]
synonym: "CCR" EXACT[]

[Term]
id: DBO:0000088
name: Czechoslovakian Vlcak(Czechoslovakian Wolfdog)
def: "In 1955, a biological experiment took place in the CSSR of that time, namely, the crossing of a German Shepherd Dog with a Carpathian Wolf. The experiment established that the progeny of the mating of a male dog to a female wolf as well as that of male wolf to female dog, could be reared. The overwhelming majority of the products of these matings possessed the genetic requirements for continuation of breeding. In 1965, after ending the experiment, a plan for the breeding of this new breed was worked out. This was to combine the usable qualities of the wolf with the favorable qualities of the dog. In 1982, the Czechoslovakian Wolfdog, through the general committee of the breeder's associations of the CSSR of that time, was recognized as a national breed.2001;The Czechoslovakian Vlcak was recorded in the Foundation Stock Service." []
is_a: DBO:0000010 ! Foundation Stock Service

[Term]
id: DBO:0000089
name: Dachshund
def: "1885;The Dachshund was officially recognized by the AKC." []
is_a: DBO:0000003 ! Hound Group
synonym: "Teckel (BNL/FR/GER)" EXACT[]
synonym: "Dackel (GER)" EXACT[]
synonym: "Weenie Dog (US) (S" EXACT[]
synonym: "Am" EXACT[]
synonym: ")" EXACT[]
synonym: "Wiener Dog/Hotdog (US)" EXACT[]
synonym: "Sausage Dog (UK/US/AUS/ZA)" EXACT[]
synonym: "Salsichinha (BR)" EXACT[]
synonym: "Bassotto (I)" EXACT[]
synonym: "Sosis (TR)" EXACT[]
synonym: "Perro Salchicha (ES/MX)" EXACT[]
synonym: "Worshond (ZA)" EXACT[]
synonym: "Taksis (LV)" EXACT[]
synonym: "Jamnik (PL)" EXACT[]
synonym: "Badger Dog (literal translation)" EXACT[]
synonym: "Tax (SE)" EXACT[]

[Term]
id: DBO:0000090
name: Dalmatian
def: "1888;The Dalmatian was officially recognized by the AKC" []
is_a: DBO:0000007 ! Non-Sporting Group

[Term]
id: DBO:0000091
name: Dandie Dinmont Terrier
def: "1886;The Dandie Dinmont Terrier was officially recognized by the AKC" []
is_a: DBO:0000005 ! Terrier Group
synonym: "Dandie" EXACT[]
synonym: "Hindlee Terrier" EXACT[]

[Term]
id: DBO:0000092
name: Danish-Swedish Farmdog
def: "Until a few decades ago, the small farmer's dog, originally known as the Danish Pincher, was a natural part of the Danish rural life. The Danish-Swedish Farmdog's everyday functions were many, including mouser/ratter, livestock herder, hunting dog, watchdog and family companion. As lifestyles have changed, smaller family farms have become rarer and so too has the faithful working Farmdog. Efforts from the Danish and Swedish Kennel Clubs to bring back this breed culminated in 1987 with the first breed standard for the Danish-Swedish Farmdog. In 1998, a DSF was imported to the United States to establish the first official breeding program there. The FCI Standard for the breed was officially published March 26, 2009. The Danish-Swedish Farmdog was recorded in the American Kennel Club Foundation Stock Services in 2011, its first step to its goal of becoming fully recognized by the AKC." []
is_a: DBO:0000010 ! Foundation Stock Service

[Term]
id: DBO:0000093
name: Deutscher Wachtelhund
def: "In the 1880s, a group of German hunters decided to recreate the Stober, a versatile breed mentioned as far back in German history as 1719. The Stober was known to have the scent following ability similar to that of a bloodhound. The Germans obtained remnants of that breed found in Bavaria and bred them with other sporting spaniels that had a proven passion for hunting. They produced the Wachtelhund (pronounced 'Valk-tel-hund') and the breed was officially recognized in 1903. The German Wachtelhund club is called the Verein fur Deutsche Wachtelhund (VDW). In Germany, only gamekeepers and hunters own this breed, they are not sold to the non-hunting public.Several Wachtelhunds were brought to the United States in the late 1950s and early 1960s, but were only bred once or twice, producing a total of 17 dogs. None were registered in North America.In Canada, several individuals, guides and hunting outfitters have owned Wachtelhunds for the past twenty years or so and utilized them as flushers, retrievers and to track and hold wounded black bear at bay. In 1993 and 1994, Dave Pepe imported a pair of Wachtelhunds to the United States and bred them four times producing 38 pups.  Since then, several other dogs have been imported and numerous breedings have occurred. Today, there are  approximately 100 to 150 dogs in the US and Canada." []
is_a: DBO:0000010 ! Foundation Stock Service

[Term]
id: DBO:0000094
name: Doberman Pinscher
def: "1908;The Doberman Pinscher was officially recognized by the AKC." []
is_a: DBO:0000004 ! Working Group
synonym: "Dobie" EXACT[]
synonym: "Dobynm" EXACT[]

[Term]
id: DBO:0000095
name: Dogo Argentino
def: "1995;The Dogo Argentino was first recorded in the Foundation Stock Service." []
is_a: DBO:0000009 ! Miscellaneous
synonym: "Dogo" EXACT[]

[Term]
id: DBO:0000096
name: Dogue de Bordeaux(French Mastiff)
def: "2008;The Dogue de Bordeaux was officially recognized by the AKC" []
is_a: DBO:0000004 ! Working Group

[Term]
id: DBO:0000097
name: Drentsche Patrijshond
def: "The breed developed from pointing dogs originating in Spain (Spioenen) and arrived in The Netherlands via France in the 16th Century. In The Netherlands, these dogs were referred to as Partridge dogs. In the eastern parts of the country, principally in the Province of Drenthe, these Partridge dogs were bred among themselves and not mixed with foreign breeds, as occurred elsewhere. Throughout its history, the breed stood on three equally important pillars: versatile hunting dog, farm yard dog, and playmate to the children. It is fundamental to the Drent breed that he hunts all upland game and water fowl, announces visitors to the home or farm (without showing aggression or fear), and is an excellent family companion, with emphasis on being an excellent companion to children. These three pillars continue to serve as guiding parameters as to what defines a Drent today. The breed was recognized by the Dutch Kennel Club on May 15, 1943." []
is_a: DBO:0000010 ! Foundation Stock Service

[Term]
id: DBO:0000098
name: Drever
def: "The small-sized German hound, the Westphalian Dachsbracke, was imported to Sweden in 1910. The first dogs were registered in 1913, but little else is known about the breed before 1930. It was from then on that it gained a reputation as a very good tracker of deer. Deer had been sparse until then, but as they grew stronger in numbers and spread further north, hunters got to hear about the advantages of the short-legged deer tracking hound. In 1947, the larger Swedish variety of the Bracke was given the name Drever. In 1953, the Drever was recognized as a Swedish breed. The Drever is considered the first choice for deer hunting but it is also a very reliable hound for hunting both hare and fox. In all essence, the Drever should be built as a track hound. It should have the ability to work efficiently in the Swedish terrain and climate. The breed is strictly kept as a hunting dog and hardly ever heard of as just a companion dog." []
is_a: DBO:0000010 ! Foundation Stock Service

[Term]
id: DBO:0000099
name: Dutch Shepherd Dog
def: "The Dutch Shepherd is a natural land-breed originating in The Netherlands. Long ago, shepherds and farmers needed a versatile dog, a "Jack-of-all-trades", well-adapted to the harsh and sparse existence of the time. In addition to its role as a shepherd's dog, at the farm they kept the hens away from the kitchen garden, herded the cows together for milking, and pulled carts laden with milk or produce to market. They also watched the children and alerted the farmer if strangers entered the farmyard.The first breed standard dates from June 12, 1898. In this original standard, any coat color was permitted, but by 1914, it was decided the Dutch Shepherd should only be brindle so as to distinguish it from other similar breeds of the time, the German Shepherd and Belgian Shepherd. Around 1900, sheep flocks in The Netherlands, and the shepherd dogs which tended them, had been mostly replaced by industrialization, and the reclamation of land for other purposes. The versatile skills of the Dutch Shepherd made it suitable for new careers such as a police dog, search and rescue, and guide dog for the blind. The breed has retained its original herding ability, and is still used for this purpose." []
is_a: DBO:0000009 ! Miscellaneous

[Term]
id: DBO:0000100
name: English Cocker Spaniel
def: "1945;The English Cocker Spaniel was officially recognized by the AKC" []
is_a: DBO:0000002 ! Sporting Group
synonym: "Cocker" EXACT[]
synonym: "Cocker Spanie" EXACT[]

[Term]
id: DBO:0000101
name: English Foxhound
def: "1909;The English Foxhound was officially recognized by the AKC" []
is_a: DBO:0000003 ! Hound Group

[Term]
id: DBO:0000102
name: English Setter
def: "1884;The English Setter was officially recognized by the AKC." []
is_a: DBO:0000002 ! Sporting Group

[Term]
id: DBO:0000103
name: English Springer Spaniel
def: "1910;The English Springer Spaniel was officially recognized by the AKC" []
is_a: DBO:0000002 ! Sporting Group

[Term]
id: DBO:0000104
name: Entlebucher Mountain Dog
def: "2011;The Entlebucher Mountain Dog was officially recognized by the AKC in 2011." []
is_a: DBO:0000008 ! Herding Group

[Term]
id: DBO:0000105
name: Estrela Mountain Dog
def: "The earliest of the Estrela ancestors were herd-guarding dogs in the Serra da Estrela, in what is now Portugal. Since there are no written records, it is uncertain whether the ancestors which contributed to this breed were brought by the Romans when they colonized the Iberian Peninsula, or later by the invading Visigoths. Regardless, there is no disagreement that the Estrela is one of the oldest breeds in Portugal.Those early guardian dogs were not the distinct breed we know today, rather, the Estrela developed over a period of hundreds of years. Shepherds would have chosen to breed the dogs that had the characteristics necessary to survive in their mountain environment and to do their job: large-sized, strong, having endurance, agile, deep-chested, able to tolerate a marginal diet, a proper set of the legs, a powerful mouth, a tuft of hair around its neck, an easy, jog-like gait, a warm coat, and a watchful, mistrustful, yet loyal temperament.Life changed little for the people and dogs of the region, even into the 20th century. The isolation of the region meant the breed was relatively unknown outside it until the early 1900s, and even then, they were mostly ignored in early dog shows. The Portuguese admired foreign breeds much more than their own and shepherds often castrated their dogs to prevent them from leaving their flocks to mate. These factors had a negative effect on the Estrela, so from 1908 to 1919, special shows called concursos were held to promote and preserve the Estrela Mountain Dog breed in the region. Special livestock guardian working trials were included in these shows. The trial consisted of an owner bringing his dog into a large field with many flocks of sheep. The dog was observed by judges for its reactions coming into the field and as the shepherd was ordered to move the flock, which inevitably produced stragglers. The dog was expected to move from his spot of guarding to bring the stragglers back, and then assume a leadership position at the head of the flock. During this period, there was some attempt at a registry, of which there is no surviving record.The first tentative, recorded breed standard was published in 1922. This standard just reflected the functional features naturally found in the best dogs of the time, although it did mention the dew claws as reflecting a "perfect" dog. The hooked tail and the turned-back ears, which later became part of the official standard, were not mentioned. The first official breed standard was written in 1933. This standard attempted to differentiate the Estrela as a distinct breed. This led to the hooked tail and double dew claws becoming a requirement. All colors were allowed.Prior to World War II, the Estrela's breeders were still primarily the shepherds and farmers of the region. Since they were mostly illiterate, they did not make any attempt to follow the official breed standard, if they even knew one existed. But by the early 1950s, interest in the breed returned, and the annual concursos were reinstated. Again, the intent was to stimulate interest among the Serra residents and to encourage them to adhere to the official standard. During this period, the long-haired variety was most popular at shows, but show dogs represented only a small portion of the Estrela population in Portugal, and still do. Many of the working dogs were, and are, short-haired.To this day, the Estrela Mountain Dog remains true to its guardian heritage. It is still a working dog, guarding flocks in its native Portugal and elsewhere. The Portuguese also use it as a police dog. In the home, it is an ideal family pet because of its alertness, loyalty, intelligence, and its instinct to nurture young, all features it needed in its earliest days." []
is_a: DBO:0000010 ! Foundation Stock Service
synonym: "Estrela" EXACT[]

[Term]
id: DBO:0000106
name: Eurasier
def: "Julius Wipfel, who resided in Germany, searched to find a successor to his black, Spitz-type dog which was very intelligent and independent. He wished for a dog that would show the adaptability and social behavior of dog's ancestor, the wolf, and a dog that would be a wonderful family pet. Wipfel and other dog enthusiasts started the long journey of trying to develop a family-oriented breed. Strict breeding plans and guided breeding resulted in the first litter of "Wolf-Chow" puppies through the cross-breeding of a Chow Chow and a Wolfspitz. Then, in 1972, a Samoyed was crossed in to introduce its friendly nature and their offspring was named "Eurasier" to reflect the breed's European and Asian heritage. In 1973, the German Kennel Club and the Federation Cynologique International acknowledged the breed. The standard was re-written in 1994." []
is_a: DBO:0000010 ! Foundation Stock Service

[Term]
id: DBO:0000107
name: Field Spaniel
def: "1894;The Field Spaniel was officially recognized by the AKC" []
is_a: DBO:0000002 ! Sporting Group
synonym: "Field" EXACT[]

[Term]
id: DBO:0000108
name: Finnish Lapphund
def: "2011;The Finnish Lapphund was officially recognized by the AKC in 2011." []
is_a: DBO:0000008 ! Herding Group

[Term]
id: DBO:0000109
name: Finnish Spitz
def: "1988;The Finnish Spitz was officially recognized by the AKC" []
is_a: DBO:0000007 ! Non-Sporting Group

[Term]
id: DBO:0000110
name: Flat-Coated Retriever
def: "1909;The Flat-Coated Retriever was officially recognized by the AKC" []
is_a: DBO:0000002 ! Sporting Group
synonym: "Flatcoat" EXACT[]
synonym: "Flattie" EXACT[]
synonym: "Flatte (Sweden)" EXACT[]
synonym: "flatt (Sweden)" EXACT[]

[Term]
id: DBO:0000111
name: French Bulldog
def: "1898;The French Bulldog was officially recognized by the AKC" []
is_a: DBO:0000007 ! Non-Sporting Group
synonym: "Frenchie" EXACT[]

[Term]
id: DBO:0000112
name: French Spaniel
def: "2008;The French Spaniel was Officially standardized by FCI." []
is_a: DBO:0000010 ! Foundation Stock Service

[Term]
id: DBO:0000113
name: German Long-Haired Pointer
def: "2010;The German Longhaired Pointer was recorded in the Foundation Stock Service" []
is_a: DBO:0000010 ! Foundation Stock Service
synonym: "GLP" EXACT[]

[Term]
id: DBO:0000114
name: German Pinscher
def: "2003;The German Pinscher was officially recognized by the AKC" []
is_a: DBO:0000004 ! Working Group

[Term]
id: DBO:0000115
name: German Shepherd Dog
def: "1908;The German Shepherd Dog was officially recognized by the AKC." []
is_a: DBO:0000008 ! Herding Group
synonym: "Alsatian" EXACT[]
synonym: "Deutscher Schaferhund" EXACT[]
synonym: "DSH" EXACT[]
synonym: "GSD" EXACT[]
synonym: "Shepherd" EXACT[]
synonym: "Schaferhund" EXACT[]

[Term]
id: DBO:0000116
name: German Short-Haired  Pointer
def: "1930;The German Shorthaired Pointer was officially recognized by the AKC." []
is_a: DBO:0000002 ! Sporting Group
synonym: "GSP" EXACT[]
synonym: "DK" EXACT[]

[Term]
id: DBO:0000117
name: German Spitz
def: "German Spitz, like all spitz, have many physical features found in oldest stone age fossil dogs in Central Europe, leading experts at the time[when?] to believe that the spitz is the oldest dog type. However, modern genetic evidence places them in a much more recent lineage, dating the Wolfsspitz-type to the 1800s.[2] The German Spitz was later brought to America, and was renamed American Eskimo Dog due to the widespread anti-German sentiment during World War I, although other breeds ("White Keeshonds" and Pomeranians, along with Japanese Spitz) were also used in the formation of the breed. The American Kennel club recognizes the breeds as separate." []
is_a: DBO:0000010 ! Foundation Stock Service

[Term]
id: DBO:0000118
name: German Wire-Haired Pointer
def: "1959;The German Wirehaired Pointer was officially recognized by the AKC" []
is_a: DBO:0000002 ! Sporting Group

[Term]
id: DBO:0000119
name: Giant Schnauzer
def: "1930;The Giant Schnauzer was officially recognized by the AKC" []
is_a: DBO:0000004 ! Working Group

[Term]
id: DBO:0000120
name: Irish Glen of Imaal Terrier
def: "2004;The Glen of Imaal Terrier was officially recognized by the AKC." []
is_a: DBO:0000005 ! Terrier Group
synonym: "Glen" EXACT[]
synonym: "Glennie" EXACT[]

[Term]
id: DBO:0000121
name: Golden Retriever
def: "1925;The Golden Retriever was officially recognized by the AKC." []
is_a: DBO:0000002 ! Sporting Group

[Term]
id: DBO:0000122
name: Gordon Setter
def: "1884;The Gordon Setter was officially recognized by the AKC." []
is_a: DBO:0000002 ! Sporting Group

[Term]
id: DBO:0000123
name: Grand Basset Griffon Vendeen
def: "2004;The Grand Basset Griffon Vendeen was first recorded in the Foundation Stock Service." []
is_a: DBO:0000009 ! Miscellaneous
synonym: "GBGV" EXACT[]

[Term]
id: DBO:0000124
name: Great Dane
def: "1887;The Great Dane was officially recognized by the AKC." []
is_a: DBO:0000004 ! Working Group
synonym: "Apollo of Dogs" EXACT[]
synonym: "Gentle Giant" EXACT[]

[Term]
id: DBO:0000125
name: Great Pyrenees
def: "1933;The Great Pyrenees was first recognized by the AKC" []
is_a: DBO:0000004 ! Working Group
synonym: "Pyr" EXACT[]
synonym: "GP" EXACT[]
synonym: "PMD" EXACT[]

[Term]
id: DBO:0000126
name: Greater Swiss Mountain Dog
def: "1995;The Greater Swiss Mountain Dog was officially recognized by the AKC." []
is_a: DBO:0000004 ! Working Group

[Term]
id: DBO:0000127
name: Greyhound
def: "1885;The Greyhound was officially recognized by the AKC" []
is_a: DBO:0000003 ! Hound Group

[Term]
id: DBO:0000128
name: Hamiltonstovare(Hamilton Hound)
def: "The Hamiltonstövare is a native breed of Sweden, where it was founded in the late 1800s by the founder of the Swedish Kennel Club, Count Adolf Patrick Hamilton. Count Hamilton sought a sturdy hound that could hunt both hare and fox in difficult terrain and harsh climate. The breed also needed to be flexible to negotiate the terrain of Sweden, which is mainly forested and mountainous. He used English Foxhounds, Harriers, and three now extinct breeds from Germany: the Curlandish Hound, Holsteiner Hound, and Heiderbracke. The hounds credited with founding the Hamiltonstövare breed were known as Pang and Stella, owned by Hamilton. The Hamiltonstövare was first shown in Sweden in 1921. They were known as the Swedish Hound then, but the name has since changed to honor the breed founder.Unlike its English relatives, the breed was not developed to hunt in a pack, but instead used as a solitary hunter or as a pair. To this day, the Hamiltonstövare still performs its original purpose in Sweden, where the breed has a popular following. Most recently, Hamiltons have started to make an impact around the world outside of Sweden, though they are still very rare in the United States." []
is_a: DBO:0000010 ! Foundation Stock Service
synonym: "Hamilton" EXACT[]

[Term]
id: DBO:0000129
name: Harrier
def: "1885;The Harrier was officially recognized by the AKC." []
is_a: DBO:0000003 ! Hound Group

[Term]
id: DBO:0000130
name: Havanese
def: "1996;The Havanese was officially recognized by the AKC" []
is_a: DBO:0000006 ! Companion and Toy Group

[Term]
id: DBO:0000131
name: Ainu-ken(Hokkaido)
def: "The Hokkaido is one of the oldest of the six native Japanese spitz breeds. They are said to have originated from medium-sized Japanese dogs that accompanied the Ainu people from Honshu (the main island of Japan) to Hokkaido during the Kamakura era in the 1140s, when exchanges were developing between Hokkaido and the Tohoku District. Over time, the Ainu people and their dogs adapted to survive the severely cold winter climate and rugged landscape. The dogs were revered by the Ainu people for their devout loyalty, bravery, and large game hunting ability. The Ainu were bear and deer hunters by culture, and their livelihood depended on their renowned bear dogs.The Hokkaido was classified as a Living Natural Monument by the government of Japan in 1937. There are two main breed registries, the Hokkaido Ken Hozonkai (Hokkaido Dog Preservation Society) and the Hokkaido Ken Kyokai (Hokkaido Dog Association). Almost no Hokkaido are registered outside of these two clubs." []
is_a: DBO:0000010 ! Foundation Stock Service
synonym: "Ainu dog" EXACT[]

[Term]
id: DBO:0000132
name: Hovawart
def: "The Hovawart is a very old German working dog breed. The name's origin stems from Middle High German (an old form of German); Hova = Hof (= yard, farm) and wart = Wächter (= watchman). Since 1922 the breeding of this breed, by using dogs similar in type still found on farms, has been restored. Apart from this, in the early years of breeding, crosses with German Shepherd Dogs, Newfoundlands, Leonbergers and other breeds were admitted. Due to the strict measurements taken in selecting the breeding stock, the original working type was attained again. In 1937, Fédération Cynologique Internationale (FCI) officially recognized the Hovawart.;The circumstances of World War II threatened the breed again. It was difficult to keep and sustain dogs. Various groups of breeders tried to revive the breed with the reduced number of dogs that remained after the War. In 1948, the Rassezuchtverein für Hovawart-Hunde e.V. (RZV) was founded from some of these groups in the Federal Republic of Germany and became a member of the Verband für das deutsche Hundewesen (VDH), the German Kennel Club.2010;The Hovawart was recorded in the Foundation Stock Service" []
is_a: DBO:0000010 ! Foundation Stock Service
synonym: "Hovie" EXACT[]

[Term]
id: DBO:0000133
name: Ibizan Hound
def: "1978;The Ibizan Hound was officially recognized by the AKC." []
is_a: DBO:0000003 ! Hound Group

[Term]
id: DBO:0000134
name: Icelandic Shepherd Dog
def: "2010;The Icelandic Sheepdog was officially recognized by the AKC." []
is_a: DBO:0000008 ! Herding Group

[Term]
id: DBO:0000135
name: Irish Red and White Setter
def: "2009;The Irish Red and White Setter was first recognized by the AKC." []
is_a: DBO:0000002 ! Sporting Group
synonym: "IRWS" EXACT[]
synonym: "Irish R&W Setter" EXACT[]

[Term]
id: DBO:0000136
name: Irish Setter
def: "1878;The Irish Setter was officially recognized by the AKC." []
is_a: DBO:0000002 ! Sporting Group

[Term]
id: DBO:0000137
name: Irish Terrier
def: "1885;The Irish Terrier was officially recognized by the AKC." []
is_a: DBO:0000005 ! Terrier Group

[Term]
id: DBO:0000138
name: Irish Water Spaniel
def: "1884;The Irish Water Spaniel was officially recognized by the AKC." []
is_a: DBO:0000002 ! Sporting Group

[Term]
id: DBO:0000139
name: Irish Wolfhound
def: "1897;The Irish Wolfhound was officially recognized by the AKC." []
is_a: DBO:0000003 ! Hound Group

[Term]
id: DBO:0000140
name: Italian Greyhound
def: "1886;The Italian Greyhound was officially recognized by the AKC." []
is_a: DBO:0000006 ! Companion and Toy Group

[Term]
id: DBO:0000141
name: German Jagdterrier
def: "After World War I, a small group of active hunters separated from the much larger Fox-Terrier Club. It was this group's aim to create a breed solely based on hunting performance. The experienced hunters and cynologists Rudolf FrieÃŸ, Walter Zangenberg and Carl-Erich GruÌˆnewald decided to select a black and tan hunting dog that was particularly suited to hunting underground. A coincidence arose in support of their efforts: a zoo director, Lutz Heck presented Walter Zangenberg with four black and tan terriers which were said to come from purebred Fox-Terrier lines. These dogs became the foundation stock of the Jagdterrier.At this time, Dr Herbert Lackner joined the founders. After many years of intensive breeding efforts and through skillful crossings with the Old English Wirehaired Terrier as well as with the Welsh Terrier, they succeeded in fixing the appearance of their breed. At the same time, they put great emphasis on breeding a multi-talented, easily-trainable, hard, tongue-giving and water-happy dog with an explicit hunting instinct. The German Hunting Terrier Club (Deutscher Jagdterrier-Club e.V.) was founded in 1926. As ever, the breeders continued to value most carefully their breed for its usefulness as a hunting dog, its steadiness of character, its courage and drive." []
is_a: DBO:0000010 ! Foundation Stock Service

[Term]
id: DBO:0000142
name: Japanese Chin(Japanese Spaniel)
def: "1888;The Japanese Chin was officially recognized by the AKC." []
is_a: DBO:0000006 ! Companion and Toy Group
synonym: "Chin" EXACT[]

[Term]
id: DBO:0000143
name: Korean Jindo
def: "2008;The Jindo was recorded in the Foundation Stock Service" []
is_a: DBO:0000010 ! Foundation Stock Service

[Term]
id: DBO:0000144
name: Tora Inu(Kai ken)
def: "1997;The Kai Ken has been recorded in the Foundation Stock Service" []
is_a: DBO:0000010 ! Foundation Stock Service
synonym: "Tora Dog" EXACT[]

[Term]
id: DBO:0000145
name: Karelian Bear Dog
def: "The Karelian Bear Dog is a Finnish breed that originated in northwestern Europe and was originally the dog of Russian and Finnish peasants, used for hunting and as a watch dog. Only the toughest survived fightings and the harsh conditions while hunting. Early dogs had red, red-gray and black and white coats. The Komi dog, also called the dog of Zyrians, is considered to be the origin of the breed, however, the basic stock dogs originated from the Lagoda's Karelia, Olonets and Russian Karelia, where they were used for all different types of game hunting. The breeding was started in 1936 with the goal to create a sturdy dog which barks at big game. In further breeding, the progeny was selected to the Karelian Bear Dog type and only black and white dogs were preferred for breeding. It was then agreed that the name of the breed was to be the Karelian Bear Dog. The first standard was established in 1945. The first Karelian Bear Dogs were registered in the Finnish Kennel Club in 1946.;Today, the breed is one of the top 10 most common breeds in Finland. The Karelian Bear Dog is primarily a hunting breed, but can be trained for and compete in obedience trials, search and rescue trials, and sled dog trials in its native country.2005;The first petition to add the Karelian Bear Dog to the Foundation Stock Service program" []
is_a: DBO:0000010 ! Foundation Stock Service

[Term]
id: DBO:0000146
name: Keeshond
def: "1930;The Keeshond was officially recognized by the AKC." []
is_a: DBO:0000007 ! Non-Sporting Group

[Term]
id: DBO:0000147
name: Irish Blue Terrier
def: "1922;The Kerry Blue Terrier was officially recognized by the AKC." []
is_a: DBO:0000005 ! Terrier Group
synonym: "Kerry" EXACT[]

[Term]
id: DBO:0000148
name: Kishu Inu(Kishu Ken)
def: "The Japanese dog breeds are ancient and developed from a common source. In Japan, spitz-type hunting dogs (canis familiaris palustris) lived over 3000 years ago. The Kishu Ken (ken meaning "dog" in Japanese) developed from tough, medium-sized dogs that roamed the mountains of Japan many centuries ago. They were the matagi's dogs, used to hunt boar and deer. The region in Japan called Wakayama is best known for the breeding and development of the Kishu. In early years, Kishus came in different colors, but the white-coated Kishus showed superior qualities and therefore were used more often for breeding. The hunters preferred the white color because of easy visibility. Working dogs were bred for efficiency and usefulness. Prior to 1934, there were Kishus in white, red, brindle and some that were spotted. But the solid colors became the only accepted colors and the spotted-coat Kishus had disappeared by 1945. Today, the white coat is the preferred color and virtually the only color seen in show Kishus. In 1934, the Kishu was designated a "Memorial of Nature" in its native country. The Japanese people are proud of their dogs and bestow honors and praise on them. This pride and commitment to their national treasures, and the Kishu is one of them, is the reason the Kishus are rarely exported." []
is_a: DBO:0000010 ! Foundation Stock Service

[Term]
id: DBO:0000149
name: Hungarian Komondor
def: "1937;The Komondor was officially recognized by the AKC." []
is_a: DBO:0000004 ! Working Group

[Term]
id: DBO:0000150
name: Kromfohrlander
def: "Many troops in World War II had a mascot animal for comfort and as a reminder of home. This was often a stray dog or cat. "Original Peter" was a scruffy terrier mix that US Army troops found in northern France and he became their mascot, but the troops lost him when they crossed into Germany at war's end. He was found by a local attorney's wife, Ilse Schleifenbaum, and after an accidental mating with a Fox Terrier named Fifi that produced uniform puppies that all looked like their father, she decided to create the breed and name it after the beautiful, local 'crooked furrows' (krumme furche) of farmland. After 10 years of careful development, the Federation Cynologique Internationale accepted the breed in August, 1955. The Kromfohrlander is still quite rare and is primarily found in Germany and other European nations. They are so rare, even in Europe, that individuals to export have been very difficult to obtain, as most breeders there prefer to keep the healthy blood-stock in close proximity." []
is_a: DBO:0000010 ! Foundation Stock Service
synonym: "Lander" EXACT[]
synonym: "Kromi" EXACT[]

[Term]
id: DBO:0000151
name: Hungarian Kuvasz
def: "1931;The Kuvasz was officially recognized by the AKC." []
is_a: DBO:0000004 ! Working Group

[Term]
id: DBO:0000152
name: Labrador Retriever
def: "1917;The Labrador Retriever was officially recognized by the AKC." []
is_a: DBO:0000002 ! Sporting Group
synonym: "Lab" EXACT[]

[Term]
id: DBO:0000153
name: Lagotto Romagnolo(Romagna Water Dog)
def: "2015;The Lagotto Romagnolo was officially recognized by the AKC" []
is_a: DBO:0000002 ! Sporting Group
synonym: "Lagotto" EXACT[]

[Term]
id: DBO:0000154
name: Lakeland Terrier
def: "1934;The Lakeland Terrier was officially recognized by the AKC." []
is_a: DBO:0000005 ! Terrier Group

[Term]
id: DBO:0000155
name: Lancashire Heeler
def: "The Lancashire Heeler's history extends back to the 17th century, but the exact origin of the breed is unknown. However, it is generally accepted that a type of Welsh Corgi was utilized to drive stock to market in northern Wales to the Lancashire market. What is known is a small black and tan dog known as the butchers' dog was common in the Ormskirk area of West Lancashire. The possible ancestors for this dog include the Corgi and Manchester Terrier.These useful farm dogs were bred for generations within this particular district, developing their own characteristics. Once bred as a cattle herder and a ratter, these friendly little dogs have gained popularity as a wonderful family dog.The breed was recognized by the Kennel Club in the U.K. in 1981 and was deemed a vulnerable native breed in 2003.Today, there is a growing interest in this great companion dog that happily participates in obedience, agility, rally and herding events. The Lancashire Heeler has gained popularity in the U.S, Sweden, the Netherlands and Australia." []
is_a: DBO:0000010 ! Foundation Stock Service

[Term]
id: DBO:0000156
name: Lapponian Herder
def: "For hundreds of years, the Lapps (Sami people) have used dogs of the same type as the Lapponian Herder to herd reindeer. The breed has been nicknamed "the reindeer herder" because of this original purpose. Acceptance to the breed register was started in the 1950s. At that time, the modern Finnish Lapphund and the Lapponian Herder were still recognized as the same breed. The Lapponian Herder was separated into its own breed October 12, 1966, as it had been noted that two different reindeer-herding breeds existed. In many regions, including its native land of Finland, the breed still herds and guards reindeer. The Lapponian Herder was accepted to the Foundation Stock Service program in April 2017." []
is_a: DBO:0000010 ! Foundation Stock Service

[Term]
id: DBO:0000157
name: Leonberger
def: "2010;The Leonberger was officially recognized by the AKC." []
is_a: DBO:0000004 ! Working Group

[Term]
id: DBO:0000158
name: Lhasa Apso(Long-Haired Lhasa Dog)
def: "1935;The Lhasa Apso was officially recognized by the AKC." []
is_a: DBO:0000007 ! Non-Sporting Group

[Term]
id: DBO:0000159
name: Lowchen(Little Lion Dog)
def: "Löwchen origins have long been subject to debate, and historians can't agree on the breed's birthplace. The name is German, but since the Middle Ages Löwchen were popular among noblewomen of France, Italy, Holland, Spain, and Russia, as well as Germany. Löwchen descend from the same ancient line that produced such companion breeds as the Bichon Frise and Maltese, and, thanks to sightings in the Renaissance art of several countries, we know that the Löwchen look hasn't changed for at least 500 years.1996;The Löwchen was officially recognized by the AKC." []
is_a: DBO:0000007 ! Non-Sporting Group

[Term]
id: DBO:0000160
name: Maltese
def: "1888;The Maltese was officially recognized by the AKC." []
is_a: DBO:0000006 ! Companion and Toy Group
synonym: "Maltese lion puppy" EXACT[]

[Term]
id: DBO:0000161
name: Manchester Terrier
def: "1886 (Toy)/1887 (Standard);The Manchester Terrier was officially recognized by the AKC." []
is_a: DBO:0000005 ! Terrier Group

[Term]
id: DBO:0000162
name: Miniature American Shepherd Dog
def: "2015;The Miniature American Shepherd was officially recognized by the AKC" []
is_a: DBO:0000008 ! Herding Group

[Term]
id: DBO:0000163
name: Miniature Bull Terrier
def: "1991;The Miniature Bull Terrier was officially recognized by AKC." []
is_a: DBO:0000005 ! Terrier Group

[Term]
id: DBO:0000164
name: Miniature Pinscher
def: "1925;The Miniature Pinscher was officially recognized by the AKC." []
is_a: DBO:0000006 ! Companion and Toy Group
synonym: "Min Pin" EXACT[]
synonym: "King of the Toys" EXACT[]

[Term]
id: DBO:0000165
name: Miniature Schnauzer
def: "1926;The Miniature Schnauzer was officially recognized by the AKC." []
is_a: DBO:0000005 ! Terrier Group

[Term]
id: DBO:0000166
name: Mountain Cur
def: "Mountain Curs are the true All-American Pioneer dog. They were a necessity to the frontier family and it is likely that the Southern Mountains could not have been settled without them. They were one of the biggest assets that the settlers had in the rough and unforgiving country of the Mountains. They guarded the family and livestock against wild animals or intruders.They were used to catch, tree, or hole wild game for the family's food. Until the 1940s, these dogs were part of the way of life for the frontiersmen. They used money from sold furs that their dogs hunted to provide for their families. The exact origins of this breed are undocumented, as there was no need for an official pedigree among the pioneers.The Mountain Cur was declared a breed in 1957 with the organization of the Original Mountain Cur Breeders of America (OMCBA). The most common strains of Mountain Cur included the McConnell, Stephens, Ledbetter, Arline and York strains, the categories being named after the owners of the dogs." []
is_a: DBO:0000010 ! Foundation Stock Service

[Term]
id: DBO:0000167
name: Hungarian Mudi
def: "The Magyars (the original name for Hungarians) kept sheepdogs starting around end of the ninth century, but pedigree breeding and classification of dogs only started in the second half of the 19th century. Before then, Hungarian sheepdogs were simply divided into two categories: large and small. When breeding, the small dogs were divided from the big ones (Kuvasz, Komondor), but the small ones were interbred. Therefore, the early history of the Mudi is more or less the same as those of the Pumi and the Puli.Around 1930, Dr. Deszö Fényesi, director of the museum in Balassagyarmat, was one of the first breeders to become involved in separate breeding of this small sheepdog. He is also the one who named the breed Mudi. By 1936, the Mudi was officially recognized as a breed.During World War II, many Hungarian breeds suffered terrible losses, some almost disappeared, and the Mudi was given no immunity as a rare breed. In the 1960s, it was rehabilitated from survivors, and in 1966, a new breed standard was written by Dr. Zoltan Balassy to apply for FCI recognition. This standard was based on only a handful of Mudis and the main differences between the original standard and this one were accepted sizes and colors. The FCI approved the breed standard in 1966, but very few people were involved in breeding then and this is still the case today.As the restoration of the breed went on over the next few decades, a naturally-occurring variability in color came to light that differed from the standard written in '66. A new standard was written in 2000 to add back most of these original colors and the present FCI breed standard dates from 2004." []
is_a: DBO:0000010 ! Foundation Stock Service

[Term]
id: DBO:0000168
name: Neapolitan Mastiff
def: "2004;The Neapolitan Mastiff was officially recognized by the AKC in 2004." []
is_a: DBO:0000004 ! Working Group

[Term]
id: DBO:0000169
name: Newfoundland
def: "1886;The Newfoundland was officially recognized by the AKC." []
is_a: DBO:0000004 ! Working Group

[Term]
id: DBO:0000170
name: Norfolk Terrier
def: "1979;The Norfolk Terrier was officially recognized by the AKC." []
is_a: DBO:0000005 ! Terrier Group

[Term]
id: DBO:0000171
name: Norrbottenspets
def: "For centuries, the people of the world's northernmost climes have bred a type of dog known as spitz. These Nordic breeds can be burly like the Alaskan Malamute or dainty like the Pomeranian, but spitz types share certain traits. These include a profusely coated tail curved tightly over the back, a wedge-shaped head usually bearing a foxlike expression, and erect, pointed ears. The Norrbottenspets (nor-bo-TEN-spets) is a member of this ancient clan of cold-weather hunters and workers.;The Norrbottenspets (or Norrbottenspitz in English) means spitz from the county of North Bothnia and probably originates from small Laika type spitz that were known to live with hunting people in the North Cape area in prehistoric time; small hunting spitz have survived for thousands of years through natural selection. In the very harsh areas of the northern parts of the Scandinavian Peninsula, hunting for food and fur was a necessity for survival. Precious furs like sable, marten-skin and ermine were the only valid currency for centuries. When fur prices dropped drastically after World War II, so did the interest for the Norrbottenspitz. The breed vanished and had no registrations for many years; hence the Swedish Kennel Club (SKK) declared it extinct. But only a decade later, news came that some true-to-type specimens had been found living as pets and watch dogs on small homesteads in the inland area of North Bothnia. Due to the very dedicated work of a few men, this old type hunting spitz was saved. In 1967, the Norrbottenspitz was reintroduced to the Registry in Sweden and a new standard was drawn up. The FCI accepted the new breed standard and the official name became Norrbottenspets.;Following the Swedish Kennel Club´s desire, Finns began to search the remote countryside of North Finland for native dogs that matched the standard to broaden the gene pool. They were successful and the majority of foundation dogs came from Finland. The studbook is still open in Finland, but was closed in the 1980s in Sweden. The Norrbottenspets population is about 1600 in Sweden and 1300 in Finland with scattered individuals counted in some tens around the world.;Norrbottenspets were accepted to the American Kennel Club's Foundation Stock Service in November 2007. As of November 2012, 181 Norrbottenspets, 175 of these with 3-generation pedigrees, were recorded with the American Kennel Club's Foundation Stock Service.2007;The Norrbottenspets was first recorded in the Foundation Stock Service." []
is_a: DBO:0000009 ! Miscellaneous

[Term]
id: DBO:0000172
name: Norwegian Buhund
def: "2009;The Norwegian Buhund was officially recognized by the AKC." []
is_a: DBO:0000008 ! Herding Group

[Term]
id: DBO:0000173
name: Norwegian Elkhound
def: "1913;The Norwegian Elkhound was officially recognized by the AKC." []
is_a: DBO:0000003 ! Hound Group

[Term]
id: DBO:0000174
name: Norwegian Lundehund
def: "2011;The Norwegian Lundehund was officially recognized by the AKC." []
is_a: DBO:0000007 ! Non-Sporting Group
synonym: "Lundehund" EXACT[]

[Term]
id: DBO:0000175
name: Norwich Terrier
def: "1936;The Norwich Terrier was officially recognized by the AKC." []
is_a: DBO:0000005 ! Terrier Group

[Term]
id: DBO:0000176
name: Nova Scotia Duck Tolling Retriever
def: "2003;The Nova Scotia Duck Tolling Retriever was officially recognized by the AKC." []
is_a: DBO:0000002 ! Sporting Group
synonym: "Toller" EXACT[]
synonym: "Duck Toller" EXACT[]

[Term]
id: DBO:0000177
name: Old English Shepherd Dog
def: "1888;The Old English Sheepdog was officially recognized by the AKC" []
is_a: DBO:0000008 ! Herding Group

[Term]
id: DBO:0000178
name: Otterhound
def: "In medieval England a huge otter population preyed on fish in rivers and stocked ponds. To protect this valuable food source, packs of Otterhounds were kept by country squires and even kings. As a sport, otter hunting was never as popular as the British gentry's cherished foxhunts, but it did help fill the spring and summer months for sportsmen waiting for the fall hunting season. Otterhound packs were so good at their work that river otters nearly went extinct and hunting them was outlawed.1909;The Otterhound was officially recognized by the AKC." []
is_a: DBO:0000003 ! Hound Group

[Term]
id: DBO:0000179
name: Papillon(Continental Toy Spaniel)
def: "1915;The Papillon was officially recognized by the AKC." []
is_a: DBO:0000006 ! Companion and Toy Group
synonym: "Butterfly Dog" EXACT[]
synonym: "Squirrel Dog (due to tail carriage)" EXACT[]

[Term]
id: DBO:0000180
name: Parson Russell Terrier
def: "1997;The Parson Russell Terrier was officially recognized by the AKC." []
is_a: DBO:0000005 ! Terrier Group

[Term]
id: DBO:0000181
name: Pekingese
def: "1906;The Pekingese was officially recognized by the AKC." []
is_a: DBO:0000006 ! Companion and Toy Group
synonym: "Peke" EXACT[]

[Term]
id: DBO:0000182
name: Pembroke Welsh Corgi
def: "1934;The Pembroke Welsh Corgi was officially recognized by the AKC." []
is_a: DBO:0000008 ! Herding Group
synonym: "Pembroke" EXACT[]
synonym: "PWC" EXACT[]
synonym: "Pem" EXACT[]
synonym: "Corgi" EXACT[]
synonym: "Welsh Corgi" EXACT[]

[Term]
id: DBO:0000183
name: Perro de Presa Canario(Canary Mastiff)
def: "There are numerous books written by Historians concerning the development of the known Perro de Presa Canario (the "Canary Dog of Prey"). Documentation of the original holding dogs date back to the fifteenth and sixteenth centuries. Following the conquest of the Canary Islands, it is theorized dogs of great size may have existed or were brought there by the Spanish Conquistadors or possibly both. What is known was the function for which these dogs were developed: guarding farms, working cattle and the extermination of wild or stray dogs.;There are several theories regarding the genetic contributions to the creation of the Presa Canario. It is almost certain that the cattle dog, the Iberian Presa (Perro de Ganado Majorero) provided a start to the founding of the Canary Presa. The Ganado was a mastiff type of average size, rustic, intelligent with an intuitive instinct; a fearless guardian. Several other Hispanic breeds contributed to the Presas formation, especially the Presa Espanol in its large varieties and the bulldog varieties (Alano), known for its clutching instincts. In time, the island dogs developed into a completely differentiated breed due to the influence of the Spanish breeds. The final ingredient that completes the foundation of the Presa Canario was the genetic infusion of the Bardino Majorero, a pre-Hispanic sheepdog originating on the Island of Fuerteventura. This dog was introduced for its intelligence, physical resistance, offering of excellent guardian instincts with little bark, extraordinary set of teeth and incorruptible courage. With the combination of all these traits, one more was added to the mix: the ability to fight.;In the 1940s, the prohibition of dog fighting was ordered throughout the islands, although clandestine fights were known to continue during the next decade. It was during this period the Presa Canario numbers truly faltered. The sovereignty of the island Presa worsened further with the introduction of the German Shepherd, Doberman Pinscher, and Great Dane. The island dog fancier's interest now focused on these new breeds, almost causing the demise of the Presa Canario breed. During this darkened period, the Presa was relegated in small numbers to farmers and herdsmen as their primary guard dog.;Reconstruction of the nearly extinct Presa Canario began in earnest back in the early 1970s. Reputable breeders bred strong Presas that were rustic, massive, vigorous, and functional, who had acute watchdog instincts, a strong temperament, calm yet confident and were extremely territorial with unlimited courage. This dog, when defending what he considers his, would withstand the harshest of punishments without surrendering his position.;Full recovery of the Presa Canario heritage started in 1982 when a group of breeders from the island of Tenerife formed an association with the goal to propagate the resurgence of the Presa Canario as started in the previous decades." []
is_a: DBO:0000010 ! Foundation Stock Service
synonym: "Presa" EXACT[]

[Term]
id: DBO:0000184
name: Peruvian Inca Orchid(Peruvian Hairless Dog)
def: "1996;The Peruvian Inca Orchid was first recorded in the Foundation Stock Service." []
is_a: DBO:0000009 ! Miscellaneous

[Term]
id: DBO:0000185
name: Petit Basset Griffon Vendeen
def: "1990;The Petit Basset Griffon Vendeen was officially recognized by the AKC." []
is_a: DBO:0000003 ! Hound Group
synonym: "PBGV" EXACT[]

[Term]
id: DBO:0000186
name: Pharaoh Hound
def: "1983;The Pharaoh Hound was officially recognized by the AKC." []
is_a: DBO:0000003 ! Hound Group

[Term]
id: DBO:0000187
name: Plott Hound
def: "2006;The Plott was officially recognized by the AKC." []
is_a: DBO:0000003 ! Hound Group

[Term]
id: DBO:0000188
name: English Pointer
def: "1884;The Pointer was officially recognized by the AKC" []
is_a: DBO:0000002 ! Sporting Group

[Term]
id: DBO:0000189
name: Polish Lowland Shepherd Dog
def: "2001;The Polish Lowland Sheepdog was officially recognized by the AKC." []
is_a: DBO:0000008 ! Herding Group
synonym: "PON" EXACT[]
synonym: "Nizinny" EXACT[]
synonym: "PLS" EXACT[]

[Term]
id: DBO:0000190
name: Pomeranian
def: "1888;The Pomeranian was officially recognized by the AKC." []
is_a: DBO:0000006 ! Companion and Toy Group
synonym: "Pompom" EXACT[]
synonym: "Pom" EXACT[]
synonym: "Tumbleweed" EXACT[]

[Term]
id: DBO:0000191
name: Porcelaine
def: "The Porcelaine is a medium-sized French scent hound. They were developed for flushing and hunting hare, deer, and wild boar. It is thought to be the oldest French scent hound breed in existence. He is also known as the Chien de Franche-Comte, referring to a French region bordering Switzerland.;As far back as the 1700s, there are records showing this breed in France and Switzerland. It is known that the background of the Porcelaine may include the English Harrier, Laufhounds, Montaimboeuf, and the Talbot Hound. Most of the breeding took place in Vaud, Savoy and the Abbeys of Luxeuil and Cluny, in particular with the family of Choiseul. During the French Revolution, the breed was nearly lost, but has since been reconstructed using French hounds such as Gray Harriers of Somerset, Gascon Saintongeois and the Billy. These outcrosses gave the Porcelaine vigor, size and strength to hunt wild boar and stag. Described as robust and tenacious, this is a hound capable of running long distances and working in steep, rugged terrain. The Club du Porcelaine in France was established in 1971 to safeguard the breed and, currently, there are moderate numbers of them in France and Italy. There are smaller numbers of the breed found throughout Europe and the United Kingdom. The breed was recognized by the FCI in 1975.;Porcelaines may have arrived in the United States as a gift from the King of France to President George Washington. There are records showing that Porcelaines were imported in the late 1800s through the Port of New Orleans, but were lost in crossbreeding with local hounds. More recently, Porcelaines were imported into the United States in 2009 and, currently, there is thought to be less than 300 in the U.S. and Canada.2017;The Porcelaine has been recorded in the Foundation Stock Service since April 2017." []
is_a: DBO:0000010 ! Foundation Stock Service

[Term]
id: DBO:0000192
name: Portuguese Pointer
def: "The Portuguese Pointer originated in the Iberian Peninsula. Its existence in Portugal can be traced back to the 12th century. It was originally bred in royal kennels to be used in falconry and is still used by falconers in Portugal today. In the 16th century, it became known as the perdigueiro, deriving this name from the Portuguese word "perdiz" meaning "partridge." During the 18th century, many English families in the business of wine production established a presence in the region of Oporto and came to know the Portuguese hunting breed, which were then taken to England where they played a part in the origin of the English Pointer. However, during the 19th century, when Portugal was experiencing considerable social hardships, the breed began a progressive decline. It wasn't until the 1920s that some breeders made an effort to salvage the breed by locating some of the ancient Portuguese dogs in the inaccessible north of Portugal. The Portuguese pedigree book was then established in 1932 and the breed standard in 1938. Today, after at least a thousand years, the breed still retains many of the same conformation and functional traits as its ancestors." []
is_a: DBO:0000010 ! Foundation Stock Service

[Term]
id: DBO:0000193
name: Portuguese Shepherd Dog
def: "Thought to be a relatively recently developed breed, the Portuguese Sheepdog's history is shrouded in mystery. Though there are a number of theories, what is definitely known is that the breed developed in Portugal, most likely in the central and southern areas, and has been found in the mountainous region of the Serra de Aires since the early 20th century. This region has been known as the native lands of other herding breeds as well, such as the Pyrenean Shepherd and Catalan Sheepdog, and one theory is that the Portuguese Sheepdog originated from the crossing of these breeds that came before it, though there is no solid evidence.;The most widely accepted theory is that the first Conde de Castro Guimaraes, Manuel Inácio de Castro Guimarães, in no earlier than 1909, imported a number of Briards from France to herd his flocks of sheep. (At the time, Briards were a well-regarded herding dog and famous throughout Europe for successfully aiding France in WWI.) Though the breed were excellent herders, they were ill-equipped to handle the local Portuguese climate and terrain. The Conde's solution was to cross his Briards with local herding breeds, possibly the previously mentioned Catalan Sheepdog and Pyrenean Shepherd. This theory is based on circumstantial evidence, though it very likely may be true due to the traits and appearance of the Portuguese Sheepdog. By the end of the 1920s, this new sheepherding breed became very well known in its native mountainous home as well as the adjacent region of Alentejo.;With Portugal's limited involvement in WWI and its complete absence from WWII, the Portuguese Sheepdog was saved from the sharp population declines prevalent in other European breeds at the time. In 1932, the Portuguese Kennel Club granted the breed full recognition, using a standard written by Dr. Antonio Cabral and Dr. Felipe Morgado Romeiros. However, due to modern technologies, the urbanization of its homelands, and a lack of international recognition, by the 1970s, the breed had become very rare and was thought to be on the verge of extinction.;Beginning in the late '70s, a group of breeders and owners banded together to bring back the breed. With the helpful push of a new group of fanciers during the '80s, the Portuguese Sheepdog was bred to be more of a companion dog and was thus discovered by middle class Portuguese suburbanites.;The FCI finally formally recognized the breed in 1996 as a member of the Herding Group. The breed is still rare outside Portugal and, within the country's borders, it is almost always seen as a companion, with only a very few dogs still herding in its native mountain region." []
is_a: DBO:0000010 ! Foundation Stock Service
synonym: "Cao macaco (monkey dog or macaque dog)" EXACT[]

[Term]
id: DBO:0000194
name: Portuguese Water Dog
def: "The Portuguese Water Dog once lived all along Portugal's coast, and was used to herd fish into nets, retrieve lost tackle, and act as a messenger between ships and shore. Fishermen counted on the strong and muscular dogs to be hardworking and seaworthy. They would ride in trawlers from the warm Atlantic waters of Portugal to the freezing cold waters off the coast of Iceland. Technology eventually laid him off from his job, but Porties are still used for water rescue.1983;The Portuguese Water Dog was officially recognized by the AKC." []
is_a: DBO:0000004 ! Working Group
synonym: "Portie" EXACT[]
synonym: "PWD" EXACT[]
synonym: "Water Dog" EXACT[]

[Term]
id: DBO:0000195
name: Pudelpointer
def: "The Pudelpointer is a rough-coated pointing dog that originates from two breeds, the Poodle and the Pointer. The idea behind the breed was to create a dog that combined the Poodle's intelligence, love of water, retrieving instincts, easy trainability, willingness to please, and protective coat with the Pointer's endless desire to hunt, birdiness, pointing instincts, field nose and endurance.;The first cross of a Poodle and an English Pointer to establish the new breed took place in Germany in 1881. The sire was an English Pointer owned by Kaiser Frederick III named Tell and the dam, a Poodle named Molly, belonged to a famous Teutonic author on the subject of hunting dogs, Hegewald.;The Poodle's genes, as a breed, seemed to have been more dominant in passing on. To alter this, many more Pointers than Poodles were introduced into the breeding program to arrive at what the Pudelpointer is today. During the first 30 years of breeding, only 11 Poodles were used as opposed to well over 80 Pointers. After that initial time period, only the occasional reintroduction of the Pointer was needed. After World Wars I and II, the breed became severely depleted and the reintroduction of the Pointer became important again to rebuild the breeding stock.;The first Pudelpointers in North America were imported in 1956. After the breed's foundation was laid, the Pudelpointer Club of North America was founded in 1977 in Canada." []
is_a: DBO:0000010 ! Foundation Stock Service

[Term]
id: DBO:0000196
name: Pug
def: "1885;The Pug was officially recognized by the AKC." []
is_a: DBO:0000006 ! Companion and Toy Group

[Term]
id: DBO:0000197
name: Hungarian Puli
def: "1936;The Puli was officially recognized by the AKC." []
is_a: DBO:0000008 ! Herding Group

[Term]
id: DBO:0000198
name: Hungarian Pumi
def: "2016;The Pumi was officially recognized by the AKC" []
is_a: DBO:0000008 ! Herding Group

[Term]
id: DBO:0000199
name: Pyrenean Mastiff
def: "While the origin of the Pyrenean Mastiff is not clearly known, it is generally accepted that the breed is descended from molosser dogs brought from Sumeria and Assyria to Spain by the Phoenicians some 3,000 years ago. Due to the remoteness of the various areas of the Pyrenees Mountains and the rest of the region now known as Spain, the original molosser dogs developed divergently by region into several livestock guardian breeds, the Pyrenean Mastiff, the Spanish Mastiff, and the breed most closely related to the Pyrenean Mastiff, the Pyrenean Mountain Dog, which is also known as the Great Pyrenees.In the early middle ages, the area that would later become Spain was split between the Christian kingdoms of Castile and Aragon in the north, and the Muslim-controlled areas of the south. In the wide and flat area of Castile, the smooth-coated Spanish Mastiff was developed to protect flocks of sheep that traveled over long distances. In the Aragon region, the less homogeneous Pyrenees Mountains developed more rugged and longer-haired livestock protectors. Following the Trashumante, or formal mass migration of flocks to and from grazing grounds established by the Visigoth King Eurico in 504 A.D, herds of sheep 1,000 strong accompanied by a shepherd and five mastiffs would make the migration through the bear and wolf-infested Pyrenees Mountains and foothills. Named for the area of their Trashumante source, the Navarran Mastin (also Mastin of Navarra) and the Mastin d'Aragon, these livestock protectors were highly esteemed, and as such, received the same food allotments as the shepherds. They also wore a carlanca, a spiked collar that protected their necks while engaging wolves and bears. This migration lasted well into the 18th century.;In 1659, Mazarino, the Regent of France, and Phillippe IV, King of Spain, signed a decree splitting ownership of the Pyrenees Mountains with the northern area becoming French territory, and the Southern area remaining Spanish territory. The northern, or French, area further refined their mastiff, developing a white, longer-haired breed, the Pyrenean Mountain Dog, that possessed a more refined head and stature. The Pyrenean Mountain Dog enjoyed widespread recognition due to its popularity and strong breeding programs, while the Spanish mastiffs in the south continued their work as livestock guardians and remained more massive, primitive, and less homogenous.;In the 1930s and '40s, the disappearance of the wolf and bear from the Pyrenees Mountains, the new reliance on rail to transport sheep, the Spanish Civil War followed by World War II, and a scarcity of food almost led to the total loss of the Mastiffs of Aragon. Being very large and expensive to support and with no further purpose besides guarding livestock, these noble dogs became almost extinct.;With the return of a pack of wolves to the Aragon region in the 1970s, there was once again a need for these dogs, now known as the Pyrenean Mastiff. At the same time, a small group of enthusiasts for this breed set to work reviving it, finding approximately 100 specimens of the breed and then narrowing it down to the best 30 that most closely resembled the standard and that displayed the proper temperament and excellent health.  Their breeding program resulted in today's Pyrenean Mastiff that is known for its great size, strong build, graceful movement, and its gentle, non-aggressive and even temperament. Yet the Pyrenean Mastiff still possesses great fighting skills, honed through centuries of protecting livestock, but will put them to use only when pressed to meet aggressive behavior to protect itself, its people, its flock, its pack or its home.;While still relatively rare, the breed has since spread throughout Western and Eastern Europe, Scandinavia, Russia, Australia, Japan, and on to Mexico, the US, and now Canada, with somewhere between 4,000 and 6,000 worldwide. They are FCI approved and are shown successfully in the FCI affiliated clubs of most of these countries.2014;The Pyrenean Mastiff was recorded in the Foundation Stock Service" []
is_a: DBO:0000010 ! Foundation Stock Service

[Term]
id: DBO:0000200
name: Pyrenean Shepherd Dog
def: "2009;The Pyrenean Shepherd was officially recognized by the AKC." []
is_a: DBO:0000008 ! Herding Group
synonym: "Pyr Shep" EXACT[]

[Term]
id: DBO:0000201
name: Rafeiro do Alentejo(Portuguese Mastiff)
def: "The Rafeiro do Alentejo is believed to descend from molosser dogs from the Middle East. On account of their size and courage, they were used by tribes whose livelihood depended on livestock husbandry, thus performing a crucial role for this type of community.;With the beginning of the transhumance in Portugal, it was noticed that the migrating herds and shepherds were exposed to many dangers during their long journeys. So on their route to the mountains in the summer and back to the plains in the winter, flocks were always accompanied by large dogs, which lead to the dogs being spread along the route from region to region. As the population settled down, the dogs eventually remained in the southern prairies, the Alentejo plains, where they adapted and began to be used to guard, not only the herds, but the big rural estates as well. The official standard of the Rafeiro do Alentejo was first established in 1953 in Portugal." []
is_a: DBO:0000010 ! Foundation Stock Service

[Term]
id: DBO:0000202
name: American Rat Terrier
def: "2013;The Rat Terrier was officially recognized by the AKC." []
is_a: DBO:0000005 ! Terrier Group
synonym: "RT" EXACT[]
synonym: "Rat" EXACT[]
synonym: "Rattie" EXACT[]

[Term]
id: DBO:0000203
name: Redbone Coonhound
def: "Redbones are one of six hounds developed by American settlers to provide a steady source of raccoon meat and fur during the new nation's expansion to the south and west. Coonhounds are often portrayed in pop culture as lazy ol' dawgs snoozing away their lives on the front porch. But anyone who's been on a "nite hunt" in pursuit of the wily, nocturnal raccoon will tell you that Redbones and their cooner cousins are among dogdom's most tireless and tenacious pursuers.2009;The Redbone Coonhound was officially recognized by the AKC." []
is_a: DBO:0000003 ! Hound Group
synonym: "Reds" EXACT[]

[Term]
id: DBO:0000204
name: Rhodesian Ridgeback
def: "1955;The Rhodesian Ridgeback was officially recognized by the AKC." []
is_a: DBO:0000003 ! Hound Group

[Term]
id: DBO:0000205
name: Rottweiler
def: "1931;The Rottweiler was officially recognized by the AKC." []
is_a: DBO:0000004 ! Working Group
synonym: "Rott" EXACT[]
synonym: "Rottie" EXACT[]

[Term]
id: DBO:0000206
name: Russell Terrier
def: "2012;The Russel Terrier was officially recognized by the AKC." []
is_a: DBO:0000005 ! Terrier Group

[Term]
id: DBO:0000207
name: Russian Toy Terrier
def: "2008;The Russian Toy was recorded in the Foundation Stock Service by KAC." []
is_a: DBO:0000010 ! Foundation Stock Service

[Term]
id: DBO:0000208
name: Russian Tsvetnaya Bolonka
def: "2015;The Russian Tsvetnaya Bolonka has been recorded in the Foundation Stock Service since February 2015 by AKC." []
is_a: DBO:0000010 ! Foundation Stock Service

[Term]
id: DBO:0000209
name: Saluki
def: "1929;The Saluki was officially recognized by the AKC." []
is_a: DBO:0000003 ! Hound Group

[Term]
id: DBO:0000210
name: Samoyed
def: "1906;The Samoyed was officially recognized by the AKC." []
is_a: DBO:0000004 ! Working Group
synonym: "Smiley" EXACT[]
synonym: "Sammy" EXACT[]

[Term]
id: DBO:0000211
name: Schapendoes
def: "2005;The Schapendoes was recorded in the Foundation Stock Service by AKC." []
is_a: DBO:0000010 ! Foundation Stock Service

[Term]
id: DBO:0000212
name: Schipperke
def: "1904;First recognized by the AKC." []
is_a: DBO:0000007 ! Non-Sporting Group
synonym: "Spitzke (until 1888)" EXACT[]
synonym: "Spits (until 1888)" EXACT[]
synonym: "Spitske (until 1888)" EXACT[]

[Term]
id: DBO:0000213
name: Scottish Deerhound
def: "1886;The Scottish Deerhound was first recognized by the AKC." []
is_a: DBO:0000003 ! Hound Group

[Term]
id: DBO:0000214
name: Scottish Terrier
def: "1885;The Scottish Terrier was officially recognized the AKC." []
is_a: DBO:0000005 ! Terrier Group
synonym: "Scottie" EXACT[]
synonym: "Aberdeenie" EXACT[]

[Term]
id: DBO:0000215
name: Sealyham Terrier
def: "1911;The Sealyham Terrier was recognized by the AKC." []
is_a: DBO:0000005 ! Terrier Group

[Term]
id: DBO:0000216
name: Shetland Shepherd Dog
def: "1911;The Shetland Sheepdog was officially recognized by the AKC." []
is_a: DBO:0000008 ! Herding Group
synonym: "Sheltie" EXACT[]

[Term]
id: DBO:0000217
name: Japanese Shiba Inu
def: "1992;The Shiba Inu was officially recognized by the AKC." []
is_a: DBO:0000007 ! Non-Sporting Group
synonym: "Shiba" EXACT[]

[Term]
id: DBO:0000218
name: Shih Tzu(Chrysanthemum Dog)
def: "1969;The Shih Tzu was officially recognized by the AKC." []
is_a: DBO:0000006 ! Companion and Toy Group

[Term]
id: DBO:0000219
name: Kochi Ken(Shikoku)
def: "2014;The Shikoku has been recorded in the Foundation Stock Service since October 2014." []
is_a: DBO:0000010 ! Foundation Stock Service

[Term]
id: DBO:0000220
name: Siberian Husky
def: "1930;The Siberian Husky was officially recognized by the AKC." []
is_a: DBO:0000004 ! Working Group
synonym: "Husky" EXACT[]
synonym: "Sibe" EXACT[]

[Term]
id: DBO:0000221
name: Silky Terrier
def: "1959;The Silky Terrier was officially recognized by the AKC." []
is_a: DBO:0000006 ! Companion and Toy Group

[Term]
id: DBO:0000222
name: Skye Terrier
def: "1887;The Skye was first registered with the AKC." []
is_a: DBO:0000005 ! Terrier Group

[Term]
id: DBO:0000223
name: Sloughi
def: "2016;The Sloughi was officially recognized by the AKC" []
is_a: DBO:0000003 ! Hound Group

[Term]
id: DBO:0000224
name: Slovensky Cuvac
def: "nan" []
is_a: DBO:0000010 ! Foundation Stock Service

[Term]
id: DBO:0000225
name: Slovensky Kopov(Slovakian Hound)
def: "2015;The Slovensky Kopov has been recorded in the Foundation Stock Service since October 2015. A well-known type of hunting dog since antiquity, today's breed was first recognised in the 1870s. The breeds of Brandlbracke (Austrian Black and Tan Hound), Chart Polski, and Magyar Agar (Hungarian Greyhound) are believed to have been used in the breed's background. The etymology of the name seems to refer to the dog's colour. The breed club was established in Bratislava in 1988.The Slovenský kopov was developed and is used as a hunting dog, not a pet or showdog. It is bred for hunting large game, especially wild boar. Although extremely common in its area of origin, it is rarely seen in other countries.The Slovenský kopov is similar to other East-European scenthounds in appearance and hunting style." []
is_a: DBO:0000010 ! Foundation Stock Service

[Term]
id: DBO:0000226
name: Smooth Fox Terrier
def: "1885;The Smooth Fox Terrier was officially recognized by the AKC." []
is_a: DBO:0000005 ! Terrier Group

[Term]
id: DBO:0000227
name: Soft-Coated Wheaten Terrier
def: "1973;The Soft Coated Wheaten Terrier was officially recognized by the AKC." []
is_a: DBO:0000005 ! Terrier Group
synonym: "Wheaten or Wheatie" EXACT[]

[Term]
id: DBO:0000228
name: Spanish Mastiff
def: "nan" []
is_a: DBO:0000010 ! Foundation Stock Service

[Term]
id: DBO:0000229
name: Spanish Water Dog
def: "2015;The Spanish Water Dog was officially recognized by the AKC." []
is_a: DBO:0000008 ! Herding Group

[Term]
id: DBO:0000230
name: Spinone Italiano
def: "2000;The Spinone Italiano was officially recognized by the AKC." []
is_a: DBO:0000002 ! Sporting Group
synonym: "Spinone" EXACT[]

[Term]
id: DBO:0000231
name: St. Bernard
def: "1885;The St. Bernard was officially recognized by the AKC." []
is_a: DBO:0000004 ! Working Group
synonym: "Saint" EXACT[]

[Term]
id: DBO:0000232
name: Stabyhoun
def: "nan" []
is_a: DBO:0000010 ! Foundation Stock Service
synonym: "Staby" EXACT[]

[Term]
id: DBO:0000233
name: Staffordshire Bull Terrier
def: "1974;The Stafford Bull Terrier was officially recognized by the AKC." []
is_a: DBO:0000005 ! Terrier Group
synonym: "Staffy" EXACT[]
synonym: "Nanny Dog" EXACT[]

[Term]
id: DBO:0000234
name: Standard Schnauzer
def: "1904;The Standard Schnauzer was officially recognized by the AKC." []
is_a: DBO:0000004 ! Working Group

[Term]
id: DBO:0000235
name: Sussex Spaniel
def: "1884;The Sussex Spaniel was officially recognized by the AKC." []
is_a: DBO:0000002 ! Sporting Group
synonym: "Sussex" EXACT[]

[Term]
id: DBO:0000236
name: Swedish Lapphund
def: "The Swedish Lapphund is the oldest of the native Swedish breeds and is believed to be one of the most ancient breeds in existence today. It was an important partner of the Sami people of Lappland (northern Norway, Sweden, Finland and northwest Russia) initially as a hunting and guarding dog and later as a herding partner with the domestication of reindeer. A characteristic of the herding Lappie is the use of his vocal talents. It is believed the Sami favored the barking Lappies for two reasons: predators were deterred from coming too close and the reindeer knew the barking, four-legged creature was friend, not foe. The herding instinct is still alive and well in the modern day Lappie.;The breed was near extinction in the mid-20th century, but through the dedicated efforts of several breeders it was revived. Today, it still remains a very rare breed with an estimate of approximately 1000-1200 worldwide, the majority of which are in Sweden." []
is_a: DBO:0000010 ! Foundation Stock Service

[Term]
id: DBO:0000237
name: Swedish Vallhund
def: "2007;The Swedish Vallhund was officially recognized by the AKC." []
is_a: DBO:0000008 ! Herding Group

[Term]
id: DBO:0000238
name: Taiwan Dog
def: "2017;The Taiwan Dog has been recorded in the Foundation Stock Service since May 2017." []
is_a: DBO:0000010 ! Foundation Stock Service

[Term]
id: DBO:0000239
name: Teddy Roosevelt Terrier
def: "August 2016;The Teddy Roosevelt Terrier first recorded in the Foundation Stock Service" []
is_a: DBO:0000010 ! Foundation Stock Service

[Term]
id: DBO:0000240
name: Thai Ridgeback
def: "The origin of the Thai Ridgeback is undocumented, but the breed was developed in eastern Thailand. The history of the breed is the subject of numerous hypotheses.The other existing purebreeds of ridgeback dog are the Rhodesian Ridgeback from Africa and the Phu Quoc Ridgeback from Vietnam, which is somewhat smaller than the Thai Ridgeback. Based on genetic-based hypothesis, both Thai Ridgeback Dog and Phu Quoc Dog are likely to be descended from Funan Ridgeback Dog which originated over 1,000 years ago in Funan Era of the region. The descendent of the Hottentot Dog or Ari Dog (as called by the tribe), a known African ridge-bearing ancestor of the Rhodesian Ridgeback, is now found as Africanis. The gene that causes the ridge has been inherited from a common ancestor: "The geographical origin of the ridge present in Ridgeback dogs is still a mystery, thus solid proof has now been provided that the ridge mutation in Ridgeback dogs is identical by descent and the likelihood of parallel mutations occurring in Asia and Africa (Epstein, 1937) can therefore be rejected."" []
is_a: DBO:0000010 ! Foundation Stock Service

[Term]
id: DBO:0000241
name: Tibetan Mastiff
def: "2007;The Tibetan Mastiff was officially recognized by the AKC." []
is_a: DBO:0000004 ! Working Group

[Term]
id: DBO:0000242
name: Tibetan Spaniel
def: "1983;The Tibetan Spaniel was officially recognized by the AKC." []
is_a: DBO:0000007 ! Non-Sporting Group

[Term]
id: DBO:0000243
name: Tibetan Terrier
def: "1973;The Tibetan Terrier was officially recognized by the AKC." []
is_a: DBO:0000007 ! Non-Sporting Group

[Term]
id: DBO:0000244
name: Tornjak(Bosnian and Herzegovinian-Croatian Shepherd Dog)
def: "nan" []
is_a: DBO:0000010 ! Foundation Stock Service

[Term]
id: DBO:0000245
name: Tosa Inu(Tosa)
def: "This breed originated in the second half of the nineteenth century. The breed started from the native Shikoku-Inu, an indigenous dog weighing about 25 kilograms (45 pounds) and standing about 55 centimetres high, which closely resembles the European Spitz. These dogs were crossed with European dog breeds, such as the Old English Bulldog in 1872, Mastiff in 1874, St. Bernard, German Pointer in 1876, Great Dane in 1924, and the Bull Terrier.[2] The aim was to breed a larger, more powerful dog. The heyday of Tosa breeding was between 1924 and 1933, when it was said that there were more than 5,000 Tosa breeders in Japan." []
is_a: DBO:0000010 ! Foundation Stock Service

[Term]
id: DBO:0000246
name: Toy Fox Terrier
def: "In the early 20th century, American breeders of Smooth Fox Terriers created the TFT by crossing their litter runts with toy dogs, Chihuahuas and Italian Greyhounds among them. The result was a dog possessing the fire of a true terrier but with a beguiling toy-breed personality. They began as barnyard ratters but soon found their way to show business, where their cleverness, grace, and nifty looks served them well as circus trick dogs. Today they perform at championship levels in competitive agility.2003;The Toy Fox Terrier was officially recognized by the AKC." []
is_a: DBO:0000006 ! Companion and Toy Group

[Term]
id: DBO:0000247
name: Transylvanian Hound
def: "nan" []
is_a: DBO:0000010 ! Foundation Stock Service

[Term]
id: DBO:0000248
name: Treeing Tennessee Brindle
def: "1995;The Treeing Tennessee Brindle was recorded in the Foundation Stock Service" []
is_a: DBO:0000010 ! Foundation Stock Service

[Term]
id: DBO:0000249
name: Treeing Walker Coonhound
def: "2012;The Treeing Walker Coonhound was officially recognized by the AKC." []
is_a: DBO:0000003 ! Hound Group
synonym: "Walker" EXACT[]

[Term]
id: DBO:0000250
name: Hungarian Vizsla
def: "1960;The Vizsla was officially recognized by the AKC in 1960." []
is_a: DBO:0000002 ! Sporting Group

[Term]
id: DBO:0000251
name: Weimaraner
def: "1943;The Weimaraner was officially recognized by the AKC." []
is_a: DBO:0000002 ! Sporting Group
synonym: "Weim" EXACT[]
synonym: "Grey Ghost" EXACT[]

[Term]
id: DBO:0000252
name: Welsh Springer Spaniel
def: "1906;The Welsh Springer Spaniel was officially recognized by the AKC." []
is_a: DBO:0000002 ! Sporting Group
synonym: "Welshie" EXACT[]

[Term]
id: DBO:0000253
name: Welsh Terrier
def: "1888;The Welsh Terrier was officially recognized by the AKC." []
is_a: DBO:0000005 ! Terrier Group

[Term]
id: DBO:0000254
name: West Highland White Terrier
def: "1908;The West Highland White Terrier was officially recognized by the AKC." []
is_a: DBO:0000005 ! Terrier Group
synonym: "Westie (or Westy)" EXACT[]

[Term]
id: DBO:0000255
name: English Whippet
def: "1888;The Whippet was officially recognized by the AKC." []
is_a: DBO:0000003 ! Hound Group

[Term]
id: DBO:0000256
name: Wire-Haired Fox Terrier
def: "1885;The Wire Fox Terrier was officially recognized by the AKC." []
is_a: DBO:0000005 ! Terrier Group
synonym: "Wire" EXACT[]

[Term]
id: DBO:0000257
name: Wire-Haired Pointing Griffon
def: "1887;The Wirehaired Pointing Griffon was officially recognized by the AKC." []
is_a: DBO:0000002 ! Sporting Group

[Term]
id: DBO:0000258
name: Wire-Haired Vizsla
def: "2014;The Wirehaired Vizsla was officially recognized by the AKC." []
is_a: DBO:0000002 ! Sporting Group

[Term]
id: DBO:0000259
name: Working Kelpie
def: "The Working Kelpie is an Australian sheep dog successful at mustering and driving with little or no command guidance. They are medium-sized dogs and come in a variety of colors. Historically, it is interesting to observe that the dogs which formed the foundation of the Australian Working Kelpie sheepdog were not owned, as one might expect, by shepherds, but land/property holders who were members of highly-respected and well-known families. George Robertson and his cousin John G. Robertson came from Scotland to Victoria; the 5 Rutherford brothers immigrated to Australia in the mid-1800s and are from a very well-established sheep farming family in Sutherlandshire, NSW; Gilbert S. Elliot and William Allan were both sons of very well-connected families in England and Scotland. The foundation of the Kelpie breed happened by sheer chance and the results have been of tremendous value to the Australian pastoral industries.;The breed's origins begin with a pair of black and tan Collies, named Brutus and Jennie, who were brought from Jedburgh, Scotland by Arthur Robinson for his brother-in-law Gilbert Elliot. Following the death of Gilbert Elliot, William Allan took Brutus with him to Queensland. Caesar, one of the litter born on the way to Australia, became the property of Mr. John Rich of Narriah station, a property that adjoined Yalgogrin. It was while Jack Gleeson was managing Yalgogrin that he mated his dog, named Kelpie, to Caesar to produce the litter of which Kings Kelpie was a part.;Because of the short time between the arrival of Brutus and Jennie, Gilbert Elliot's death, and Williams Allan's move to Queensland, the bloodlines of this imported Collie pair was limited and, to date, the only records held are that Caesar mated to Gleeson's Kelpie producing Kings Kelpie; Nero owned by James Cunningham of Kildary station; Swan ll and Wylie ll all of which bred on well; Laddie, Caesar's litter brother, was mated to King's Kelpie to produce the dam of The Barb and a couple of unnamed dogs bred and owned by R M Macpherson. During the 1800s, these early ancestors of the Working Kelpie were shown and displayed at various sheepdog trials and other competitions, where they won not only the competitions, but the love and admiration of the people who watched them work so quickly and effortlessly.;Kelpies have been exported throughout the world and are used to muster livestock, primarily sheep, cattle and goats. They were brought to North America around the turn of the century to expedite livestock handling.2014;The Working Kelpie was recorded in the Foundation Stock Service." []
is_a: DBO:0000008 ! Herding Group

[Term]
id: DBO:0000260
name: Yorkshire Terrier
def: "1885;The Yorkie was first recognized by the AKC." []
is_a: DBO:0000006 ! Companion and Toy Group
synonym: "Yorkie" EXACT[]

[Term]
id: DBO:0000261
name: Toy Manchester Terrier
def: "Like the Manchester Terrier, the Toy version was developed from the old English Black and Tan Terrier, known in Britain for some 400 years. Like his larger relative, the Toy triumphed as a ratter. Despite his small stature, he was formidable to vermin as was demonstrated in 1848 when a proud owner bet his dog could kill 300 rats in three hours. The match, held in the Queen's Hotel Tavern in London, pitted Tiny The Wonder against the vermin. The 5-1/2-pounder did in the entire lot in just 54 minutes and 50 seconds! The Toy Manchester breed suffered a setback toward the mid-19th century, when breeders became more concerned with small size than health and soundness. Fortunately, there were enough caring breeders to correct the problems and put the Toy Manchester back on its feet." []
is_a: DBO:0000006 ! Companion and Toy Group

[Term]
id: DBO:0000262
name: American Cocker Spaniel
def: "When Cocker Spaniels were imported to North America in the 1880s, the breed gradually changed as breeders produced a smaller dog, higher on leg, shorter in back, with a sloping topline, shorter muzzle, more domed skull, heavier coat and profuse leg furnishings. By the 1930s, the differences between North American and English Cockers were so obvious, efforts were made to split the breed. In 1947, the original Cocker was renamed the English Cocker Spaniel and the new variety retained the name Cocker Spaniel in the U.S. Elsewhere, it is known as the American Cocker Spaniel. The breed almost became too popular for its own good when Ch. My Own Brucie took Best in Show at the famed Westminster Kennel Club show in 1940 and '41. Overpopulation threatened to destroy the Cocker's merry temperament, but the trend has now reversed and the breed's personality is as attractive as its appearance." []
is_a: DBO:0000002 ! Sporting Group

[Term]
id: DBO:0000263
name: Wire-Haired Collie
def: "A native of Scotland, the Rough Collie is believed to have descended from herding dogs brought to Britain at the time of the Roman invasion. The breed has been mentioned in writings dating back to the 14th century. It was used primarily as a herding dog. The breed owes its initial popularity to Queen Victoria who brought some of the breed back from Scotland and installed them in the royal kennels at Windsor. Then along came the popular books of Albert Payson Terhune and 'Lassie' of movie and TV fame and the breed surged into the hearts of North Americans. It is believed that a cross to the Borzoi gave the breed its long, aristocratic head." []
is_a: DBO:0000008 ! Herding Group
synonym: "Collie Rough" EXACT[]

[Term]
id: DBO:0000264
name: Smooth-Haired Collie
def: "Identical to the Rough Collie in all respects except for coat length, the Smooth Collie is of the same lineage. Though the Smooths were also herding dogs, they proved to be more popular for driving sheep. Collies take their name from the black-faced Scottish sheep that were known as "colleys" (meaning black) and were called "colley dogs."" []
is_a: DBO:0000008 ! Herding Group
synonym: "Collie (Smooth Coat)" EXACT[]

[Term]
id: DBO:0000265
name: Dutch Smoushond
def: "The exact origins of the Smoushond are unknown. The breed was popular in the late 1800's as a gentleman's companion, but World War II pushed it near extinction. In the 1970's a Mrs. H.M. Barkman began collecting information on the breed and was able to recreate it through selective breeding. Today it breeds true for both type and temperament. The breed is hardly known outside of the Netherlands. ;; The Dutch Smoushond was recognized by the United Kennel Club in 2006." []
is_a: DBO:0000005 ! Terrier Group

[Term]
id: DBO:0000266
name: Treeing Feist
def: "The word "feist" is an ancient one referring to a small, often noisy, dog. Like the Cur breeds, the Feist breeds were developed in the rural South by breeders who needed low-maintenance dogs to hunt small game and to eliminate vermin. Feists were often the result of crosses between hunting hounds and terriers. Todays Treeing Feist is the result of generations of breeding for performance and it is still primarily used to hunt squirrel, although they are also used to hunt raccoon, rabbits and flushing game birds. ;; The Treeing Feist was recognized by UKC on November 1, 1998." []
is_a: DBO:0000005 ! Terrier Group

[Term]
id: DBO:0000267
name: Alaunt
def: "The Molossus descended into Epirus in about 1200 BC,[clarification needed] also from the north. However, their artifacts did not resemble the Mastiff prototype, as they had a long nose of a narrow type, and a long mane. Varro, however, described a herding dog of Epirus which was white, large headed, and slightly undershot, used to defend sheep and goats.[1] One group of Alans arrived in what is now Albania in the fifth or sixth centuries BC.[2] Molossis of Epirus is located in Southern Albania.[3] It is most plausible the Alaunt gave rise to the fighting dogs of the Molossi,[citation needed] which were introduced to Britain by Roman Invasion in 55BC. The Alans provided cavalry for Rome and in 50AD, 5,500 Alans were sent to Britain to guard Hadrian's Wall.[4] Thus, the Alaunt genetic template most plausibly gave rise to the British Pugnaces as fighting dogs which English Mastiffs and Bulldogs descend from.In the 370s AD, Hun invasions divided the Alani into the Eastern and Western Alans. The Eastern Alani tribes merged with the Ossetians and other nations, introducing their dogs into the bloodlines of many Balkan breeds, such as the Shar Mountain Dog, Metchkar, Qen Ghedje, Hellenikos Poimenikos and other Molossers of the region.[citation needed] Some believe[who?] that the white-coloured Alaunts were the direct ancestors of Balkan breeds, which in turn influenced all other white dogs in the Balkans.The Western Alans joined the Vandals on their raids through Europe and by the 410s AD, their fierce dogs were influencing many breeds in France, Spain, Portugal, England and other countries, spreading the use of the "alaunt" name, which became synonymous with a type of a working dog, rather than a specific breed. Through breeding with various scenthounds and sighthounds, some alaunts became valued large game hunting dogs, existing in a variety of types, dictated by regional preferences. In 1500 AD, Spain was known for breeding the best Alaunts and used them to conquer the New World.In France, Alaunts were separated into three main categories, based on physical appearance and the duties they performed. The lightest type was the Alaunt Gentil, a greyhound-like dog, which eventually became assimilated into the local hunting breeds with the Alaunt Veantre. The original mastiff variety, known as the Alaunt de Boucherie, was crucial in the development of the fighting and baiting dogs of France. The Alaunt de Boucherie in France was known as the Alaunt Butchers in England and the Alano in Spain and Italy and were termed the original Bulldogs as they were used to control and defend herds of cattle. In Spain, the three categories were the Mastins, Alanos, and Lebrels, further separated as the ayuda (defense types) and the presa (offense types), such as the Presa Canario, Fila Brasileiro, and Cuban Mastiff." []
is_a: DBO:0000011 ! Extinct

[Term]
id: DBO:0000268
name: Alpine Mastiff
def: "The Alpine Mastiff is an extinct Molosser dog breed, the progenitor of the St. Bernard, and a major contributor to the modern Mastiff (through such dogs as "Couchez"),as well as to other breeds that derive from these breeds or are closely related to them. M.B. Wynn wrote, "In 1829 a vast light brindle dog of the old Alpine mastiff breed, named L'Ami, was brought from the convent of Great St. Bernard, and exhibited in London and Liverpool as the largest dog in England." William Cavendish, 5th Duke of Devonshire, is believed to have bred Alpine Mastiffs at Chatsworth House.The names "Alpine Mastiff" and "Saint Bernard" were used interchangeably in the early 19th century, though the variety that was kept at the hospice at the Great St. Bernard Pass was significantly altered by introducing other breeds, including Newfoundland and Great Dane,and it is this composite breed that now carries the name St. Bernard. Inevitably these Mountain dogs filtered through to the wider population, and the original variety dwindled in its pure form, though a rare breed, the "Cane Garouf" or "Patua",found in the part of the Alps formerly inhabited by the Alpine Mastiff, may also descend from the extinct breed.The Alpine Mastiff was, along with the Tibetan Mastiff and Caucasian Shepherd Dog, one of the earliest breeds of dog to reach truly gigantic size. It was one of the very first true mastiffs, originating in northern Europe before 500 B.C. The largest individuals may have reached more than 1 m (39 in) tall at the shoulder and weighed 160 kg (350 lb) or more, surpassing the modern Saint Bernard and English Mastiff in size. Beginning in the 1970s, there have been some efforts to breed back the Alpine Mastiff, mainly by using breeds such as the Saint Bernard, Great Dane, Great Pyrenees, and Bernese Mountain Dog." []
is_a: DBO:0000011 ! Extinct

[Term]
id: DBO:0000269
name: Alpine Spaniel
def: "Alpine spaniels were kept by the canons of the monasteries in the Alps in order to search for travellers during heavy snow storms, including the Great St Bernard Hospice in the Great St Bernard Pass between Italy and Switzerland.[3][5] The dogs would be dispatched in pairs to search for fallen travellers, and were trained so that upon finding them would return to the canons in order to lead rescuers back to the unfortunate individuals.[6] The Alpine breed was also used as a watchdog to guard sheep and cattle of mountainous regions, including the Himalayas.Between 1800 and 1814, a dog named Barry lived as a rescue dog at the hospice, and was famous enough at the time for his body to be preserved at the Natural History Museum of Bern. However, during the preservation, the taxidermist and the director of the Museum agreed to modify the body towards what they thought was a good example of the breed during that period. The head itself was further modified in 1923 to represent the Saint Bernard of that era. Prior to this the skull was a great deal flatter with a moderate stop.In 1829 a Mastiff like dog was brought from the Great St Bernard Hospice and was exhibited in London and Liverpool to thousands of people. This publicised the existence of an Alpine Mastiff, but drawings of the dog did not match descriptions of the Alpine Spaniel from before the exhibition, and the descriptions of the Spaniel were ridiculed by later publications.Because of the treacherous conditions in which this breed of dog was used, coupled with a succession of accidents, talk of the whole stock becoming extinct was raised as early as 1839.[10] However at some point prior to 1847 a pestilence swept through the region and reduced the number down to a single specimen, which forced the canons into crossing it with other breeds." []
is_a: DBO:0000011 ! Extinct

[Term]
id: DBO:0000270
name: Blue Paul Terrier
def: "No one seems to have full knowledge as to how the Blue Pauls were bred or from where they originally came. There was a story that Paul Jones, the pirate, brought them from abroad and landed some when he visited his native town of Kirkcudbright about 1770. The gypsies around the Kirkintilloch district kept Blue Pauls, which they fought for their own amusement. They were game to the death and could suffer much punishment. They were expert and tricky in their fighting tactics, which made them great favorites with those who indulged in this sport. They maintained that the breed originally came from the Galloway coast, which lends support to the Paul Jones legend. The first dogs to arrive in the United States with the English immigrants in the mid-19th century were the Blue Paul Terrier and the Bull and Terrier." []
is_a: DBO:0000011 ! Extinct

[Term]
id: DBO:0000271
name: Braque du Puy
def: "The Braque du Puy was an old breed of hunting dog in France, bred for hunting in the lowlands and known for being fast and flexible. The breed was created in Poitou in the 19th century by crossing other Braques with greyhound-type dogs. One story is that two brothers named du Puy crossed their Braque Francais dog with a Sloughi brought back from Africa by a French soldier.Colour of the Braque du Puy was white with orange or liver coloured marks, and was a medium to large size. The breed has now either died out or has died out in its original form, although the type may be reconstituted from other breeds and called Braque du Puy (or variants of the name) for the rare breed pet market in various parts of the world. The Braque du Puy was known for its refined, sight hound-like appearance and its skill as a hunting companion. The Braque du Puy was relatively popular at one point although it never achieved the numbers or fame of some other French Braques. The Braque du Puy is now generally considered extinct, although a few fanciers insist that the breed continues to exist in remote regions of Europe, and Braque du Puys are even occasionally offered for sale through rare breed dealers although these dogs are likely recreations rather than the original breed. The Braque du Puy is also known as the Braque Dupuy, the Dupuy Pointer, and the Du Puy Pointer." []
is_a: DBO:0000011 ! Extinct

[Term]
id: DBO:0000272
name: Bullenbeisser(German Bulldog)
def: "The Bullenbeisser became extinct by crossbreeding rather than by a decadence of the breed, as happened with the Old Time Bulldog, for instance. The size of the Bull Biters varied from about 40 to 70 cm by 1850; the smaller lived from what today is Netherlands and Belgium, and the bigger, in Germany. In the late 1870s, German breeders Roberth, Konig, and Hopner used the dog to create a new breed, today called the Boxer. Some 30 Bullenbeissers were already crossed by the Boxer Kennel Club of Germany at 1900 in with Bulldogs brought from the British Isles. The blood composition was 50/50 at that time, however, the German owners started crossing their dogs with all kinds of Bulldogs and Boxers, which produced an undistinguishable breed after World War II. One reason why such quantity of German blood was used to create the Boxer dog was the wish to eliminate the excessive white colour of the breed, and the necessity of producing thousands of dogs for one of the most popular breeds in the world." []
is_a: DBO:0000011 ! Extinct

[Term]
id: DBO:0000273
name: Chien-gris(Grey St. Louis Hound)
def: "The Chien-gris a.k.a. Gris de Saint-Louis (Grey St. Louis Hound) was a breed of dog, now extinct, which originated in Medieval times. Like the Chien de Saint-Hubert it was a scenthound, and formed part of the royal packs of France, which were composed, from about 1250 till 1470, exclusively of hounds of this type.[1] According to King Charles IX,(1550–1574) they supposedly were introduced to France through Saint Louis (i.e. King Louis IX, 1226–1270), who had encountered these hounds while a prisoner during the Crusades, and subsequently received some as a gift. Old writers on hunting liked to ascribe an ancient and remote origin to their hounds, and these were claimed to be originally from Tartary. They were large, and, even though they did not have such good noses, were preferred by the Kings to the St Huberts, which were said to be only of medium size.Jaques du Fouilloux,in the 16th century, says they were common, and describes them as 'gris' (grey) on the back with forequarters and legs tan or red, some having near black hair on the back. They were roughhaired, and were ancestors of the modern French rough-coated Griffon breeds.However the rough coats were not mentioned by Charles IX or du Fouilloux, and it has been suggested they were acquired later through interbreeding with indigenous French hounds.They were headstrong, wide casting hounds, inclined to change or overshoot, but determined in their pursuit of a quarry to the death. However, by the nineteenth century, like the St Hubert, they had become virtually impossible to find, because of mixed breeding and the effect of the Revolution on French hunting.George Turberville translated du Fouilloux' book on hunting into English, and used the term 'Dun hound' to translate 'Chien-gris'. We may presume he did not translate it literally as 'grey-hound' to avoid confusion. One finds the term 'dun-hound' in some subsequent writing in English, suggesting that the kind also existed in Britain, and it has been supposed that these 'dun-hounds' went into the make up of the Bloodhound, accounting for the 'badgering' of the hair in the saddles of some bloodhounds.However, Turberville did not make it very clear that his book was a translation, and it is highly possible that people mistakenly believed his work was about English hunting. Early references to the dun-hound may simply come from people relying, like Nicolas Cox, on Turberville,[8] [3] and it is quite possible that the dun hound was never a significant animal in British hunting." []
is_a: DBO:0000011 ! Extinct

[Term]
id: DBO:0000274
name: Cordoba Fighting Dog
def: "The Cordoba Fighting Dog originated in Córdoba, Argentina.It was noted for its willingness to fight to the death, and its high pain tolerance.[4] In addition, many members of this breed died in the dog fighting pits, contributing to the breed's extinction.The Cordoba was capable of hunting in a small pack of a male and female; otherwise it was likely to turn on its pack-mates.The Dogo Argentino is directly derived from this breed.In the 1920s, breeders developed the Dog by crossing the Cordoba Fighting Dog with other breeds such as the Great Dane, Great Pyrenees, Bulldog, Bull Terrier and Dogue de Bordeaux." []
is_a: DBO:0000011 ! Extinct

[Term]
id: DBO:0000275
name: Cumberland Shepherd Dog
def: "Cumberland sheepdogs were described in Dogs In Britain, A Description of All Native Breeds and Most Foreign Breeds in Britain by Clifford LB Hubbard, 1948." []
is_a: DBO:0000011 ! Extinct

[Term]
id: DBO:0000276
name: Dogo Cubano(Cuban Bloodhound)
def: "The Cuban Mastiff developed from several breeds of bulldogs, Mastiffs and cattle dogs becoming an ideal fighter and property guardian. It is possible that some specimens of this breed were brought to America where they were employed as watchdogs. They were also used as slave retrievers by the British during the Second Maroon War, by the French during the Saint-Domingue expedition, as well as the American in the southern States.The breed is considered extinct since the end of the 19th century, but there have been reports which state that although no pure Dogo Cubanos remain, the dogs used in today's fighting pits in Cuba are descendants of the crossbreed between Pit Bulls, Cordoba Fighting Dogs, Dogo Argentinos and the few pure Dogo Cubanos that were remaining by the beginning of the 20th century. The modern descendant of this rare dog breed is much larger and stronger than the original and resembles the American Pit Bull Terrier." []
is_a: DBO:0000011 ! Extinct

[Term]
id: DBO:0000277
name: English Water Spaniel
def: "In 1570, Dr John Caius described the Water Spaniel. It has been suggested that Shakespeare also knew the breed "for he mentions the `water rug' in Macbeth. "Furthermore, Shakespeare specifically mentions the breed in Act III Scene 1 of The Two Gentlemen of Verona when Launce says of his love, "She hath more qualities than a water-spaniel."The breed is mentioned specifically by name as early as 1802, in Sportsman's Cabinet, where it is described as having "hair long and naturally curled, not loose and shaggy"; the description accompanied an engraving of a liver and white curly coated spaniel. This shows that they pre-date the Irish Water Spaniel which was not developed as a breed until the 1830s. Unfortunately as the person credited with developing the Irish Water Spaniel, Justin McCarthy, left no written records, it is unknown if the English Water Spaniel was involved in its development.[2] During the first half of the 18th century, the English Water Spaniel was used for duck hunting in East Anglia.The Kennel Club initially had a class for "Water spaniels other than Irish" as no standard was specifically set up for the English Water Spaniel and the judging of this class was described as "chaos" by Hugh Dalziel in British Dogs: Their Varieties, History, Characteristics, Breeding, Management, And Exhibition.Writing in 1897, Dalziel said of the breed, "I do not believe the breed is lost, but that scattered throughout the country there are many specimens of the old English water spaniel, which it only requires that amount of encouragement to breeding which it is in the power of show committees to give to perpetuate the variety and improve its form."[4] Dalziel bemoaned the fact that while the Irish Water Spaniel continued, the English Water Spaniel was allowed to quietly be absorbed into other Spaniel breeds.The stud book of the Kennel Club also had a class for "Water spaniels other than Irish", however only fourteen dogs were registered in the twelve years up to 1903. This led some writers and judges of that time to believe that the English Water Spaniel was merely a cross of the Irish Water Spaniel as entrants in dogs shows in that same class do not match the description of the dog from earlier periods. Dogs awarded prizes as Water Spaniels during this period have been described as having "coats as flat as a Clumber, but with a bit of longish hair about the top of the skull."Writing in 1967, author John F. Gordon stated, "After two centuries of breeding it is now extinct. None have been seen for over thirty years."Descendant breeds of the English Water Spaniel are thought to include the American Water Spaniel, which was also developed using additional stock from the Irish Water Spaniel and the Flat Coated Retriever breeds. The Curly Coated Retriever is considered to have descended from the Poodle, the retrieving setter, the St. John's water dog and the English Water Spaniel.Records for the origin of the modern Field Spaniel are more precise and show that one of the four progenitor dogs used in creating the breed was an English Water Spaniel-Cocker Spaniel cross which was registered at the time as a Sussex Spaniel due to his liver colour." []
is_a: DBO:0000011 ! Extinct

[Term]
id: DBO:0000278
name: English White Terrier
def: "Small bred working terriers have existed in Great Britain since at least the late 18th Century. These dogs have always been quite variable in terms of size and shape, with dogs ranging in size from 10 to 15 inches, and with both drop ears and prick ears, smooth, broken, and rough coats.(Burns, 2005).With the rise of dog shows in the 1860s, breed fancy enthusiasts raced to name and "improve" every type of dog they could find, and terriers were at the very top of their list. From the long-extent white-bodied working terriers came the Fox terrier, the Jack Russell terrier, the Parson Russell terrier, and the Sealyham terrier.In the rush to create and claim new breeds, competing groups of dog breeders sometimes came up with different names for the same dog, and it was very common for entirely fictional breed histories to be cobbled up as part of a campaign to declare a new breed and create a bit of personal distinction for a dog's originator (to say nothing of sales).In the 1860s and 1870s, a small group of dog show enthusiasts tried to claim that prick-eared versions of white working terriers were an entirely different breed from those same dogs with dropped ears. The problems with this claim were legion, however. For one thing, prick and drop-eared dogs were often found in the same litter, while entirely white dogs had a propensity for deafness and were therefore nearly useless in the field. (Briggs, 1894).In 1894, Rawdon Briggs Lee wondered, in his book Modern Dogs, about the relatively recent origin of the "English white terrier" and noted that, "It has been surmised that the original English white terrier had been a fox terrier crossed with a white Italian greyhound" (i.e. a toy breed).Lee noted that at the London dogs shows where the breed first appeared in 1863–1864, the dogs were presented in two classes: "one being for dogs and bitches under six or seven pounds weight, as the case may be; the other for dogs and bitches over that standard."In 1894, about the time that English white terriers finally disappeared from the Kennel Club scene (it was always a pet and show dog, and never a working dog), Lee noted that "The most recent London-bred specimens I have seen have been comparative toys, under 10lb. in weight, and with a rounded skull, or so-called 'apple head," which so persists in making its appearance in lilliputian specimens of the dog – an effect of inbreeding."Though Lee included a club description of the dog claiming the dog could be found as heavy as 20lbs in weight, Lee (a noted Kennel Club judge and Kennel Editor of The Field sport hunting magazine) took the trouble to note that "As a matter of fact, I do not ever remember seeing a really so-called pure English white terrier up to 20lbs, the maximum allowed by the club."Lee describes the English white terrier as "the most fragile and delicate of all our terriers," noting that "he is not a sportsman's companion," but that he "makes a nice house dog" but "requires a considerable amount of cuddling and care."Lee notes that at some of the early dog shows "some of the specimens were shaped more like an Italian greyhound than as a terrier" and that the dog "is particularly subject to total or partial deafness."Though the dog still existed as a breed in 1894, Briggs could see the writing on the wall and did not bemoan the possible extinction of this show-ring failure: "While regretting extremely the decay of the White English Terrier, I am afraid they must bow to the inevitable, and give place to dogs better suited to the wants and conveniences of the present day than they unfortunately are."" []
is_a: DBO:0000011 ! Extinct

[Term]
id: DBO:0000279
name: Hare Indian Dog
def: "It is thought by one writer that the breed originated from a cross between native Tahltan bear dogs and dogs brought to the North American continent by Viking explorers, as it bears strong similarities to Icelandic breeds in appearance and behavior. Sir J. Richardson of Edinburgh, on the other hand, who studied the breed in the 1820s, in their original form before being diluted by crossings with other breeds, could detect no decided difference in form between this breed and a coyote, and surmised that it was a domesticated version of the wild animal. He wrote, "The Hare Indian or Mackenzie River Dog bears the same relation to the prairie wolf [coyote] as the Esquimeaux Dog [Malamute] does to the great grey wolf."The breed seemed to be kept exclusively by the Hare Indians and other neighboring tribes, such as the Bear, Mountain, Dogrib, Cree, Slavey and Chippewa tribes living in the Northeastern Territories of Canada and the United States around the Great Bear Lake, Southwest to Lake Winnipeg and Lake Superior and West to the Mackenzie River.[1] They were valued by the Indians as coursorial hunters, and they subsisted almost entirely on the produce of each hunt. Although not large enough to pose a danger to the moose and reindeer they hunted, their small size and broad feet allowed them to pursue large ungulates in deep snow, keeping them at bay until the hunters arrived.It was too small to be used as a beast of burden.[2] It was the general belief among the Indians that the dog's origin was connected to the Arctic fox. When first examined by European biologists, the Hare Indian dog was found to be almost identical to the coyote in build (save for the former's smaller skull) and fur length. The first Hare Indian dogs to be taken to Europe were a pair presented to the Zoological Society of London, after Sir John Richardson's and John Franklin's Coppermine Expedition of 1819–1822. Though originally spread over most of the northern regions of North America, the breed fell into decline after the introduction of firearms made its hunting abilities unnecessary. It gradually intermingled with other breeds such as the Newfoundland dog, the Canadian Eskimo dog and mongrels." []
is_a: DBO:0000011 ! Extinct

[Term]
id: DBO:0000280
name: Hawaiian Poi Dog
def: "The original Hawaiian poi dog were descended from the Polynesian dogs brought to the Hawaiian Islands by the Polynesian people. Referred as the ʻīlio in the Hawaiian language, the modern name of this breed is derived from poi, a Hawaiian staple food made from kalo or taro root. Poi was used to fatten the dogs for use as food because meat was too valuable to be used as dog food. Since the Hawaiian Islands did not have large land mammals other than feral hogs, Poi dogs were not needed for hunting. The dogs were never deliberately bred to a standard, but human and natural selection still came into play.European explorers like Captain Cook encountered pot-bellied, short-legged poi dogs that freely associated with hogs in the village. The dogs had very short hair that could come in any color, but brown poi dogs were regarded as distinct enough to warrant a specific name. The dogs also had peculiarly flattened heads. The latter trait is sometimes ascribed to the diet of the dogs in some unspecified way. Considering that poi does not require chewing, the dogs might have lost the need to maintain strong temporalis muscles; a reduced temporal fossa will cause a dog's head to appear flattened.[1] Poi dogs were considered rather dim-witted and sluggish – any good hunting dog with acute senses would neither make a good poi dog, nor be particularly useful on the islands – however, the dogs were strong-willed and not easily commanded.The poi dog was a two-purpose breed – used for food and as a lucky charm. Unsuited for anything else, the breed declined to extinction as the native religion was abandoned and eating dog meat became unfashionable. Feral dogs of European settlers interbred with the poi dogs, and by the early 20th century at latest, the breed disappeared as a distinct entity." []
is_a: DBO:0000011 ! Extinct

[Term]
id: DBO:0000281
name: Kunming Wolfdog
def: "Most of the exact dog breeds used in the gene pool for the Kunming wolfdogs is ambiguous due to the lack of proper pedigrees and the fact that a majority of them were crossbreeds although the German Shepherd and some wolfdog crosses are known to play a huge part in the breed's origin. The Kunming wolfdog was created in the early 1950s to meet the need for military dogs in Yunnan.A group of ten shepherd type dogs mixed with unknown breeds were brought to Kunming from a military K9 training program in Beijing in 1953. These ten dogs were insufficient for the immediate need, and so fifty suitable household dogs from Kunming were recruited as well as forty similar dogs from the city of Guiyang in Guizhou province (like the first ten, the exact breeds of these dogs are unknown other than that they were crossbreeds). After training, the best twenty of these ninety dogs were then selected. Ten wolfdogs bred in Beijing, twenty 'civil dogs' plus an additional ten 'shepherd dogs' imported from East Germany were added to the pool from which the Kunming Dog was developed. The Chinese Public Security Bureau officially recognized the Kunming Dog as a breed in 1988.Kunming Dogs are used by the Chinese military and police, and have also found their way into use as civilian watchdogs and guard dogs." []
is_a: DBO:0000011 ! Extinct

[Term]
id: DBO:0000282
name: Kuri
def: "Kurī is the Māori language name for the Polynesian dog. It was introduced to New Zealand by Māori during their migrations from East Polynesia sometime around 1280 AD. It was used by Māori as a food source.In addition, they used the skins and fur to make dog-skin cloaks (Kahu kurī),[2] belts, decorating weapons,and poi.The kurī became extinct in New Zealand some time after the arrival of European settlers. The remains of the last known specimens, a female and her pup, are now in the collection of the Museum of New Zealand Te Papa Tongarewa.According to Māori tradition, the demigod Māui transformed his brother-in-law Irawaru into the first dog." []
is_a: DBO:0000011 ! Extinct

[Term]
id: DBO:0000283
name: Miniature Shar Pei
def: "This breed goes back to around 200 BC in China where it was a cross of relatives to the chow chow, mastiff, terrier, and bulldog. Over the years this breed became larger as the mastiff influence began to come out.What many people do not know is that the Miniature actually represents a more accurate build of the breed's true dimensions. Until Shar Pei became AKC recognized, and the larger standard was adopted, those breeding what are now known as Miniature Shar Pei were actually breeding the more original size. This was recently discovered through the finding of the gene responsible for the miniature size.Before this many thought that the smaller sized dogs were unhealthy or considered to be mistakes. Today Miniature Shar Pei breeders believe that this breed is special unto itself and worthy of approval by the American Kennel Club." []
is_a: DBO:0000011 ! Extinct

[Term]
id: DBO:0000284
name: Molossus
def: "This ancient extinct breed of dog is considered to be the ancestor (in rivalry with the Alaunt, the dog of the Alans) of today's Mastiff-type dogs and of many other modern breeds.Mastiff-type dogs are often referred to as Molossus dogs or Molossers. It is one of the best-known breeds of antiquity; however, its function and physical characteristics are debated. This large ancient breed was, along with the Tibetan Mastiff, an important ancestor of modern breeds such as the English Mastiff, St. Bernard, Great Pyrenees, Rottweiler, Great Dane, Newfoundland, Greater Swiss Mountain Dog, and Bernese Mountain Dog and its most direct relative, the Neapolitan Mastiff.Dogs were used by the Epirotan tribes in war, and were undoubtedly used much earlier in history. The Roman Empire, starting with Marcus Aurelius, also used dogs in combat. The Romans trained the Molossian dog (or canis molossus) specifically for battle, often coating them in protective spiked metal collars and mail armor, arranging them into attack formations.Some scholars contend the Molossus was used by the Ancient Greeks for fighting.Described as having a wide, short muzzle and a heavy dewlap (similar to modern Mastiff breeds), the Molossus was used to fight tigers, lions, elephants, and men in battle. A Roman copy of a sculpture of a guard dog (known as the Jennings Dog) on display at the British Museum, is generally considered to represent a Molossus.Others argue it was primarily a lightweight dog used for hunting and herding — with physical characteristics more akin to Greyhounds or possibly the American Pit Bull Terrier.Most scholars agree the Molossus originated with the Molossis people in the mountainous regions of ancient Epirus (part of modern Albania and Greece). The Molossians were renowned for their vicious hounds, used by Molossian shepherds in the mountains of Epirus[6] to guard their flocks. The poet Grattius, a contemporary of Ovid, writes "...when serious work has come, when bravery must be shown, and the impetuous War-god calls in the utmost hazard, then you could not but admire the renowned Molossians so much."The breed was native to ancient Epirus (present day Albania and Greece) and the Balkan region. It later spread to Italy, around the Mediterranean and across Europe. Virgil says the Ancient Greeks and Romans used the heavier Molossian dogs for hunting (canis venaticus), to guard the home, and watch over livestock (canis pastoralis). "Never, with them on guard," says Virgil, "need you fear for your stalls a midnight thief, or onslaught of wolves, or Iberian brigands at your back." Aristotle mentions them in The History of Animals, praising their bravery and physical superiority.The breed's name was used to name the bat Molossus and, in turn, the family Molossidae." []
is_a: DBO:0000011 ! Extinct

[Term]
id: DBO:0000285
name: Moscow Water Dog
def: "The Moscow Water Dog, also known as the Moscow Diver, Moscow Retriever or Moskovsky Vodolaz, is a little-known dog breed derived from the Newfoundland, Caucasian Shepherd Dog and East European Shepherd. It is now extinct, but was used in the development of the Black Russian Terrier. The Moscow Water Dog was produced only by the Red Star Kennels, the state operated organization chartered to provide working dogs for the armed services.After World War II, there were very few working dogs in the Soviet Union as many had been killed during the war. Some were imported but there were not enough to establish a dedicated breeding programme for a specific breed. The Central Military School of Working Dogs (the Red Star Kennels), under the command of Colonel G. P. Medvedev began working on developing a number of their own specialised breeds by crossing the available stock. A few breeds were established including the Moscow Newfoundland, a cross of German Shepherd Dog and Newfoundland; the Moscow Great Dane, using German Shepherd and Great Dane; the Brudasty Hound, which was an Airedale Terrier and Russian Hound mix; the Moscow Watchdog, a combination of St. Bernard and Caucasian Shepherd Dog; and the Moscow Water Dog. The most successful breed to come out of the programme was the Black Russian Terrier, which gained international recognition in 1984; it derived from a combination of 14 different breeds including the Moscow Water Dog in the later stages of its development.Moscow Water Dogs were bred in Krasnaya Zvezda, Belarus, by interbreeding Newfoundland males with East European Shepherd and Caucasian Shepherd Dog females, and by mating the offspring with each other. They were developed as a water rescue/lifesaving dog, but according to O. Krasnovskaya, "That was not a good idea as [they] were not willing to save drowning people, but mostly were looking to bite them so this breed was never developed"." []
is_a: DBO:0000011 ! Extinct

[Term]
id: DBO:0000286
name: Norfolk Spaniel
def: "The Norfolk Spaniel was believed to have come about from a cross of spaniels with the Black and Tan Terrier, which was cultivated by an unspecified Duke of Norfolk." []
is_a: DBO:0000011 ! Extinct

[Term]
id: DBO:0000287
name: North Country Beagle
def: "The origins of the North Country Beagle are equally unclear. Most writers suggest that it was developed from the Talbot, whose origins are also uncertain, but which some have claimed originated in Normandy. The Talbot was a predominantly white, slow, deep-throated, scent hound. At some point the Talbots were crossed with Greyhounds to give them an extra turn of speed, but they remained comparatively slow dogs that relied more on their nose than speed in the chase." []
is_a: DBO:0000011 ! Extinct

[Term]
id: DBO:0000288
name: Paisley Terrier
def: "In 1894, it was speculated that Paisley Terrier, possibly bred by Glasgow enthusiasts selecting Skye Terriers, was primarily a pet despite its rat-catching abilities. The breed, valued for its blue and tan coat, became a popular showdog. Although initially seen as a fancier's dog, by 1903, it was acknowledged as a Skye Terrier variant. The Kennel Club recognized it in 1888, considering it a Skye Terrier variety, despite separate classes in 1887." []
is_a: DBO:0000011 ! Extinct
synonym: "Silky" EXACT[]

[Term]
id: DBO:0000289
name: Rastreador Brasileiro
def: "nan" []
is_a: DBO:0000011 ! Extinct

[Term]
id: DBO:0000290
name: Russian Tracker
def: "nan" []
is_a: DBO:0000011 ! Extinct

[Term]
id: DBO:0000291
name: Seskar Seal Dog
def: "A Spitz-type seal-hunting dog was known in the Baltic Sea already during the Stone Age. In Finland, these dogs spread to the areas of Saaristomeri, Suomenlahti, Ahvenanmaa and parts of the Gulf of Bothnia. Dogs were used for searching nest caves and breathing holes of seals until the 1950s, but soon after this they died out - mainly because they were no longer needed in their original work.[3] The breed is named after the isle of Seskar." []
is_a: DBO:0000011 ! Extinct
synonym: "Seiskari" EXACT[]

[Term]
id: DBO:0000292
name: Southern Hound
def: "nan" []
is_a: DBO:0000011 ! Extinct

[Term]
id: DBO:0000293
name: St. John's Water Dog
def: "The St. John's water dog was the ancestor of the modern retrievers, including the Flat Coated Retriever, Curly Coated Retriever, the Chesapeake Bay Retriever, the Golden Retriever, and the Labrador Retriever. The St. John's dog was also an ancestor to the large and gentle Newfoundland dog, probably through breeding with Mastiffs brought to the island by the generations of Portuguese fishermen who had been fishing offshore since the 15th century.During the 19th and early 20th centuries, St. John's dogs were exported from Newfoundland to England. These dogs were crossbred with other dogs to create the retrievers." []
is_a: DBO:0000011 ! Extinct

[Term]
id: DBO:0000294
name: Tahltan Bear Dog
def: "Raised by the Tahltan people to hunt bear, the Tahltan Bear Dog was a mighty power in a small package. Before a hunt, the dogs were ceremonially bled by stabbing them in the hindquarters with the fibula bone of a fox or wolf. The morning of the hunt, two dogs were carried in a sack over the hunter's shoulder until fresh bear tracks were sighted. Upon release, these little dogs moved lightly over the crust of snow while the bear was slowed down by the deep drifts. Their fox-like staccato yaps harassed the bear into submission or confused it until the hunter could come close enough for a kill. To prepare for a foray against big cats, a claw from a dead lynx was used to ceremonially mark the dog's face.The Tahltan Bear Dog had the courage to face a bear, but was friendly and gentle with smaller animals and with humans. They lived in the tent with the family, sharing bed and board.Descended from pariah-type dogs that had come with prehistoric migrations, the Tahltan Dogs were centralized in the remote mountainous areas of northwestern British Columbia and the Southern Yukon. Their usual diet was small bits of birds, meat and fish, and they flourished in the bitter cold. Outside their native environment, they succumbed to distemper, heat prostration and problems due to dietary changes. As white explorers came into the territory, bringing a variety of other dogs, the Tahltan Dog became diluted.There are no living descendants past 1960-70. Genetic references in the archeological record show no modern relationship of Tahltan dogs to any modern populations. No modern breeds have any known genetic relationship with extant dogs." []
is_a: DBO:0000011 ! Extinct
synonym: "Tahltan" EXACT[]

[Term]
id: DBO:0000295
name: Talbot
def: "The talbot breed's claimed origins in Normandy and its association with William the Conqueror lack evidence. While mentioned as individual hounds in Medieval times, it wasn't recognized as a distinct breed until the 17th century, described as large, slow 'talbot-like' hounds. The breed persisted until the late 18th century, disappearing along with related breeds like the Northern and Southern Hound." []
is_a: DBO:0000011 ! Extinct

[Term]
id: DBO:0000296
name: Toy Bulldog
def: "nan" []
is_a: DBO:0000011 ! Extinct

[Term]
id: DBO:0000297
name: Toy Trawler Spaniel
def: "The specific origin of the breed is unknown but in 1919 was thought to have been descended from the originally curly-coated King Charles Spaniel and the old-fashioned curly-coated Sussex Spaniel.[1] Its original purpose may have been as a sporting dog, but it became more frequently used as a toy dog. By 1907, the breed was more popular in Europe than in the UK, especially in the Netherlands and Italy.There is a preserved specimen at the Natural History Museum at Tring. Named Robin, it was bred by Lady Wentworth and was born in 1911. It died in 1920 when the breed was said to be "nearly extinct". Lady Wentworth wrote about using Toy Trawler Spaniels to re-breed the original King Charles Spaniel in her book "Toy Dogs and Their Ancestors Including the History And Management of Toy Spaniels, Pekingese, Japanese and Pomeranians" published under the name of the "Hon. Mrs Neville Lytton" in 1911." []
is_a: DBO:0000011 ! Extinct

[Term]
id: DBO:0000298
name: Tweed Water Spaniel
def: "The village of Norham, Northumberland, just south of the River Tweed was noted as being "long famous" for a breed of water spaniel of which were "invariably brown".In 1816, Richard Lawrence wrote of the origins of the Tweed Water Spaniel, "Along rocky shores and dreadful declivities beyond the junction of the Tweed with the sea of Berwick, water dogs have derived an addition of strength, from the introduction of a cross with the Newfoundland dog, which has rendered them completely adequate to the arduous difficulties and diurnal perils in which they are systematically engaged."[3] Although the quote refers specifically to the Newfoundland breed, it is actually more likely to mean the now extinct breed of the St. John's water dog which was sometimes referred to by its homeland's location of Newfoundland and Labrador.Stanley O'Neil, an expert in Flat-coated Retrievers, wrote of the Tweed Water Spaniel in a letter during the late 19th century, "Further up the coast, probably Alnmouth, I saw men netting for salmon. With them was a dog with a wavy or curly coat. It was a tawny colour but, wet and spumy, it was difficult to see the exact colour, or how much was due to bleach and salt. Whilst my elders discussed the fishing I asked these Northumberland salmon net men whether their dog was a Water-Dog or a Curly, airing my knowledge. They told me he was a Tweed Water Spaniel. This was a new one on me. I had a nasty suspicion my leg was being pulled. This dog looked like a brown Water Dog to me, certainly retrieverish, and not at all spanielly. I asked if he came from a trawler, and was told it came from Berwick."Linda P. Case, of the University of Illinois, speculated the Tweed Water Spaniel was so named because it was developed on the estate of Lord Tweedmouth, and in fact was simply the original name for a breed of dog that later became the Golden Retriever.However, this theory is against the documented evidence, as the early development of the Golden Retriever was fully documented and listed the three Tweed Water Spaniels involved specifically by breed" []
is_a: DBO:0000011 ! Extinct

[Term]
id: DBO:0000299
name: Saint Bernard
def: "In the year 1050, at a snowy pass within the Alps, a monk named Bernard of Menthon (later canonized) established a hospice to aid pilgrims journeying to Rome. At 8,000 feet above sea level, with drifts as high as 40 feet, crossing the pass was treacherous. Over several centuries the hospice monks developed powerful working dogs able to locate and rescue luckless travelers buried by drifts and avalanches. Myth busted: Dogs of the Great St. Bernard Pass didn't carry casks of brandy around their necks." []
is_a: DBO:0000004 ! Working Group

[Term]
id: DBO:0000300
name: American Leopard Hound
def: "American Leopard Hounds are one of the oldest of the tree dog breeds in the Americas. The exact origins of the American Leopard are unknown. Those who have researched the history of the breed maintain that dogs brought to the New World by Spanish conquistadors played a role in their evolution.;Opinions vary as to what other dogs were involved in the breed's development. Some researchers suggest that the conquistadors' dogs were mixed with dogs native to Mexico and were later brought to the United States by settlers, where they continued to develop into the breed known today. Others contend that the breed's entire development took place within the southern United States from a mixture of Spanish, French, English, Irish, and Scottish hound and herding breeds.;By the early 18th century, American Leopard Hounds had become established in eastern North Carolina. From there, it made its way west into Tennessee and Kentucky and, later, south into Texas and Oklahoma.;During the early 20th century, the breed began to decline and was allowed to cross with other breeds, so much so that by the 1950s, few purebred examples could be found. Realizing this, three individuals, J. Richard McDuffie, Leroy E. Smith, and A.W. Carter, began to independently search for any examples of the breed. Meeting in 1960, these three men established the American Leopard Cur Breeders Association (ALCBA) to establish and promote the breed.;The American Leopard Hound has been bred as an all-purpose tree dog. They are unique in the tree dog world because of their intense desire to please their master; no breed is more easily trained. They are also unsurpassed in their ability to fight and hold game at bay without getting hurt. They stay in close on the quarry, but have the unique ability to "duck and dodge" to avoid injury. In the home, they are extremely affectionate and protective with children.2012;The American Leopard Hound was recorded in the Foundation Stock Service." []
is_a: DBO:0000010 ! Foundation Stock Service
synonym: "Griffon" EXACT[]
synonym: "Griff" EXACT[]
synonym: "Bruss" EXACT[]

[Term]
id: DBO:0000301
name: Brussels Griffon
def: "1910;The Brussels Griffon was officially recognized by the AKC" []
is_a: DBO:0000010 ! Foundation Stock Service
synonym: "Crested" EXACT[]
synonym: "Puff" EXACT[]
synonym: "Curtis" EXACT[]

[Term]
id: DBO:0000302
name: Chinese Crested
def: "1991;The Chinese Crested was officially recognized by the AKC." []
is_a: DBO:0000006 ! Companion and Toy Group
synonym: "Cockers" EXACT[]

[Term]
id: DBO:0000303
name: Cocker Spaniel
def: "1878;The Cocker Spaniel was offcially recognized by the AKC." []
is_a: DBO:0000002 ! Sporting Group

[Term]
id: DBO:0000304
name: Collie
def: "1885;The Collie was officially recognized by the AKC." []
is_a: DBO:0000008 ! Herding Group

[Term]
id: DBO:0000305
name: English Toy Spaniel
def: "1886;The English Toy Spaniel was officially recognized by the AKC" []
is_a: DBO:0000006 ! Companion and Toy Group

[Term]
id: DBO:0000306
name: English Mastiff
def: "1885;The Mastiff was officially recognized by the AKC." []
is_a: DBO:0000004 ! Working Group

[Term]
id: DBO:0000307
name: Nederlandse Kooikerhondje(Nederlandse Little Cager Dog)
def: "The origins of the Nederlandse Kooikerhondje (Dutch Decoy Dog) can be found as far back as the 1500s. It is said that the decoy dog owned by William of Orange saved his life by warning him of the Spanish attack. Many of the Dutch Masters painted family portraits that depict a small decoy-type dog. It is believed that this dog originated from the spaniel.Between 1626 and 1679, the breed was developed to work in the duck decoys. The hunter would train his dog to lure the ducks into a "trap." While the hunter would hide behind a series of "blinds," he would signal his dog to walk along side the canal. Upon another signal from the hunter, the dog would then disappear behind the blinds, only to come out again at a different location. The quiet, playful dog would "lure" the ducks deeper into the canal or "pipe" with this weaving behavior. The white bushy tail of the dog would attract the curiosity of the ducks, which would continue swimming deeper into the "pipe." Eventually the dog would lure the ducks all the way into the catching pen. The hunter would then take the captured ducks to market. By the 19th century, the duck decoy business had decreased significantly, though there are still a few working decoys found in Holland today. They are mostly used for research and tagging of ducks.By the 1930s this lovely breed was nearly extinct. Through the devotion of M.C.S. Baroness van Hardenbroek, the breed was rediscovered. She began her breeding program in 1939. The Dutch Kennel Club officially recognized the Nederlandse Kooikerhondje in 1966." []
is_a: DBO:0000002 ! Sporting Group

[Term]
id: DBO:0000308
name: Poodle(Standard)
def: "nan" []
is_a: DBO:0000007 ! Non-Sporting Group

[Term]
id: DBO:0000309
name: Poodle(Mininature)
def: "nan" []
is_a: DBO:0000007 ! Non-Sporting Group

[Term]
id: DBO:0000310
name: Portuguese Podengo
def: "The probable origin of the Portuguese Podengo is with the primitive, multi-purpose hunting dogs obtained, used and distributed by Phoenician traders during the circumnavigation of Africa in 600 BC and reaching Portugal in the 700s BC. This is evidenced by artifacts found under the Lisbon Cathedral. The Podengos were developed into different sizes in Portugal due to their functionality, the largest being the Podengo Grande, which was developed for deer and wild boar hunting. It will exhaust and detain large game and await the hunter's gun. The Podengo Medio, being slightly smaller, was used for rabbit hunting. Due to Portugal's relative isolation at the western edge of Europe, unlike the other two sizes, the Medio evolved to its present form without much influence from other breeds and, as a result, has the most strongly established and homogeneous type and greatest genetic stability of the three sizes. The Medio embodies the authentic type of the Portuguese Podengo.;The Portuguese Podengo is one of ten National Dogs of Portugal and has the honor of being the symbol of the Portuguese Kennel Club (the Clube Portugues de Canicultura or CPC). The Club do Podengo Portugues (CPP) is the national breed club in Portugal. Ironically for this breed, which in the Medio and Pequeno sizes has evolved for the past 2,000 years as a dog of the people, the efforts to save and improve the breed over the past 100 years have included many members of Portugal's upper classes, who saw in this and the other nine indigenous breeds an essential element of the national patrimony.;The first purebred Portuguese Podengos came to the United States in the 1990s and now reside in more than forty-five states. The first documented Portuguese Podengos of any size in America were the wirehaired Portuguese Podengo Medios imported in August, 1994.2004;First recognized by the AKC in 2004." []
is_a: DBO:0000009 ! Miscellaneous

[Term]
id: DBO:0000311
name: Portuguese Podengo Pequeno
def: "2013;The Portuguese Podengo Pequeno  was officially recognized by the AKC" []
is_a: DBO:0000003 ! Hound Group

[Term]
id: DBO:0000312
name: Small Munsterlander Pointer
def: "Prior to the 19th century hunting was the privilege of landed upper class who had the financial resources to breed, train and manage large kennels of specialty dogs. The middle class arose in the 1800's and gained access to hunting through land ownership. These hunters wanted companion dogs with diverse hunting skills. Within Germany, however, aristocratic hunters strove to preserve the traditional hunting ethic with its profound respect for game animals.This ethic necessitated versatile hunting dogs skilled in recovering lost and wounded game, and not just in locating or retrieving downed birds or animals. Thus, the concept of the versatile hunting dog, Jagdgebrauchhund, became popular at the beginning of the 20th century, and several versatile hunting breeds were founded at that time.In the Münsterland area of Germany (roughly east of Holland to Hannover and north through the moors) a search began about 1870 for a versatile long haired Wachtelhund (quail dog) breed. Hunting dogs in this part of Germany were already noted for their staunch point, their enormous search drive and their outstanding nose, capable of both air scenting and tracking.Several hunting aristocrats as well the famous poet, Hermann Löns, and his brother, Edmund, were among the leaders of this group. On March 17, 1912, a group of 68 formed the Verein für Kleine Münsterländer Vorstehhunde (Heidewachtel)-the Small Munsterlander Pointer (Heath quail) Club--in the town of Osnabrück, north of the city of Münster.Small Munsterlanders at that time were mostly plated, with many color variations (except black). Braunschimmel (roan) dogs first appeared in the mid 1920's, probably through one or more crossings with German Shorthairs. Liver and white are now the predominant colors for Small Munsterlanders, although glints of auburn are often apparent in their coats, particularly around the ears." []
is_a: DBO:0000009 ! Miscellaneous
synonym: "Xolo" EXACT[]
synonym: "Xolito" EXACT[]

[Term]
id: DBO:0000313
name: Xoloitzcuintli(Mexican Hairless Dog)
def: "2010;The Xoloitzcuintli was officially recognized by the AKC.;Their origin dates far back in history. The meat of the Xoloitzcuintle or Xoloitzcuintli in Nahuatl language, Xoloitzcuintle in Spanish was considered a delicacy in pre Hispanic Mexico, eaten by the indigenous Mexicans in special ceremonies as a ritual to their beliefs and was regarded as a representative of the god "Xolotl", from which its name obviously originates.  Its task was to guide the souls of the dead to their eternal destination. Therefore the dog became scarce, reaching a point of near extinction. The Federación Canófila Mexicana (Mexican Kennel Club) rescued this native breed and has used the Xoloitzcuintle on its logo since 1940. The hairless variety of the breed is also known by the name "perro pelón mexicano" (Mexican Hairless Dog). The coated variety was known by the natives as "itzcuintle"." []
is_a: DBO:0000007 ! Non-Sporting Group

[Term]
id: DBO:0000314
name: American Bulldog
def: "Bulldogs in England were originally working dogs that drove and caught cattle and guarded their masters' property. The breed's strength, courage, and familiarity with livestock led to its popularity in the brutal sport of bull baiting. When this sport was outlawed in England, the original type of Bulldog disappeared from Britain and was replaced with the shorter, stockier, less athletic dog we now know as the English Bulldog. ; The original Bulldog, however, was preserved by working class immigrants who brought their working dogs with them to the American South. Small farmers and ranchers used this all-around working dog for many tasks. By the end of World War II, however, the breed was almost extinct. Mr. John D. Johnson, a returning war veteran, decided to resurrect this breed. Along with Alan Scott and several other breeders, Johnson began carefully to breed American Bulldogs, keeping careful records and always with an eye for maintaining the breed's health and working abilities. ; Because of the many different types of work this breed can do, several distinct lines evolved, each emphasizing the traits needed to do a specific job. The best known lines are usually referred to as the Johnson and Scott types. ; The Scott dogs, commonly referred to as 'standard', are more of a performance style, athletic dog, sleeker in appearance than the bully dogs, with less bone, longer muzzles, more moderate stop and a less extreme undershot bite. Today, however, many American Bulldogs have crosses to two or more of the original lines and are considered to be hybrid in type, with characteristics of more than one of the original lines of bulldogs. ; The Johnson dogs, commonly referred to as 'bully', are bulkier in body, heavier in bone, with larger heads that have more stop, a shorter muzzle and a more pronounced undershot bite. They generally have more muscle mass as well. ; The modern American Bulldog continues to serve as an all-purpose working dog; a fearless and steady guard dog; and a loyal family companion. ; The American Bulldog was recognized by the United Kennel Club on January 1, 1999." []
is_a: DBO:0000010 ! Foundation Stock Service

[Term]
id: DBO:0000315
name: American Pit Bull Terrier
def: "Sometime during the nineteenth century, dog fanciers in England, Ireland and Scotland began to experiment with crosses between Bulldogs and Terriers, looking for a dog that combined the gameness of the terrier with the strength and athleticism of the Bulldog. The result was a dog that embodied all of the virtues attributed to great warriors; strength, indomitable courage, and gentleness with loved ones. Immigrants brought these bull-and-terrier crosses to the United States. The American Pit Bull Terrier's many talents did not go unnoticed by farmers and ranchers who used their APBTs as catch dogs for semi-wild cattle and hogs, to hunt, to drive livestock, and as family companions. Today, the American Pit Bull Terrier continues to demonstrate its versatility, competing successfully in Obedience, Rally Obedience, Tracking, Agility, Lure Coursing, Dock Jumping and Weight Pulls, as well as Conformation. ; The United Kennel Club was the first registry to recognize the American Pit Bull Terrier. UKC founder C. Z. Bennett assigned UKC registration number 1 to his own APBT, Bennett's Ring, in 1898." []
is_a: DBO:0000005 ! Terrier Group
synonym: "Farmer Dog" EXACT[]

[Term]
id: DBO:0000316
name: Australian Kelpie
def: "Kelpie' was the name bestowed on a pup from the mating of two black-and-tan Smooth Collies imported to Australia. She was eventually mated to a pup produced by two more imported sheepdogs, and a female pup from that litter went to C.B.K. King of Wollongough Station, New South Wales. This pup was dubbed 'Kelpie,' Gaelic for 'water sprite,' after her mother. An impressive win in the first Australian sheepdog trials in 1872 made her famous. Her offspring were known as Kelpie pups, which gave rise to the breed name." []
is_a: DBO:0000010 ! Foundation Stock Service

[Term]
id: DBO:0000317
name: Large Munsterlander
def: "The Large Munsterlander is descended from the parti-colored bird and hawking dogs used in the Middle Ages. It was developed in Germany, and was divided into a distinct breed, separate from the other German Longhaired pointing breeds, in 1919. The breed was recognized by the United Kennel Club in 2006." []
is_a: DBO:0000010 ! Foundation Stock Service

[Term]
id: DBO:0000318
name: Toy Poodle
def: "The Toy Poodle is the smallest descendent of the Poodle brigade that began as a breed of continental water dogs known in Germany and Russia since the 16th century. Though there are references to tiny Poodles in the breed literature, no attempt was made to develop a true Toy until after the Miniature had been given separate breed status in England in 1910. With the success of the Miniature, breeders couldn't resist the challenge to reduce this popular breed even more. Presumably it was done by mating the smallest Miniatures though it has been suggested that some other Toy breeds may have been used to hasten the progress. By the late 1940s and early 1950s, the breed had become so well established that it was granted separate breed status. The Toy Poodle is identical to both the Standard and Miniature except for size." []
is_a: DBO:0000006 ! Companion and Toy Group
synonym: "Stumpy" EXACT[]
synonym: "Stumpy[-]Tail" EXACT[]
synonym: "Heeler" EXACT[]

[Term]
id: DBO:0000319
name: Australian Stumpy Tail Cattle Dog
def: "The Stumpy Tail shares its early history with the Australian Cattle Dog – both were developed by 19th-century Australian farmers to protect, herd and drive livestock over long distances. The difference between them is that unlike the Australian Cattle Dog, the Stumpy Tail has no Kelpie blood." []
is_a: DBO:0000008 ! Herding Group
synonym: "Bleu Picard" EXACT[]

[Term]
id: DBO:0000320
name: Blue Picardy Spaniel
def: "A long-legged spaniel with setter characteristics, the Blue Picardy is a versatile sporting dog with a reputation for locating and retrieving game under the most adverse conditions. The first French spaniels had their beginnings in the Middle East when French knights travelled to the Holy Land accompanied by their pointers and hounds, which interbred with Arabian Greyhounds. Over time, the spaniels of France separated into regional types. Picardie, France, was a paradise for hunters of waterfowl and, at the end of the 19th century, British hunters and dogs came to hunt in the area's marshes and moors. When the British quarantine was put into effect, many English hunters boarded their setters on Picardie farms. Consequently, Picard spaniels were crossed with blue belton English and Gordon Setters and the Blue Picardy Spaniel was the result." []
is_a: DBO:0000002 ! Sporting Group

[Term]
id: DBO:0000321
name: Braque d'Auvergne
def: "The Auvergne pointer is a very ancient breed, present in the Cantal region for more than two centuries. Descending from a multi-pointer common source, derivation has been made by a selection to which the Knights of Malta might have participated. Created by and for hunters, it has a strong identity reinforced by its coat." []
is_a: DBO:0000002 ! Sporting Group
is_a: DBO:0000008 ! Herding Group

[Term]
id: DBO:0000322
name: Canadian Eskimo Dog
def: "A dog of the Canadian Arctic, the Canadian Eskimo Dog is called 'Qimmiq' by the Inuit. The breed proved popular with Arctic explorers and earned a reputation as a sled dog that could pull the heaviest loads over the greatest distances on the least amount of food. As snowmobiles gained favour, the number of Eskimo Dogs declined dramatically. In the 1970s, a project headed by William Carpenter and funded by The Canadian Kennel Club, the Canada Council and private individuals saved the breed from extinction." []
is_a: DBO:0000004 ! Working Group

[Term]
id: DBO:0000323
name: Long-Coated Chihuahua
def: "Up until its time of development as a pure breed in the United States, the origin of the long-coated version of the Chihuahua is identical to that of the short-coated variety. The long, soft coat is thought to have been achieved by crossbreeding the Short Coat with other Toy breeds. The Papillon, Pomeranian, Pekingese and Yorkshire Terrier have been suggested as possible crosses." []
is_a: DBO:0000006 ! Companion and Toy Group

[Term]
id: DBO:0000324
name: Short-Coated Chihuahua
def: "The origin of the world's smallest dog is one of the world's biggest puzzles. Some say its ancestors lived in Egypt some 3,000 years ago and point to mummified remains of small dogs. Others state that the Chihuahua was domesticated in Mexico prior to 1519 and played a part in religious ceremonies. They believe the dogs were taken back to Spain after the Spanish Conquest and then spread throughout Europe and the Mediterranean. And finally, it has also been theorized that the breed was brought to Mexico by Chinese traders. Take your choice. Whatever the breed's beginnings, it was discovered late in the 19th century by American tourists in Mexico who took some of these dogs back to the States and it is from these that the breed developed. They were named for the Mexican state, Chihuahua, where they were found." []
is_a: DBO:0000006 ! Companion and Toy Group
synonym: "BRAQUE FRANÇAIS - TYPE GASCOGNE" EXACT[]

[Term]
id: DBO:0000325
name: Gascogne Braque Francais(French Pointing Dog-Gascogne Tye)
def: "The Braque Français (French Pointer) is believed to have derived from dogs used to point game in the Mediterranean region as early as the 1300s. When these brown-and-white pointers spread throughout Europe, they evolved into regional types. In France, each type took on the name of its province." []
is_a: DBO:0000002 ! Sporting Group

[Term]
id: DBO:0000326
name: Greenland Dog
def: "Since the Inuit people of Canada's Arctic were known to have emigrated from Greenland many centuries ago bringing their sled dogs with them, it's possible this hardy polar Spitz breed is the forerunner of our native Canadian Eskimo Dog. The relationship to other northern Spitz breeds – such as the Alaskan Malamute, Siberian Husky and Canadian Eskimo – is unmistakable. Used primarily as sled dogs in the Scandinavian countries, Greenland Dogs were also put to work by the native people as hunting dog whose superior sense of smell was used to track down seal breathing holes." []
is_a: DBO:0000004 ! Working Group

[Term]
id: DBO:0000327
name: Japanese Spitz
def: "Although white Spitz-like dogs were known in Japan from about 1900, the breed didn't become established until after World War II. Bearing a remarkable physical resemblance to the Samoyed, it is considerably smaller in size. The British Kennel Club recognized the breed in 1977, establishing it in that country as well. It is still rather rare on this continent." []
is_a: DBO:0000007 ! Non-Sporting Group

[Term]
id: DBO:0000328
name: Kleiner Munsterlander Vorstehund
def: "The setter-like Small Münsterländer hails from the town of Munster in Westphalia, Germany, where it was created in the early 1900s by crossing old-time Spanish spaniels with German pointers and other continental gun dogs. Herr Edmund Loens is credited with having discovered the breed, appreciating its hunting qualities and working toward the formation of a parent club in 1912. A tireless and enthusiastic hunter, even in the worst of weather, the breed is confident on point with excellent retrieving skills." []
is_a: DBO:0000002 ! Sporting Group

[Term]
id: DBO:0000329
name: Miniature American Eskimo Dog
def: "nan" []
is_a: DBO:0000007 ! Non-Sporting Group

[Term]
id: DBO:0000330
name: Miniature Long-Haired Dachshund
def: "Like his larger relative, the Standard, this smaller version of the Long-haired Dachshund was developed in Germany to rid farms of destructive pests. The Standard Dachsies were bred to hunt down badgers but the quarry for the Mini Dachshunds was the rabbit that destroyed the crops. The little dogs must be small enough to slip down rabbit holes and in their native land, they are classified according to girth, not weight. They can measure no more than 13.75 in (35 cm) around the body." []
is_a: DBO:0000003 ! Hound Group

[Term]
id: DBO:0000331
name: Miniature Smooth-Haired Dachshund
def: "Like his larger relative, the Standard, this smaller version of the Long-haired Dachshund was developed in Germany to rid farms of destructive pests. The Standard Dachsies were bred to hunt down badgers but the quarry for the Mini Dachshunds was the rabbit that destroyed the crops. The little dogs must be small enough to slip down rabbit holes and in their native land, they are classified according to girth, not weight. They can measure no more than 13.75 in (35 cm) around the body." []
is_a: DBO:0000003 ! Hound Group

[Term]
id: DBO:0000332
name: Miniature Wire-Haired Dachshund
def: "The Mini Wire has grown tremendously in popularity in North America in recent years, partly due to the bubbling personality of the breed and to its appealing appearance, combining Dachsie charm and terrier-like looks. Like the Mini Smooth and Mini Long-haired, the Mini Wire was bred to control rabbits that destroyed German crops." []
is_a: DBO:0000003 ! Hound Group

[Term]
id: DBO:0000333
name: Miniature Xoloitzcuintli(Miniature Mexican Hairless Dog)
def: "One of the world's oldest and rarest breeds, the Xoloitzcuintli (pronounced show-low-eets-queent-lee) can be called the first dog of the Americas. The name is derived from the Aztec god Xolotl and the Aztec word for dog Itzcuintli. Highly prized for their curative and mystical powers, the Xolo held a place of special religious significance for many ancient cultures. The Miniature and Standard Xolos were first registered in Mexico in 1955." []
is_a: DBO:0000007 ! Non-Sporting Group

[Term]
id: DBO:0000334
name: Smooth-Haired Vizsla
def: "The Vizsla, or Hungarian Pointer, may be of ancient lineage or it may be a product of the last century, depending on which dog historian one chooses to believe. Those who favour the theory of the breed's antiquity cite stone etchings from the 10th century and a 14th-century manuscript on falconry illustrated with a picture of a dog resembling the Vizsla. Whatever its history, the Vizsla was perfectly suited to perform the duties of a pointer and retriever in the open plains of Hungary. Two world wars dealt harshly with the breed and only action by concerned breeders in Hungary and those countries to which the breed had been exported kept it from extinction. The breed has rebounded and is now considered the national dog of Hungary." []
is_a: DBO:0000002 ! Sporting Group

[Term]
id: DBO:0000335
name: Standard American Eskimo Dog
def: "A member of the ancient Spitz family of dogs that harks back to prehistoric times, the Eskie is a handsome snow-white dog that is believed to have descended from European spitz breeds. The predecessors may have been the white German Spitz, Keeshond, Pomeranian and the Volpino Italiano (Italian Spitz). The breed first appeared on this continent during the 19th century and arrived here in the company of German immigrants. Eventually, the breed became known as the American Spitz. First registered with the United Kennel Club (in the U.S.) in 1913, the Eskie underwent a name change to American Eskimo Dog in 1917. The American Kennel Club recognized the breed in 1995." []
is_a: DBO:0000007 ! Non-Sporting Group

[Term]
id: DBO:0000336
name: Standard Long-Haired Dachshund
def: "Developed from the original Standard Smooth Dachshund, the Long-haired was created by crossing the breed with the Field Spaniel. This variety has all the attributes of the Smooth but the outline is enhanced by soft feathering on the throat, ears, underbody and tail, giving it an unmistakable elegance." []
is_a: DBO:0000003 ! Hound Group

[Term]
id: DBO:0000337
name: Standard Smooth-Haired Dachshund
def: "The granddaddy of all Dachshunds was developed in Germany and used to hunt badger and fox since the 16th century. The name means "badger dog" in German and if ever a dog deserved to be designated as a terrier, it was the Dachshund since it was used to go to ground (dig) after the badger. But when Queen Victoria's consort Prince Albert introduced the breed to Britain, "hund" was translated to mean "hound" and the breed has been classified as a hound ever since. Tenacious and keen-nosed, Dachshunds work in packs and are strong and fearless when sent underground to rout out the ferocious badger." []
is_a: DBO:0000003 ! Hound Group

[Term]
id: DBO:0000338
name: Standard Wire-Haired Dachshund
def: "The granddaddy of all Dachshunds was developed in Germany and used to hunt badger and fox since the 16th century. The name means "badger dog" in German and if ever a dog deserved to be designated as a terrier, it was the Dachshund since it was used to go to ground (dig) after the badger. But when Queen Victoria's consort Prince Albert introduced the breed to Britain, "hund" was translated to mean "hound" and the breed has been classified as a hound ever since. Tenacious and keen-nosed, Dachshunds work in packs and are strong and fearless when sent underground to rout out the ferocious badger." []
is_a: DBO:0000003 ! Hound Group

[Term]
id: DBO:0000339
name: Standard Xoloitzcuintli(Standard Mexican Hairless Dog)
def: "One of the world's oldest and rarest breeds, the Xoloitzcuintli (pronounced show-low-eets-queent-lee) can be called the first dog of the Americas. Clay and ceramic effigies of Xolo's date back over 3000 years and have been discovered in the tombs of the Toltec, Mayan, Zapoteca and Colima Indians. The Miniature and Standard Xolos were first registered in Mexico in 1955. Before then, the breed was kept alive by secluded Indian tribes in remote parts of Mexico and South America. The Countess Lascelle De Premio Real was primarily responsible for the re-establishment of this almost extinct native breed, which is now designated as the official dog of Mexico." []
is_a: DBO:0000007 ! Non-Sporting Group

[Term]
id: DBO:0000340
name: Polish Tatra Shepherd Dog
def: "Developed to herd and guard flocks in the Carpathian Mountains in southern Poland, the Tatra's history follows that of similar dogs from Czechoslovakia, Hungary and Rumania, all of which trace back to flock guardians brought west by the Phoenicians. The Polish Kennel Club restored the breed after it was brought to the brink of extinction during World War II." []
is_a: DBO:0000008 ! Herding Group

[Term]
id: DBO:0000341
name: Toy American Eskimo Dog
def: "The American Eskimo can probably trace its beginnings back to the Peat Bog Dog of the New Stone Age, some 6,000 years ago. Remains of this, one of the first dog breeds, have been found in Scandinavian countries as well as Russia, Finland and Germany. All Spitz breeds share certain characteristics. The American Eskimo may have come down through the German Spitz and the white Pomeranian. During the 19th century, many of these small, white dogs were found in German communities in the U.S., having arrived with their immigrant owners. Eventually they came to be known as the American Spitz and were popular in the trick dog acts of travelling circuses. The breed was first registered with the United Kennel Club (in the U.S.) in 1913 and in 1917, the name of American Eskimo was adopted. In 1995, the American Kennel Club recognized the breed with three separate size divisions." []
is_a: DBO:0000006 ! Companion and Toy Group

[Term]
id: DBO:0000342
name: Toy Xoloitzcuintli(Toy Mexican Hairless Dog)
def: "One of several hairless breeds found throughout the world is the Xoloitzcuintli (pronounced show-low-eats-queent-lee). The name is derived from that of the Aztec Indian god Xolotl and Itzcuintli, the Aztec word for dog. Many folk tales surround the breed, one being that it has great curative powers. The breed is indeed hairless though some sport wisps on the skull, nape, tail tip and feet. There is also a coated variety, covered in a short, smooth, dense coat." []
is_a: DBO:0000006 ! Companion and Toy Group

[Term]
id: DBO:0000343
name: Alaskan Klee Kai
def: "The Alaskan Klee Kai was developed in Alaska by Linda Spurlin and her family, to be a companion-sized version of a type of dog referred to as the Alaskan Husky. From the early 70's through 1988, the Spurlins carefully selected dogs who met their high standards for appearance and soundness. In 1988, they made the Alaskan Klee Kai available to others. Mrs. Spurlin originally called her new breed the "Klee Kai", but in 1995 it was changed to "Alaskan Klee Kai". ; The Alaskan Klee Kai was recognized by the United Kennel Club January 1, 1997." []
is_a: DBO:0000004 ! Working Group

[Term]
id: DBO:0000344
name: Alpine Drachsbracke
def: "In the late 19th Century, the gamekeepers for Crown Prince Rudolf were using a hunting/shooting dog that bore a strong resemblance to the modern Alpine Drachsbracke. The breed was used as a tracking dog for wounded deer and a scenthound for hare and fox. In 1932 the breed was recognized in Austria, and in 1991 it was accepted as a Scenthound by FCI. ; The Alpine Drachsbracke was recognized by the United Kennel Club January 1, 1996." []
is_a: DBO:0000003 ! Hound Group

[Term]
id: DBO:0000345
name: Anglo-Francais de Petite Venerie
def: "Developed in France, most likely beginning during the 16th Century, the Anglo Francais de Petite Venerie was created by crossing English hounds with the French hounds. It was used as a scenthound for hunting small game. ; The Anglo Francais de Petite Venerie was recognized by the United Kennel Club January 1, 1996." []
is_a: DBO:0000003 ! Hound Group

[Term]
id: DBO:0000346
name: Ariegeois
def: "Developed in the French province of Ariege, from a series of matings between the Grand Bleu de Gascogne, Grand Gascon-Saintongeois and local Briquet hounds, the Ariegeois excels in hunting hare in the dry, rocky regions of its homeland. (Note; "Briquet" is often mistakenly translated as "Beagle", but actually does not denote any certain breed. Rather, the term is used to describe medium-sized hounds which are finer-boned, shorter-coupled and more compact than the larger "Grand" breeds.) ; The Ariegeois was recognized by the United Kennel Club on January 1, 1993." []
is_a: DBO:0000003 ! Hound Group
synonym: "Bracke (colloquially called Vieräugl)" EXACT[]

[Term]
id: DBO:0000347
name: Austrian Black and Tan Hound
def: "The Austrian Black and Tan Hound appears to be a true descendant of the ancient Celtic Hound. They are a universally popular hunting dog, prized for their ability to do heavy work on high mountains, as well as on flat country. ; The Austrian Black and Tan Hound was recognized by the United Kennel Club in 2006." []
is_a: DBO:0000003 ! Hound Group

[Term]
id: DBO:0000348
name: Austrian Pinscher
def: "The Austrian Pinscher descends from the ancient Austrian country pinschers that were still widespread in the second half of the 19th century and used as versatile farm dogs. Pure breeding of this breed began in 1921. ; The Austrian Pinscher was recognized by the United Kennel Club in 2006." []
is_a: DBO:0000005 ! Terrier Group
synonym: "BOSANSKI OSTRODLAKI GONIC-BARAK" EXACT[]

[Term]
id: DBO:0000349
name: Barak
def: "The Barak was registered with FCI in 1965 under the name of Illyrian Hound. In 1973 the name was changed to Bosnian Broken Haired Hound (or Bosnian Coarse Haired Hound), and the breed is called the Barak. ; The Barak was recognized by the United Kennel Club In 2006." []
is_a: DBO:0000003 ! Hound Group
synonym: "BAN" EXACT[]

[Term]
id: DBO:0000350
name: Basset Artesien Normand
def: "A group of serious French breeders formed a breed society to combine the Normand (from Normandy) and Artesien (from Artois) Bassets strains, merging them to develop the one breed that we have today. Although the breed has been streamlined from the original cumbersome, unwieldy dog, some people feel that this resulted in a lack of stamina and hound voice. No one can argue, however, that the resulting Basset Artesien Normand has a good temperament and is an energetic extrovert. The appealing nature of the breed makes them attractive to pet homes and families. Dedicated breeders strive to maintain the hunting instincts of the breed. ; The Basset Artesien Normand was recognized by the United Kennel Club on January 1, 1995." []
is_a: DBO:0000003 ! Hound Group

[Term]
id: DBO:0000351
name: Basset Bleu De Gascogne(Blue Gascony Basset)
def: "The Basset Bleu de Gascogne's historical rootstock is from the Grand Bleu de Gascogne, a Scenthound of ancient lineage. ; The existence of the Basset Bleu de Gascogne is supreme evidence of the antiquity of the parent breed and is, therefore, itself a very ancient and important breed when speaking of Basset varieties in general and Bleu de Gascogne hounds specifically. The Basset Bleu de Gascogne evolved directly from the Grand Bleu de Gascogne, shows certain signs of distinction, and reflects an aristocratic air shared with the parent breed. ; The Basset Bleu de Gascogne was recognized by the United Kennel Club in January 1991." []
is_a: DBO:0000003 ! Hound Group

[Term]
id: DBO:0000352
name: Bavarian Mountain Hound
def: "The Bavarian Mountain Hound is descended from the original hunting dogs that were called 'Bracken'. All Bracken have outstanding abilities for tracking and trailing. The Bavarian Mountain Hound was bred to be a lighter leash trailing scenthound that could be used in mountainous regions. They have been so successful that today they are the classic companion in the mountains of Bavaria for the professional hunter and gamekeeper. ; The Bavarian Mountain Hound was recognized by the United Kennel Club January 1, 1996." []
is_a: DBO:0000003 ! Hound Group

[Term]
id: DBO:0000353
name: Beagle Harrier
def: "Beagle Harriers were bred in France in the 19th Century. They were bred to hunt hare or deer in packs. They could be a mixture of the Beagle and the Harrier breeds, or they could be the mid-point between the two breeds, the truth is not really known. They were recognized by the FCI in 1974. The breed is very rare. ; The Beagle Harrier was recognized by the United Kennel Club January 1, 1996." []
is_a: DBO:0000003 ! Hound Group

[Term]
id: DBO:0000354
name: Billy
def: "The Billy originated in the 19th Century in Western Central France. They were created by combining a number of hound breeds which are now all extinct. They were, and still are, used to hunt roe deer and wild boar in packs. ; The Billy was recognized by the United Kennel Club January 1, 1996." []
is_a: DBO:0000003 ! Hound Group

[Term]
id: DBO:0000355
name: Black Mouth Cur
def: "The origin of the Black Mouth Cur is uncertain. Some writers have claimed that the breed originated in the mountains of Tennessee while others believe the breed originated in Mississippi. In any event, these dogs were widely used by early American settlers as all-round working dogs. As Americans moved west, the Black Mouth Curs moved with them, serving as a hunting dog and family guardian. ; The Black Mouth Cur was recognized by UKC on November 1, 1998." []
is_a: DBO:0000003 ! Hound Group

[Term]
id: DBO:0000356
name: Bouvier des Ardennes
def: "The Bouvier des Ardennes originated as a cattle drover in the Belgian Ardennes. Only the most hard and hardworking dogs from a very restricted population were retained and used to drive the herds, mostly cattle but also sometimes sheep, pigs and horses. They were also used to track deer and wild boar, and during the two World Wars they became poachers' dogs. During the 20th Century, the disappearance of farms in the Ardennes and the reduction in the herds of milking cattle greatly diminished the number of working dogs, including the Bouvier des Ardennes. ; Around 1985 a few survivors of this breed were discovered, and some breeders set out to produce dogs that adhered to the original standard of the breed which had been published in 1923. ; The Bouvier des Ardennes was recognized by the United Kennel Club July 1, 2006." []
is_a: DBO:0000008 ! Herding Group

[Term]
id: DBO:0000357
name: Braque de l'Ariege(Ariege Pointing Dog)
def: "A Continental pointing breed that is descended from the old French Braques, which were combined during the 19th Century with the orange and white Southern Braques to give them more lightness and activity. A few huntsmen from the Ariegeois region continued to use the breed, which saved them from extinction. In 1990 a team of breeders decided to devote themselves to the breed's survival. ; The Braque de l'Ariege was recognized by the United Kennel Club in 2006." []
is_a: DBO:0000003 ! Hound Group

[Term]
id: DBO:0000358
name: Braque Saint Germain(St. Germain Pointing Dog)
def: "A French pointing breed that was created around 1830 by crossing an English Pointer with a Continental Pointer. The breed was in great vogue until the beginning of the 20th Century; being the most shown pointing breed in the first French dog shows. ; The Braque Saint Germain was recognized by the United Kennel Club in 2006." []
is_a: DBO:0000003 ! Hound Group

[Term]
id: DBO:0000359
name: Briquet Griffon Vendeen
def: "Briquet means "medium sized dog" in French, and this is the only breed to retain that name. The Briquet Griffon Vendeen was bred down in size from the Grand Griffon Vendeen, beginning before the First World War. They are used as pack animals on roe deer, wild boar and also on small game. ; The Briquet Griffon Vendeen was recognized by the United Kennel Club January 1, 1996." []
is_a: DBO:0000003 ! Hound Group

[Term]
id: DBO:0000360
name: Ca de Bestiar (Majorca Shepherd Dog)
def: "The Ca de Bestiar originated in Spain. It is also known as the Majorca Shepherd Dog. ; The Ca de Bestiar was recognized by the United Kennel Club in 2006." []
is_a: DBO:0000008 ! Herding Group

[Term]
id: DBO:0000361
name: Catalonian Shepherd Dog
def: "The Catalonian Sheepdog is a flock driver that originated in the Catalonian Pyrenees Mountains. The breed is also used as a guardian. ; The Catalonian Sheepdog was recognized by the United Kennel Club July 1, 2006." []
is_a: DBO:0000008 ! Herding Group

[Term]
id: DBO:0000362
name: Cesky Fousek
def: "The Cesky Fousek (Bohemian Wire-Haired Pointing Griffon) was at one time the most widely kept pointing dog in the area of the modern day Czech and Slovakian Republics. During the First World War, the breed was nearly eradicated, but through carefully planned breedings it was brought back and today it is the second most popular of all hunting breeds in it's original home territory. ; The Cesky Fousek was recognized by the United Kennel Club January 1, 1996." []
is_a: DBO:0000003 ! Hound Group

[Term]
id: DBO:0000363
name: Chart Polski (Polish Greyhound)
def: "The Chart Polski is an ancient, short haired sighthound. Its presence in Poland has been attested to in literature since the 13th Century. The breed probably originated from the Asiatic sighthounds that were of Saluki type. The breed was historically used for hunting hare, fox, roe-deer, bustard and wolf. ; The Chart Polski was recognized by the United Kennel Club January 1, 1996." []
is_a: DBO:0000003 ! Hound Group

[Term]
id: DBO:0000364
name: Chien d'Artois(Artois Hound)
def: "Formerly named the Picard, the Chien d'Artois is an ancient French hunting breed that is widely used on deer, hare and wild boar. They generally hunt in a small pack of six to eight hounds. Following the Second World War, it was feared that the breed was one that had been lost, but in the early 1970's the breed was reconstructed in its homeland. ; The Chien d'Artois was recognized by the United Kennel Club in 2006." []
is_a: DBO:0000003 ! Hound Group

[Term]
id: DBO:0000365
name: Chien Francais Blanc et Noir(French White and Black Hound)
def: "The Chien Francais Blanc et Noir is a large pack scenthound developed for hunting large game. ; The Chien Francais Blanc et Noir was recognized by the United Kennel Club January 1, 1996." []
is_a: DBO:0000003 ! Hound Group

[Term]
id: DBO:0000366
name: Chien Francais Tricolore(French Tricolour Hound)
def: "The Chien Francais is a French breed developed to hunt big game. ; The Chien Francais Tricolore was recognized by the United Kennel Club January 1, 1996." []
is_a: DBO:0000003 ! Hound Group

[Term]
id: DBO:0000367
name: Ciobanesc Romanesc Carpatin(Carpathian Shepherd Dog)
def: "The Romanian Carpathian Shepherd Dog has been used for centuries by the Romanian shepherds in the Carpathian Mountains to defend the herds and guard the camps. Selection was based upon performance rather than breed type until the first breed standard was written in 1934. ; The Romanian Carpathian Shepherd Dog was recognized by the United Kennel Club July 1, 2006." []
is_a: DBO:0000008 ! Herding Group

[Term]
id: DBO:0000368
name: Ciobanesc Romanesc Mioritic(Romanian Mioritic Shepherd Dog)
def: "The Romanian Mioritic Shepherd Dog was developed in the Carpathian Mountains of Romania for use as a herd guard dog. The breed has many admirers in its native land. ; The Romanian Mioritic Shepherd Dog was recognized by the United Kennel Club July 1, 2006." []
is_a: DBO:0000008 ! Herding Group

[Term]
id: DBO:0000369
name: Croatian Shepherd Dog
def: "The Croatian Sheepdog (also known as the Hrvatski Ovcar) is a native breed that is descended from the dogs the Croats brought with them when the settled the land. It has been bred and used as a sheep and cattle herder in the plains of Slavonia for centuries. The earliest written document that has been found about the breed dates from the year 1374. ; The Croatian Sheepdog was recognized by the United Kennel Club July 1, 2006." []
is_a: DBO:0000008 ! Herding Group

[Term]
id: DBO:0000370
name: Deutsche Bracke(German Hound)
def: "From the many varieties of Bracken that originally existed, only one survived in Germany, the Westphalian Bracke. These were interbred with local Steinbracken, and one type evolved, which has been known since 1900 as the Deutsche Bracke, or German Bracke Hound. ; The Duetsche Bracke was recognized by the United Kennel Club January 1, 1996." []
is_a: DBO:0000003 ! Hound Group

[Term]
id: DBO:0000371
name: Dunker(Norwegian Hound)
def: "The Dunker originated in Norway. ; The Dunker was recognized by the United Kennel Club January 1, 1996." []
is_a: DBO:0000003 ! Hound Group

[Term]
id: DBO:0000372
name: English Shepherd
def: "According to legend, the English Shepherd is a combination of native dogs of the British Isles and the Roman sheep and cattle dog brought to the British Isles by Caesar when he invaded in 55 B.C. ; Romans used these dogs to herd the livestock brought along to feed the troops. As the livestock was depleted, surplus dogs were left along the way, and were used by local natives and interbred with existing types of dogs with similar herding talents to intensify those instincts. ; The English Shepherd was brought to the American colonies by some of the first settlers and followed the development of the United States from east to west. This multi-purpose breed was highly prized as it was used to herd valuable livestock and to protect the isolated homesteads. ; The United Kennel Club is the original registrar of the English Shepherd and has recognized them since 1927." []
is_a: DBO:0000008 ! Herding Group

[Term]
id: DBO:0000373
name: Epagneul Pont-Audemer(Pont-Audemer Spaniel)
def: "Descended from the Picardy spaniel and possibly the Barbet and the Poodle, the Epagneul de Pont-Audemer has always been a rare breed, and so few existed after the Second World War that it was necessary to breed them with Irish Water Spaniels to keep the breed alive. A water specialist, the breed is also used to point and flush. ; The Epagneul de Pont-Audemer was recognized by the United Kennel Club January 1, 1996." []
is_a: DBO:0000002 ! Sporting Group
is_a: DBO:0000006 ! Companion and Toy Group

[Term]
id: DBO:0000374
name: Epagneul Picard(Picardy Spaniel)
def: "The Picardy Spaniel is descended from the old French spaniels that were crossed with English Setters and Gordon Setters. In 1921 the Picard Spaniel and Blue Picardy Spaniel Club was formed. ; The Epagneul Picard was recognized by the United Kennel Club January 1, 1996." []
is_a: DBO:0000003 ! Hound Group

[Term]
id: DBO:0000375
name: Finnish Hound
def: "At the beginning of the 19th Century, there were many dogs in Finland that resembled the European hounds. Those dogs were crossed with the Finnish country dogs, and the resultant dogs were the beginning of the Finnish Hound. The first standard was written in 1932. They are used as a fox and hare hunter. ; The Finnish Hound was recognized by the United Kennel Club January 1, 1996." []
is_a: DBO:0000003 ! Hound Group

[Term]
id: DBO:0000376
name: Francais Blanc et Orange
def: "The Francais Blanc et Orange was recognized by the United Kennel Club January 20, 1996." []
is_a: DBO:0000003 ! Hound Group

[Term]
id: DBO:0000377
name: Grand Bleu de Gascogne(Great Gascony Blue)
def: "The Grand Bleu de Gascogne is a Scenthound of ancient lineage, eminently French. They are descended from the original scenting dogs of Gaul and the Phoenician hound trade, and are one of the two types from which most modern hound breeds developed. The Grand is probably the closest, of the four Bleu de Gascogne breeds, to the ancient hounds in size and build. Gascony Province, the specific area of their root-stock and development, is located on the southwestern coast of France. ; The Grand Bleu de Gascogne is first and fundamentally a hunting/working breed, a trail hound "par excellence," which has retained the extreme physical and hunting characteristics of its ancient stem. Every point of the Grand Bleu de Gascogne is for a purpose relevant to preserving the breed and its uniqueness. Judges are asked by the sponsoring breed club to keep this fact in mind when evaluating the merits of an individual hound. ; The Grand Bleu de Gascogne was recognized by the United Kennel Club in January 1991." []
is_a: DBO:0000003 ! Hound Group

[Term]
id: DBO:0000378
name: Grand Gascon-Saintongeois
def: "This breed was created by Baron Joseph de Carayon-LaTour of Chateau Virelade, who came into possession of the only specimens of the Saintongeois hound to survive the French Revolution (one female and two males). (The Saintongeois is now considered an extinct breed.) These he mated with Grand Bleu de Gascognes from the kennel of the Baron de Ruble. The first generation offspring were of such magnificent quality that the two men continued to breed in such manner, and the resulting descendants were given the name "Grand Gascon-Saintongeois". ; The Grand Gascon-Saintongeois was recognized by the United Kennel Club on January 1, 1993." []
is_a: DBO:0000003 ! Hound Group

[Term]
id: DBO:0000379
name: Grand Griffon Vendeen
def: "In the early 16th Century, a breed known as the Grand Vendeen existed. It was a short coated Vendeen bred down from 'the King's white hounds'. When the Grand Vendeen was crossed with several of the other Griffon breeds, the Grand Griffon Vendeen was born. It was used on large game such as stag, roe deer, wild boar and fox, generally in a pack. ; The Grand Griffon Vendeen was recognized by the United Kennel Club January 1, 1996." []
is_a: DBO:0000003 ! Hound Group

[Term]
id: DBO:0000380
name: Great Anglo-Francais Tricolor Hound
def: "The Great Anglo-Francais Tricolor Hound (Grand Anglo-Francais Tricolore) originated in France. ; The Great Anglo-Francais Tricolor Hound was recognized by the United Kennel Club in 2006." []
is_a: DBO:0000003 ! Hound Group

[Term]
id: DBO:0000381
name: Great Anglo-Francais White and Black Hound
def: "The Great Anglo-Francais White and Black Hound (Grand Anglo-Francais Blanc et Noir) originated in France. ; The Great Anglo-Francais White and Black Hound was recognized by the United Kennel Club January 20, 1996." []
is_a: DBO:0000003 ! Hound Group

[Term]
id: DBO:0000382
name: Great Anglo-Francais White and Orange Hound
def: "The Great Anglo-Francais White and Orange Hound (Grand Anglo-Francais Blanc et Orange) was recognized by the United Kennel Club in 2006." []
is_a: DBO:0000003 ! Hound Group

[Term]
id: DBO:0000383
name: Griffon Bleu de Gascogne(Blue Gascony Griffon)
def: "The Griffon Bleu de Gascogne is a breed of very ancient Pyrenean origin. It is the result of crossing a medium sized Gascony Blue with a Griffon. After having nearly become extinct, the breed is experiencing a considerable revival. It is used to hunt hare and wild boar. ; The Griffon Bleu de Gascogne was recognized by the United Kennel Club January 1, 1991." []
is_a: DBO:0000003 ! Hound Group

[Term]
id: DBO:0000384
name: Griffon Fauve de Bretagne(Fawn Brittany Griffon)
def: "The Griffon Fauve de Bretagne is one of the oldest of the French scenthound breeds. There was a pack in existence in the 14th Century. They were used to hunt wolves until those disappeared, then on hare, roe deer, fox and wild boar. ; The Griffon Fauve de Bretagne was recognized by the United Kennel Club January 1, 1996." []
is_a: DBO:0000003 ! Hound Group

[Term]
id: DBO:0000385
name: Griffon Nivernais
def: "Rough-coated hounds, used by farmers and shepherds to control wolves and wild boars, have been bred in the highlands of Central France for many centuries. After the French Revolution, a renewed interest in this type of dog precipitated the development of the Griffon Nivernais, originally known as the Griffon-Vendeen-Nivernais. They are known as wild boar hunters without compare. ; The Griffon Nivernais was recognized by the United Kennel Club on January 1, 1995." []
is_a: DBO:0000003 ! Hound Group

[Term]
id: DBO:0000386
name: Haldenstover (Halden Hound)
def: "The Haldenstover originated in Norway. ; The Haldenstover was recognized by the United Kennel Club in 2006.The Halden is one of three Norwegian hare hound breeds, and is the smallest in size. Bred for scent hunting, the breed is believed to have been developed through crossing local Norwegian scenthounds with scenthounds from Sweden, Germany, and England. It was first developed in the early 1900s, and the breed standard was established in the 1950s. The Halden is relatively rare, seldom seen outside Norway." []
is_a: DBO:0000003 ! Hound Group

[Term]
id: DBO:0000387
name: Hanoverian Hound
def: "The Hanoverian Scenthound originated in Germany. It has developed nearly unchanged from the so-called Liam Hound of the early middle Ages. With the invention of firearms, dogs were needed to search for wounded game. The Hanoverian Hunting Estate in the kingdom of Hannover developed this hound and their breeding has been strictly with regard to their working ability. They are used exclusively as specialists for tracking cloven hoofed game. ; The Hanoverian was recognized by the United Kennel Club January 1, 1996." []
is_a: DBO:0000003 ! Hound Group

[Term]
id: DBO:0000388
name: Hellenic Hound
def: "The Hellenic Hound is a medium sized scenthound that originated in Greece.; The Hellenic Hound was recognized by the United Kennel Club in 2006." []
is_a: DBO:0000003 ! Hound Group

[Term]
id: DBO:0000389
name: Hungarian Greyhound (Magyar Agar)
def: "The Hungarian Greyhound is an original hunting breed, dating back to the time when the Magyars conquered Hungary. The breed was used for coursing game by sight, though it also has a good nose, and also for racing, at which it excels at long distances. ; The Hungarian Greyhound was recognized by the United Kennel Club in 2006." []
is_a: DBO:0000003 ! Hound Group

[Term]
id: DBO:0000390
name: Hygen Hound
def: "The Hygen Hound is a medium sized scenthound breed that originated in Norway. ; The Hygen Hound was recognized by the United Kennel Club in 2006." []
is_a: DBO:0000003 ! Hound Group

[Term]
id: DBO:0000391
name: Istrian Short-Haired Hound
def: "An ancient breed that originated in Croatia, the Istrian Short-Haired Hound is frequently encountered in Istria and neighboring regions, where it is highly prized for fox and hare hunting. ; The Istrian Short-Haired Hound was recognized by the United Kennel Club in 2006." []
is_a: DBO:0000003 ! Hound Group

[Term]
id: DBO:0000392
name: Italian Hound
def: "The origins of the Italian Hound go back to antiquity. They are certainly descended from the ancient hounds of Egypt that were used for hunting. They have been maintained practically without change through the centuries. ; The Italian Hound was recognized by the United Kennel Club in 2006." []
is_a: DBO:0000003 ! Hound Group
synonym: "JRT" EXACT[]
synonym: "Jack" EXACT[]

[Term]
id: DBO:0000393
name: Jack Russell Terrier
def: "The Reverend John Russell was a 19th century parson with a passion for fox hunting, for which he developed a well-known strain of fox hunting terriers. From this strain was developed the Parson Russell Terrier and the Jack Russell Terrier. The Jack Russell Terrier was a smaller, longer-bodied, shorter-legged dog that was used almost exclusively to hunt vermin and bolt rabbits. For years, Jack Russell Terrier breeders referred to these dogs as "puddin' dogs" or "puds," and some-times just "shorties." ; In England, Ireland, and Australia, the longer-legged square dog is known as the Parson Russell Terrier while the lower, longer dog is called the Jack Russell Terrier. ; UKC recognized the short-legged dogs as Russell Terriers on January 1, 2001; and on January 1, 2009 revised the breed name to Jack Russell Terrier." []
is_a: DBO:0000005 ! Terrier Group
synonym: "Kobe Terrier" EXACT[]
synonym: "Mikado Terrier" EXACT[]
synonym: "Oyuki (snowy) Terrier" EXACT[]

[Term]
id: DBO:0000394
name: Japanese Terrier
def: "In the 17th Century, smooth-haired Fox Terriers were imported to Japan from the Netherlands. These dogs were bred with small pointers and native type dogs, and the Japanese Terrier eventually emerged, with type being set in the breed around 1930. The breed is kept mainly as a lap dog. ; The Japanese Terrier was recognized by the United Kennel Club in 2006." []
is_a: DBO:0000005 ! Terrier Group
synonym: "Kooiker" EXACT[]

[Term]
id: DBO:0000395
name: Kooikerhondje(Little Cager Dog)
def: "The Kooikerhondje was widely used in the 17th and 18th century by Dutch hunters to lure ducks into traps. Thereafter, however, the breed declined until Baroness van Hardenbroek van Ammerstol single-handedly rescued the breed. In the middle of World War II and during the occupation of her country by the enemy, she gave a photo of a Kooikerhondje and a lock of Kooiker hair to a peddler and instructed him to tell her when he saw any dogs that resembled the photo. The female he found for her became the foundation for the revived breed. The Kooikerhondje was recognized by the Dutch Kennel Club in 1971. ; The Kooikerhondje was recognized by United Kennel Club in 1996." []
is_a: DBO:0000003 ! Hound Group

[Term]
id: DBO:0000396
name: Mi-Ki
def: "The Mi-Ki (pronounced Mee-Kee) originated in the 1980s by Mikki Mackin, who resided in Wisconsin, and who was trying to create a new smaller, long-haired breed with a calm, quiet nature. Prior to starting the Mi-Ki, she was a Shih Tzu breeder. She added mixed and purebred Papillion, Maltese, Yorkshire Terriers and Japanese Chin to her Shih Tzu to start the original breed. Unfortunately, she did not keep accurate records, so the degree of mixture or exact combination remains unknown. Connie Faye Abel, Annette Jurkiewicz and Cindy Jurkiewicz founded the International Mi-Ki Registry, Inc., in March of 1999 with the idea to further develop the original Mi-Ki obtained from Mikki Mackin, (aka Maureen Westberg or Van Wormer) from 1996-1999 into a recognized purebred companion breed, while preserving its health, exceptional temperament and Gremlin look, with its long, silky, non-shed coat. ; The Mi-Ki was recognized by the United Kennel Club on January 1, 2016" []
is_a: DBO:0000006 ! Companion and Toy Group

[Term]
id: DBO:0000397
name: Montenegrin Mountain Hound
def: "This version of the Balkan hound was developed in the Republic of Montenegro. The first standard dates to 1924. ; The Montenegrin Mountain Hound was recognized by the United Kennel Club in 2008." []
is_a: DBO:0000003 ! Hound Group

[Term]
id: DBO:0000398
name: Mountain Feist
def: "The word "feist" is an ancient one referring to a small, often noisy dog. Like the Cur breeds, the Feist breeds were developed in the rural South by breeders who needed low-maintenance dogs to hunt small game and to eliminate vermin, Feist were often the result of crosses between hunting hounds and terriers. Todays Mountain Feist is the result of generations of breeding for performance and is still primarily used to hunt squirrel, although they are also used to hunt raccoon, rabbits and more. ; The Mountain Feist was recognized by the United Kennel Club on February 1, 2015." []
is_a: DBO:0000005 ! Terrier Group

[Term]
id: DBO:0000399
name: Patterdale Terrier
def: "The Patterdale Terrier is descended mainly from the black, smooth-coated Fell Terrier which was developed in the harsh environment of Northern England. The Fell Terriers were used to control vermin that were predatory on sheep. They were bred to bolt the quarry out of the den or to dispatch it if it chose to fight. Its characteristics result in an extremely game, 'tough as nails' dog. ; The Patterdale Terrier was recognized by the United Kennel Club on January 1, 1995." []
is_a: DBO:0000005 ! Terrier Group

[Term]
id: DBO:0000400
name: Petit Bleu de Gascogne(Small Blue Gascony)
def: "The Petit Bleu de Gascogne is a Scenthound of ancient lineage, eminently French, showing signs of certain distinction. They are descended from the original scenting dogs of Gaul and the Phoenician hound trade; specifically they developed from the Grand Bleu de Gascogne. They are generally used to hunt hare. Gascony Province, the area of their development, is located on the southwestern coast of France. Every point of the Petit Bleu de Gascogne is for a purpose relevant to preserving the breed and its uniqueness. Judges are asked by the sponsoring breed club to keep this fact in mind when evaluating the merits of the individual hound. ; The Petit Bleu de Gascogne was recognized by the United Kennel Club in January 1991." []
is_a: DBO:0000003 ! Hound Group

[Term]
id: DBO:0000401
name: Petit Gascon-Saintongeois
def: "In essence, the Petit Gascon-Saintongeois is a "reduction" of the Grand Gascon-Saintongeois, individuals of which were undoubtedly mated with Airegeois and other local Briquet hounds to achieve their present size and type. At this time, the Petit Gascon-Saintongeois is one of the most rare hound breeds in France. ; The Petit Gascon-Saintongeois was recognized by the United Kennel Club on January 1, 1993." []
is_a: DBO:0000003 ! Hound Group

[Term]
id: DBO:0000402
name: Podenco Canario(Canary Islands Hound)
def: "An ancient breed of Egyptian origin, its ancestors were probably brought to the Canary Islands by the Phoenicians, the Greeks, the Carthaginians and the Egyptians themselves. The breed dates back about seven thousand years. It hunts rabbits and ferrets by sight, scent and sound and has extraordinary survival skills. ; The Podenco Canario was recognized by the United Kennel Club July 1, 2006." []
is_a: DBO:0000003 ! Hound Group

[Term]
id: DBO:0000403
name: Poitevin
def: "The Poitevin is a large scenthound that originated in France. ; The Poitevin was recognized by the United Kennel Club January 1, 1996." []
is_a: DBO:0000003 ! Hound Group

[Term]
id: DBO:0000404
name: Posavaz Hound
def: "The Posavaz is an ancient hound breed indigenous to Croatia. Its origins are lost in the mists of time, but books bear witness to its antiquity. It is a good scenthound with excellent stamina, used to hunt hare and fox. It can also be used as a trailing leash hound. ; The Posavaz was recognized by the United Kennel Club in 2006." []
is_a: DBO:0000003 ! Hound Group

[Term]
id: DBO:0000405
name: Saarloosewolfdog
def: "In 1932, a gentleman named Leendert Saarloos crossed a male German Shepherd Dog with a female European wolf. He then bred the offspring back to their sire, and with that pool of dogs he created the Saarloosewolfdog. The breed was not created for any specific working purpose, but rather to be a hardy, self reliant companion and housedog. ; The Saarloosewolfdog was recognized by the United Kennel Club July 1, 2006." []
is_a: DBO:0000008 ! Herding Group

[Term]
id: DBO:0000406
name: Schiller Hound
def: "The Schiller Hound originated in Sweden. It is descended from Swiss hounds, along with an infusion of British hound blood, mostly Harrier. It was recognized by the Swedish KC in 1907. The breed is used for hunting fox and hare. It is not a pack hound. ; The Schiller Hound was recognized by the United Kennel Club in 2006." []
is_a: DBO:0000003 ! Hound Group

[Term]
id: DBO:0000407
name: Serbian Hound
def: "The Serbian Hound was originally known as the Balkan Scenthound. Because the breed was most widespread in Serbia, in 1996 the name was changed to Serbian Hound. ; The Serbian Hound was recognized by the United Kennel Club in 2006." []
is_a: DBO:0000003 ! Hound Group

[Term]
id: DBO:0000408
name: Serbian Tricolor Hound
def: "The Serbian Tricolor Hound has the same origins as the other Balkan scenthounds. It was originally considered a variety of the Serbian Hound, but was given its own breed status in 1946, though except for color the standards are nearly identical. ; The Serbian Tricolor Hound was recognized by the United Kennel Club in 2006." []
is_a: DBO:0000003 ! Hound Group

[Term]
id: DBO:0000409
name: Silken Windhound
def: "After considering options since 1975, a Borzoi breeder, Francie Stull, determined that a smaller hound with wonderful temperament, long coat, all-around good health, with the poise and sporting abilities of the larger sighthounds, would be an ideal second breed for her kennel. ; In the early 1980's, an advertisement appeared in The Sighthound magazine for a Borzoi litter. Included was the famous Borzoi bitch, American, English Champion Stillwater Virginia Reel. This beautiful bitch caught the eye of Kristull Kennel and the purchase of a pick puppy from her next litter was negotiated.; When bred to Stillwater White Lightning, Stillwater Virginia Reel produced a blue brindle puppy, Stillwater Kristull Peacock. Peacock had the structure, personality and coat that formed the basis for the Silken Windhound when she was bred to Windsprite Autumnal Xenon. ; With more than two hundred champion Borzoi in the record books, Kristull's Silken Windhound foundation stock combined dogs from some of the best show and coursing Borzoi lines, a multi-generational line of small Whippet-based lurchers, and Whippets from both show and coursing lines. ; The result of the breeding program was a magnificent little sighthound designed to fill a gap in the line-up of sighthound breeds - a medium-sized, elegant hound at home both in the show ring and in the field, about 18-24 inches at the shoulder, with an easy-care, long, silken coat in all sighthound colors and color combinations, and a steady, affectionate and confident personality. ; Typically, Silken Windhounds live very healthy, active lives. While most live into their late teens, the oldest known Silken Windhound lived a few months past her 20th birthday. ; Silken Windhounds arrived as a breed with the "D" litter whelped in 1985. In 1998 the name Silken Windhound was officially adopted and the Yahoo Windhounds list was formed. The International Silken Windhound Society, chartered in 1999, maintains all pedigrees and DNA-verified registrations for the breed. ; Silken Windhounds are now found throughout the United States as well as Austria, Commonwealth of the Bahamas, Canada, Finland, Germany, Italy, Mexico, Japan, Slovenia, Sweden, Switzerland, The Netherlands, New Zealand, Norway, United Arab Emirates, United Kingdom and Union of South Africa. ; The Silken Windhound was recognized by the United Kennel Club March 18, 2011." []
is_a: DBO:0000003 ! Hound Group

[Term]
id: DBO:0000410
name: Slovakian Wire-Haired Pointing Dog
def: "The Slovakian Wire-Haired Pointing Dog is a Continental type Braque breed that originated in Slovakia. The breed is used to point and retrieve game from land and water. ; The Slovakian Wire-Haired Pointing Dog was recognized by the United Kennel Club in 2006." []
is_a: DBO:0000003 ! Hound Group

[Term]
id: DBO:0000411
name: Smaland Hound
def: "The Smaland Hound originated in Sweden. It is a combination of scenthounds from Germany and Poland, mixed with English hounds and local spitz type dogs. As recently as the 1950's new blood has been added to the breed by recognizing dogs that were of similar type but unknown pedigree. ; The Smaland Hound was recognized by the United Kennel Club in 2006." []
is_a: DBO:0000003 ! Hound Group

[Term]
id: DBO:0000412
name: Small Swiss Hound
def: "At the turn of the century, the system of hunting in enclosed hunting grounds was introduced to Switzerland. The larger, popular Swiss Hounds were too fast for this sort of hunting, so it was decided to replace them with smaller, shorter legged scenthounds. The new, smaller breed was developed through controlled and selective breeding. They are low on leg and come in attractive colors that are similar to the medium sized Swiss Hounds. ; The Small Swiss Hound was recognized by the United Kennel Club in 2006." []
is_a: DBO:0000003 ! Hound Group

[Term]
id: DBO:0000413
name: South Russian Shepherd Dog
def: "The history of the South Russian Shepherd Dog is shrouded in antiquity. There are many variations in the descriptions of their origin that are available. One thing seems certain; this is a native Russian breed, directly descended from the wolf, with additions of local shepherd dogs and sighthounds. They were used as flock herders and guardians in the Russian steppes. ; The South Russian Shepherd Dog was originally recognized on January 1, 1996 by the United Kennel Club as the South Russian Ovcharka. Effective January 1, 2009, the breed name was changed to South Russian Shepherd Dog, and the breed moved from the Guardian Dog Group to the Herding Dog Group." []
is_a: DBO:0000008 ! Herding Group

[Term]
id: DBO:0000414
name: Spanish Greyhound
def: "The Spanish Greyhound is descended from the ancient Asian greyhounds, and is an ancestor of the English greyhound. Historically used to hunt hare, he was also sometimes used on fox and boar. ; The Spanish Greyhound was recognized by the United Kennel Club in 2006." []
is_a: DBO:0000003 ! Hound Group

[Term]
id: DBO:0000415
name: Spanish Hound
def: "The Spanish Hound was described in the 14th Century by King Alphonse XI. He is generally used for hunting small game, but is not adverse to hunting large game and is an excellent blood tracker for large game. ; The Spanish Hound was recognized by the United Kennel Club January 1, 1996." []
is_a: DBO:0000003 ! Hound Group

[Term]
id: DBO:0000416
name: Sporting Lucas Terrier
def: "The Sporting Lucas Terrier is a modern breed with a well-documented history. The breed is named for Major Sir Jocelyn Lucas, MC, KBE, MP, a Baron's son with a keen interest in hunting dogs. After returning from World War I, he began breeding Sealyhams. Concerned about the increasing size of the show-bred Sealyhams, Sir Jocelyn began crossing his hunting Sealys with Norfolk Terriers. With his partner, the Hon. Mrs. Enid Plummer, they carefully developed this small, workmanlike Terrier, designed to work in a pack and push game out of thick cover. Today, the breed is maintained primarily as a working Terrier in Great Britain, where it is used to hunt ground vermin and go to ground when required. ; The Sporting Lucas Terrier was recognized by UKC in March, 2002." []
is_a: DBO:0000005 ! Terrier Group

[Term]
id: DBO:0000417
name: Stephens' Cur
def: "Originally a strain of Mountain Cur, the little black dogs bred by the family of Hugh Stephens in Kentucky soon became sufficiently distinct that they were recognized as a separate breed. The Stephens' Stock Cur excels at hunting squirrel and raccoon, but is also used in packs on mountain lion and bears. ; The Stephens' Stock Cur was recognized by UKC on November 1, 1998." []
is_a: DBO:0000003 ! Hound Group
synonym: "STEIRISCHE RAUHHAARBRACKE" EXACT[]

[Term]
id: DBO:0000418
name: Styrian Wire-Haired Hound
def: "The breed is fairly recent, having been created in Austria from a cross between a Hanoverian Scenthound and a coarse haired Istrian Hound. The best puppies from the litter were kept and used for selective breeding to create the Styrian Coarse Haired Hound. ; The Styrian Coarse Haired Hound was recognized by the United Kennel Club in 2006." []
is_a: DBO:0000003 ! Hound Group

[Term]
id: DBO:0000419
name: Swiss Hound
def: "The Swiss Hound is a hunting dog used for hare, fox, roe deer and boar. The breed has ancient origins and was influenced by French hounds that were brought back to Switzerland by the mercenaries. The breed exists in four color varieties. ; The Swiss Hound was recognized by the United Kennel Club in 2006." []
is_a: DBO:0000003 ! Hound Group

[Term]
id: DBO:0000420
name: Treeing Cur
def: "The Cur breeds were developed in remote and rural parts of the United States. Cur breeders had little interest in standardizing the looks of their dogs - they were only interested in performance. Most Cur breeders were not well off and so they required a dog that could serve multiple purposes; hunter, guardian, and stock dog. The result was the Treeing Cur, which is the most varied in size and colors of the Cur breeds. The Treeing Cur is primarily used to hunt squirrel, raccoon, and all types of big game. ; The Treeing Cur was recognized by UKC on November 1, 1998." []
is_a: DBO:0000003 ! Hound Group

[Term]
id: DBO:0000421
name: Tyrolean Hound
def: "The Tyrolean Hound descends from the ancient Celtic hounds. Pure breeding from the old Bracke hounds began in Tyrol around 1860 and in 1896 a standard was drawn up. The Tyrolean Hound is an excellent hunting dog for the woods and mountains, used to hunt hare and fox and for tracking all sorts of wounded game. ; The Tyrolean Hound was recognized by the United Kennel Club in 2006." []
is_a: DBO:0000003 ! Hound Group

[Term]
id: DBO:0000422
name: Welsh Hound
def: "The Welsh Hound is also known as the Welsh Foxhound and Welsh Bytheuad. It is an ancient breed, thought to be descended from the extinct Celtic Hound and the old Staghound. Organized Hunts have kept well-known packs of pure Welsh Hounds for nearly 200 years. ; The Welsh Hound was recognized by the United Kennel Club January 1, 2006." []
is_a: DBO:0000003 ! Hound Group

[Term]
id: DBO:0000423
name: Westphalian Dachsbracke
def: "The Westphalian Dachsbracke is a small scenthound that originated in Germany. ; The Westphalian Dachsbracke was recognized by the United Kennel Club in 2006." []
is_a: DBO:0000003 ! Hound Group

[Term]
id: DBO:0000424
name: White Shepherd Dog
def: "The White Shepherd is a direct descendant of the German Shepherd Dog. In the first half of the twentieth century, German cavalry officer Max von Stephanitz, created the German Shepherd Dog using a variety of German sheepdogs as his foundation stock. Initially, color was not considered as long as the dog demonstrated working ability. During the late 30s, however, the white color fell into disfavor. ; There were, however, always breeders who appreciated the beauty of the white dogs and who continued to breed them. Because of their exclusion from most German Shepherd Dog breeding programs, the whites rather quickly evolved into a distinct type, and eventually into a separate breed. ; The White Shepherd was recognized by the United Kennel Club on April 14, 1999." []
is_a: DBO:0000008 ! Herding Group
synonym: "Alpine Dachsbracke" EXACT[]

[Term]
id: DBO:0000425
name: Alpine Dachsbracke
def: "Already in ancient times, a hunting/shooting dog was used which bore a remarkable resemblance in appearance to the Alpine Dachsbracke. Crown Prince Rudolf of Habsburg in 1881 and 1885 made his gamekeepers from Mursteg and Ischl include Alpine Dachsbracken on his hunting trips to Turkey and to Egypt. In 1932 the "Alpine- Erzgebirgs-Dachsbracke" was recognized by the top canine organisations in Austria as the third Scenthound breed. In 1975 the name was altered to "Alpenländische Dachsbracke" and the F.C.I. declared Austria as the country of origin. In 1991 the Alpenländische Dachsbracke was included in Section 2 of Scenthounds in the FCI nomenclature." []
is_a: DBO:0000003 ! Hound Group

[Term]
id: DBO:0000426
name: Brazilian Terrier
def: "The ancestors of the Brazilian Terrier do not originate from Brazil. In the last century and in the beginning of the present, many young Brazilians studied in the European universities, especially in France and England. These young people often returned married and their wives brought with them a small Terrier type dog. The young Brazilians and their families went back to the farms they had left. The little dog adapted to farm life and crossed with local dogs and bitches. Thus, a new model was shaped and the phenotype was fixed within a few generations. With the development of big cities, the farmers, with their families and employees were attracted by the great urban centres. In this way the little dog suffered another change in his surroundings. " []
is_a: DBO:0000005 ! Terrier Group
synonym: "EPAGNEUL NAIN CONTINENTAL" EXACT[]

[Term]
id: DBO:0000427
name: Continental Toy Spaniel
def: "nan" []
is_a: DBO:0000006 ! Companion and Toy Group

[Term]
id: DBO:0000428
name: English Toy Terrier
def: "nan" []
is_a: DBO:0000005 ! Terrier Group

[Term]
id: DBO:0000429
name: French Tricolour Hound
def: "nan" []
is_a: DBO:0000003 ! Hound Group

[Term]
id: DBO:0000430
name: French White And Orange Hound
def: "nan" []
is_a: DBO:0000003 ! Hound Group
synonym: "Virelade Hound" EXACT[]

[Term]
id: DBO:0000431
name: Gascon Saintongeois
def: "Great G.S.; In the middle of the 19th century the Count Joseph de Carayon-Latour, wanting to regenerate the declining breed of the Hound of Saintonge, crossed the last descendants with the Bleu de Gascogne of Baron Ruble, thus creating the Gascon Saintongeois but causing the extinction of the Hound of Saintonge. Small G.S.; In the middle of the 20th century some hunters from the South West of France selected the smallest subjects from their litters of Great Gascon Saintongeois and thus created this variety, intended originally for hare hunting." []
is_a: DBO:0000003 ! Hound Group

[Term]
id: DBO:0000432
name: Hanoverian Scent Hound
def: "The Hannoverscher Schweißhund has developed almost unchanged from the so called «liam hound» (leash hound) of the early Middle Ages. The Liam hound, from the breed section of the «Bracke», already played an extraordinary part at the time of the establishment of clan rights of the Germanic tribes (in about 500AD). With the invention of firearms, the methods of hunting big game altered. Dogs were needed to search for wounded game. The liam hound offered the best conditions for this and so he became a « Liam-Scenthound ». This breed description stayed in place until the hunting estate of the Kingdom of Hannover got more involved with this breed The Hanoverian hunting estate in the kingdom of Hannover developed this breed further and preserved the proven methods of handling these hounds.The Deutsche Schweißhund developed into the Hannoversche Schweißhund. Since 1894 the registered «Verein Hirschmann e.V.» has been taking care of the breed, Since then the breeding of these dogs has continued strictly with regard of their working ability and the dogs are used exclusively in hunting grounds for big game as specialists in tracking cloven-hoof game. The dissertation of Dr. Wolf-Eberhardt Barth of the "Forstlichen Fakultät of the GeorgAugust University in Gőttingen" about the subject "Der Hannoversche Schweißhund as an example of the development of the German Gundogs" (Magazines of the Landesjagdverbands Freie und Hansestadt Hamburg e.V., Landesjägerschaft, Magazine 2, Hamburg 1970, 96 S) is the scientific base for the insight into the history of this old gundog breed, which is correctly named German culture asset (Deutscher Schweißhund)." []
is_a: DBO:0000003 ! Hound Group

[Term]
id: DBO:0000433
name: Hungarian Hound-Transylvanian Scent Hound
def: "The Erdelyi Kopo is an ancient Hungarian breed, which has been determined by the peculiarities of the climate, the territory and the hunting conditions. The breed reached its climax in the Middle Ages, at a time when it was the favourite hunting dog of the aristocracy. Regarding its original use, it was pushed back into the path-less woods of the Carpathian mountains, due to the developments in agriculture and forestry. As a result of the influence of the various conditions of the terrain, two varieties of the Erdelyi Kopó evolved; the long legged and the short legged variety. These two varieties were always kept together. Originally the long legged Hungarian Hound was used for hunting big game like buffaloes and later bears, wild boars and lynxes, while the short legged Hound was used for hunting small game like foxes or hares in overgrown terrain and chamois in rocky areas. At the beginning of the 20th century, the Hungarian Hound was nearly extinct. The determined breeding was resumed in 1968. Nowadays a significant number of dogs of the long legged variety exists in Hungary and in the neighbouring Romania; the short legged variety disappeared." []
is_a: DBO:0000003 ! Hound Group

[Term]
id: DBO:0000434
name: Istrian Wire-Haired Hound
def: "The breed descends from the "East Adriatic white hound with markings". The hair is wire-haired due to the climate, where the breed was bred. These are mountain areas at the east Adriatic coast, where temperatures are low.The earliest description of the wire-haired Istrian Hound can be found in the manuscript of the Dakovoe Bishop Petar Bakic from the year 1719, where it says that the breeding of this breed was already known before the 14th century. The earliest picture document of this breed can be found in the cathedral of the Evangelist Markus in Makarska. The FCI published the first standard for the Istrian WireHaired Hound on the 6th of April 1955" []
is_a: DBO:0000003 ! Hound Group
synonym: "Segugio" EXACT[]

[Term]
id: DBO:0000435
name: Italian Wire-Haired Segugio
def: "The origin of the Segugio loses itself in the passing of time. Dogs of the same type and stature as the present Segugio adorn the statutes of Diane the Huntress (Naples Museum) and that of Diana with Bow and Arrow (Vatican Museum). In a Lombard necropolis of the province of Verona, there have recently been discovered two skeletons in perfect state of conservation, of which the conformation is identical to that of the modern Segugio. At the castle of Borso d'Este (1600), one can see a painting that gives an excellent representation of the present Segugio." []
is_a: DBO:0000003 ! Hound Group
synonym: "Segugio" EXACT[]

[Term]
id: DBO:0000436
name: Italian Short-Haired Segugio
def: "The origin of the Segugio goes back to ancient times. These dogs are certainly descendants of the primitive hounds of ancient Egypt, used for hunting game. They were introduced along the Mediterranean coast by Phoenician merchants and finally arrived in Italy. Numerous drawings executed under divers dynasties of Egyptian Pharaohs bear witness to the presence of dogs very much resembling the present Segugio. Lets point out in particular the presence of hanging ears, undoubtedly a sign of an advanced domestication. One may therefore assume that the ancient dog for the scent-hunting game, landed in Italy and gave birth to the present Segugio, whose general anatomical particularities have been maintained practically without change throughout the centuries. Dogs of the same type and stature as the present Segugio figure on statues of "Diane the huntress" in the Naples Museum and that of "Diane with bow and arrow" in the Vatican Museum. In the castle of Borso d'Este (1600) there is a painting, which represents the ideal type of the present Segugio." []
is_a: DBO:0000003 ! Hound Group

[Term]
id: DBO:0000437
name: Polish Hunting Dog
def: "Hunting with scent hounds was refered to in Polish literature as early as the XIIIth century. Poland has always been a country covered by deep forests, full of big game where the scent hound was the precious auxiliary of the hunter. Hunting with scent hounds was highly esteemed by Polish nobility as attested by XIVth century chronicles. In the XVIIth century, at least two different types of Polish scent hounds were already well distinguished. Detailed descriptions are found in XIX th century hunting literature ; in 1819 Jan Szytier (Poradnik Mysliwych) describes the Polish "brach" and the Polish scent hound; in 1821, in the magazine "Sylwan", W.Kozlowski gives a description and provides illustrations of both types, the Polish "brach" (heavier) and the Polish scent hound (lighter); the very detailed description of Ignacy Bogatynski (1823- 1825, Nauka Lowiectwa) could be used as the first breed standard. After the first World War, the Polish scent hound was still used for hunting in Poland; in the eastern regions but especially in the mountains on particularly difficult terrains. In the Podkarpacle region, the famous Polish cynologist, Jozef Pawuslewicz (1903 – 1979) hunted with Polish scent hounds; he was engaged in the development of breeding this dog. He wrote the first Breed Standard and it is thanks to him that these dogs were officially registered by the Polish Cynological Association." []
is_a: DBO:0000003 ! Hound Group

[Term]
id: DBO:0000438
name: Posavatz Hound
def: "Posavatz, the scent hound from the Save Valley is an old hound breed, which descents from a type of the "Illyrischen Hound of Red Colour with markings". In the cemetery chapel next to the village of Beram (Istrien) one can find in the fresco, dating from 1474, "The bow of the three Kings" a dark wheaten dog with dropped ears. This was the first portrayal of the Posavatz Hound. The next portrayal is the altar fresco "The motherhood of the Holy Virgin Mary" from the 16th century in the Mother of the Angels Church in Veli Losinj, where the ancestor of today's Posavatz Hound is depicted. There is also a description of this hound in a manuscript from the year 1719 of the Dakovear Bishop Petar Bakic, where it says, that the breeding of these hounds was already well known in the 14th century. Franjo Bertic describes the Posavatz Hound in the year 1854. The FCI published the first Standard for the Posavatz Hound on April 8th 1955." []
is_a: DBO:0000003 ! Hound Group

[Term]
id: DBO:0000439
name: Estonian Hound
def: "Like with many Scandinavian scent hound breeds, the East- and West European as well as British scent hound breeds form the base of Estonian Hound breed. Significant measure in breed development was a lower height at the withers to protect the bovine animals and to prevent from big hounds that might track game too fast. Thousands of hounds were summoned, evaluated and registered to be called the Estonian Hound, as the breed standard was officially approved in 1954." []
is_a: DBO:0000003 ! Hound Group

[Term]
id: DBO:0000440
name: Prague Ratter
def: "Historically, this breed has been known since the remote past of the Czech state. Because of its small size, quick movement and highly developed sense of smell it was used for killing rats (which gave it the name "Krysařík" = Ratter). This quality was gained during its long historical development. This small active dog was often seen at aristocratic feasts of Czech kings at the Prague castle. It adorned courts of Bohemian aristocracy and as a gift from Bohemian kings it came to other European rulers and later to the ordinary citizens. The search of historical facts resulted in proofs that this breed really is of Bohemian origin and can be traced to the early history of the Czech nation. In 1980 its regeneration successfully started. Pražský krysařík is again a favourite pet that lives as a family dog and is becoming popular also in many other countries worldwide." []
is_a: DBO:0000006 ! Companion and Toy Group

[Term]
id: DBO:0000441
name: Segugio Maremmano
def: "Segugio Maremmano originated from unregistered hunting dog population located in Maremma Toscana (southern part of Tuscany region, Central Italy). The breed is present in the original diffusion area since 1930s, the attempt of an official recognition by dog lovers and specialized club members traces back to those years. Thank to Dr Bosio, Veterinary and President of the specialized club for scenthounds in Italy, and to many people interested in Segugio Maremmano breed, and official standard was officially recognized. Tuscan wild board hunters created this Italian breed adapted to wild boar hunting and to the biotope of that southern area of Tuscany" []
is_a: DBO:0000003 ! Hound Group

